<?xml version="1.0"?>
<rdf:RDF xmlns="https://vocab.plataformasimple.es/def/logistics/federated/DigitalTwin#"
     xml:base="https://vocab.plataformasimple.es/def/logistics/federated/DigitalTwin"
     xmlns:dc="http://purl.org/dc/elements/1.1/"
     xmlns:owl="http://www.w3.org/2002/07/owl#"
     xmlns:rdf="http://www.w3.org/1999/02/22-rdf-syntax-ns#"
     xmlns:xml="http://www.w3.org/XML/1998/namespace"
     xmlns:xsd="http://www.w3.org/2001/XMLSchema#"
     xmlns:rdfs="http://www.w3.org/2000/01/rdf-schema#"
     xmlns:skos="http://www.w3.org/2004/02/skos/core#"
     xmlns:vann="http://purl.org/vocab/vann/"
     xmlns:terms="http://purl.org/dc/terms/">
    <owl:Ontology rdf:about="https://vocab.plataformasimple.es/def/logistics/federated/DigitalTwin">
        <owl:versionIRI rdf:resource="https://vocab.plataformasimple.es/def/logistics/federated/DigitalTwin/0.2.2"/>
        <owl:imports rdf:resource="https://ontology.tno.nl/logistics/federated/DigitalTwin"/>
        <dc:creator>Alberto Megina (Ontology Engineering Group - Universidad Politécnica de Madrid)</dc:creator>
        <dc:creator>Mario de Lucas (Ontology Engineering Group - Universidad Politécnica de Madrid)</dc:creator>
        <dc:creator>Oscar Corcho (Ontology Engineering Group - Universidad Politécnica de Madrid)</dc:creator>
        <dc:creator>XXXXX (Indra)</dc:creator>
        <dc:identifier>https://vocab.plataformasimple.es/def/logistics/federated/DigitalTwin</dc:identifier>
        <dc:title>Ontology for the representation of the extensions to the Digital Twins ontology of the Federated platform, as required by the SIMPLE project</dc:title>
        <terms:hasFormat>https://vocab.plataformasimple.es/def/logistics/federated/DigitalTwin.owl</terms:hasFormat>
        <terms:issued>2022-07-03</terms:issued>
        <terms:license>https://creativecommons.org/licenses/by/4.0</terms:license>
        <vann:preferredNamespacePrefix>simple-dt</vann:preferredNamespacePrefix>
        <vann:preferredNamespaceUri>https://vocab.plataformasimple.es/def/logistics/federated/DigitalTwin#</vann:preferredNamespaceUri>
        <rdfs:comment>This ontology has been created in the context of the SIMPLE project</rdfs:comment>
        <owl:versionInfo xml:lang="en">Release containing entities required for the representation of road and train transport</owl:versionInfo>
    </owl:Ontology>
    


    <!-- 
    ///////////////////////////////////////////////////////////////////////////////////////
    //
    // Annotation properties
    //
    ///////////////////////////////////////////////////////////////////////////////////////
     -->


    


    <!-- http://purl.org/dc/elements/1.1/identifier -->


    <owl:AnnotationProperty rdf:about="http://purl.org/dc/elements/1.1/identifier"/>
    


    <!-- http://purl.org/dc/elements/1.1/title -->


    <owl:AnnotationProperty rdf:about="http://purl.org/dc/elements/1.1/title"/>
    


    <!-- http://purl.org/dc/terms/hasFormat -->


    <owl:AnnotationProperty rdf:about="http://purl.org/dc/terms/hasFormat"/>
    


    <!-- http://purl.org/dc/terms/license -->


    <owl:AnnotationProperty rdf:about="http://purl.org/dc/terms/license"/>
    


    <!-- http://purl.org/vocab/vann/preferredNamespacePrefix -->


    <owl:AnnotationProperty rdf:about="http://purl.org/vocab/vann/preferredNamespacePrefix"/>
    


    <!-- http://purl.org/vocab/vann/preferredNamespaceUri -->


    <owl:AnnotationProperty rdf:about="http://purl.org/vocab/vann/preferredNamespaceUri"/>
    


    <!-- 
    ///////////////////////////////////////////////////////////////////////////////////////
    //
    // Object Properties
    //
    ///////////////////////////////////////////////////////////////////////////////////////
     -->


    


    <!-- https://vocab.plataformasimple.es/def/logistics/federated/DigitalTwin#relatedDocumentation -->


    <owl:ObjectProperty rdf:about="https://vocab.plataformasimple.es/def/logistics/federated/DigitalTwin#relatedDocumentation">
        <rdfs:domain rdf:resource="https://ontology.tno.nl/logistics/federated/BusinessService#BusinessTransaction"/>
        <rdfs:range rdf:resource="https://ontology.tno.nl/logistics/federated/DigitalTwin#Document"/>
        <rdfs:comment xml:lang="es">Esta propiedad permite asociar documentos a transacciones de negocio</rdfs:comment>
        <rdfs:comment xml:lang="en">This property allows associating documents to business transactions</rdfs:comment>
        <rdfs:label xml:lang="es">Documentación relacionada</rdfs:label>
        <rdfs:label xml:lang="en">related documentation</rdfs:label>
    </owl:ObjectProperty>
    


    <!-- 
    ///////////////////////////////////////////////////////////////////////////////////////
    //
    // Classes
    //
    ///////////////////////////////////////////////////////////////////////////////////////
     -->


    


    <!-- https://ontology.tno.nl/logistics/federated/BusinessService#BusinessTransaction -->


    <owl:Class rdf:about="https://ontology.tno.nl/logistics/federated/BusinessService#BusinessTransaction"/>
    


    <!-- https://ontology.tno.nl/logistics/federated/Event#Event -->


    <owl:Class rdf:about="https://ontology.tno.nl/logistics/federated/Event#Event"/>
    


    <!-- https://vocab.plataformasimple.es/def/logistics/federated/DigitalTwin#CMR -->


    <owl:Class rdf:about="https://vocab.plataformasimple.es/def/logistics/federated/DigitalTwin#CMR">
        <rdfs:subClassOf rdf:resource="https://ontology.tno.nl/logistics/federated/DigitalTwin#Document"/>
        <rdfs:comment xml:lang="en">Also known as CMR consignment note, it is a document used for the regulation of road freight transport, and serves as an international agreement. The document has been adopted by most of the European states with the purpose to regulate legal issues concerning road freight transportation</rdfs:comment>
        <rdfs:comment xml:lang="es">La carta de porte es un documento del transporte terrestre que rige el traslado de mercancía. Este documento legal, emitido por el transportista, es el equivalente al conocimiento de embarque en el transporte marítimo. En este se especifican todos los datos relevantes de la mercancía transportada</rdfs:comment>
        <rdfs:label xml:lang="en">CMR</rdfs:label>
        <rdfs:label xml:lang="es">Carta de porte</rdfs:label>
    </owl:Class>
</rdf:RDF>



<!-- Generated by the OWL API (version 5.1.18) https://github.com/owlcs/owlapi/ -->


