@prefix : <http://data.europa.eu/949/> .
@prefix owl: <http://www.w3.org/2002/07/owl#> .
@prefix rdf: <http://www.w3.org/1999/02/22-rdf-syntax-ns#> .
@prefix xml: <http://www.w3.org/XML/1998/namespace> .
@prefix xsd: <http://www.w3.org/2001/XMLSchema#> .
@prefix rdfs: <http://www.w3.org/2000/01/rdf-schema#> .
@base <http://data.europa.eu/949/> .

<http://data.europa.eu/949/> rdf:type owl:Ontology ;
                              owl:imports <http://www.opengis.net/ont/geosparql#> ;
                              <http://creativecommons.org/ns#license> <https://creativecommons.org/licenses/by/4.0/> ;
                              <http://purl.org/dc/terms/author> <https://julianrojas.org/#me> ;
                              <http://purl.org/dc/terms/contributor> <https://dylanvanassche.be/#me> ,
                                                                     <https://pietercolpaert.be/#me> ,
                                                                     "Edna Ruckhaus" ,
                                                                     "Ivo Velitchkov" ,
                                                                     "Marina Aguado" ,
                                                                     "Oscar Corcho" ,
                                                                     "Polymnia Vasilopoulou" ,
                                                                     "Wouter Beek" ;
                              <http://purl.org/dc/terms/issued> "2020-07-29"^^xsd:date ;
                              <http://purl.org/dc/terms/modified> "2022-10-20"^^xsd:date ;
                              <http://purl.org/dc/terms/publisher> "European Union Agency for Railways" ;
                              <http://purl.org/dc/terms/title> "ERA vocabulary"@en ;
                              rdfs:comment "This is the human and machine readable Vocabulary/Ontology governed by the European Union Agency for Railways. It represents the concepts and relationships linked to the sectorial legal framework and the use cases under the AgencyÂ´s remit. Currently, this vocabulary covers the European railway infrastructure and the vehicles authorized to operate over it. It is a semantic/browsable representation of the [RINF](https://www.era.europa.eu/sites/default/files/registers/docs/rinf_application_guide_for_register_en.pdf) and [ERATV](https://www.era.europa.eu/sites/default/files/registers/docs/iu-eratv_application_guide_for_register_2016-797_en.pdf) application guides that were built by domain experts in the RINF and ERATV working parties."@en ;
                              rdfs:label "ERA vocabulary"@en ;
                              owl:priorVersion "https://git.fpfis.eu/datateam/ERA/era-vocabulary/-/releases/v2.5.2"^^xsd:anyURI ;
                              owl:versionInfo "v2.5.3" ;
                              owl:versionURI "https://git.fpfis.eu/datateam/ERA/era-vocabulary/-/releases/v2.5.3"^^xsd:anyURI .

#################################################################
#    Annotation properties
#################################################################

###  http://creativecommons.org/ns#license
<http://creativecommons.org/ns#license> rdf:type owl:AnnotationProperty .


###  http://data.europa.eu/949/eratvIndex
:eratvIndex rdf:type owl:AnnotationProperty ;
            <http://purl.org/dc/terms/created> "2020-11-03"^^xsd:date ;
            <http://purl.org/dc/terms/modified> "2020-11-03"^^xsd:date ;
            rdfs:comment "Index code used in the original definition of a parameter in ERATV."@en ;
            rdfs:isDefinedBy <http://data.europa.eu/949/> ;
            rdfs:label "eratv index"@en ;
            <http://www.w3.org/2003/06/sw-vocab-status/ns#term_status> "stable" .


###  http://data.europa.eu/949/isCoreParameter
:isCoreParameter rdf:type owl:AnnotationProperty ;
                 rdfs:range xsd:boolean .


###  http://data.europa.eu/949/rinfIndex
:rinfIndex rdf:type owl:AnnotationProperty ;
           <http://purl.org/dc/terms/created> "2020-11-03"^^xsd:date ;
           <http://purl.org/dc/terms/modified> "2020-11-03"^^xsd:date ;
           rdfs:comment "Index code used in the original definition of a parameter in RINF."@en ;
           rdfs:isDefinedBy <http://data.europa.eu/949/> ;
           rdfs:label "rinf index"@en ;
           <http://www.w3.org/2003/06/sw-vocab-status/ns#term_status> "stable" .


###  http://data.europa.eu/949/routebookIndex
:routebookIndex rdf:type owl:AnnotationProperty ;
                rdfs:comment "The index of a vocabulary term in Appendix D2 Elements the infrastructure manager has to provide to the railway undertaking for the Route Book from the document Commission Implementing Regulation (EU) 2019/773 of 16 May 2019 on the technical specification for interoperability relating to the operation and traffic management subsystem of the rail system within the European Union and repealing Decision 2012/757/EU."@en ;
                rdfs:isDefinedBy <http://data.europa.eu/949/> ;
                rdfs:label "routebook index"@en ;
                <http://www.w3.org/2004/02/skos/core#definition> "The index of a vocabulary term in Appendix D2 Elements the infrastructure manager has to provide to the railway undertaking for the Route Book from the document Commission Implementing Regulation (EU) 2019/773 of 16 May 2019 on the technical specification for interoperability relating to the operation and traffic management subsystem of the rail system within the European Union and repealing Decision 2012/757/EU."@en .


###  http://purl.org/dc/elements/1.1/title
<http://purl.org/dc/elements/1.1/title> rdf:type owl:AnnotationProperty .


###  http://purl.org/dc/terms/author
<http://purl.org/dc/terms/author> rdf:type owl:AnnotationProperty .


###  http://purl.org/dc/terms/created
<http://purl.org/dc/terms/created> rdf:type owl:AnnotationProperty .


###  http://purl.org/dc/terms/isReplacedBy
<http://purl.org/dc/terms/isReplacedBy> rdf:type owl:AnnotationProperty .


###  http://purl.org/dc/terms/issued
<http://purl.org/dc/terms/issued> rdf:type owl:AnnotationProperty .


###  http://purl.org/dc/terms/modified
<http://purl.org/dc/terms/modified> rdf:type owl:AnnotationProperty .


###  http://purl.org/dc/terms/publisher
<http://purl.org/dc/terms/publisher> rdf:type owl:AnnotationProperty .


###  http://purl.org/dc/terms/source
<http://purl.org/dc/terms/source> rdf:type owl:AnnotationProperty .


###  http://www.w3.org/1999/02/22-rdf-syntax-ns#label
rdf:label rdf:type owl:AnnotationProperty .


###  http://www.w3.org/2002/07/owl#versionURI
owl:versionURI rdf:type owl:AnnotationProperty .


###  http://www.w3.org/2003/01/geo/wgs84_pos#alt
<http://www.w3.org/2003/01/geo/wgs84_pos#alt> rdf:type owl:AnnotationProperty ;
                                              rdfs:comment """The WGS84 altitude of a SpatialThing (decimal meters 
above the local reference ellipsoid).""" ;
                                              rdfs:label "altitude" ;
                                              rdfs:domain <http://www.w3.org/2003/01/geo/wgs84_pos#SpatialThing> .


###  http://www.w3.org/2003/01/geo/wgs84_pos#lat
<http://www.w3.org/2003/01/geo/wgs84_pos#lat> rdf:type owl:AnnotationProperty ;
                                              rdfs:comment "The WGS84 latitude of a SpatialThing (decimal degrees)." ;
                                              rdfs:label "latitude" ;
                                              rdfs:domain <http://www.w3.org/2003/01/geo/wgs84_pos#SpatialThing> .


###  http://www.w3.org/2003/01/geo/wgs84_pos#location
<http://www.w3.org/2003/01/geo/wgs84_pos#location> rdf:type owl:AnnotationProperty ;
                                                   rdfs:subPropertyOf <http://xmlns.com/foaf/0.1/based_near> ;
                                                   rdfs:range <http://www.w3.org/2003/01/geo/wgs84_pos#SpatialThing> .


###  http://www.w3.org/2003/01/geo/wgs84_pos#long
<http://www.w3.org/2003/01/geo/wgs84_pos#long> rdf:type owl:AnnotationProperty ;
                                               rdfs:comment "The WGS84 longitude of a SpatialThing (decimal degrees)." ;
                                               rdfs:label "longitude" ;
                                               rdfs:domain <http://www.w3.org/2003/01/geo/wgs84_pos#SpatialThing> .


###  http://www.w3.org/2003/06/sw-vocab-status/ns#term_status
<http://www.w3.org/2003/06/sw-vocab-status/ns#term_status> rdf:type owl:AnnotationProperty .


###  http://xmlns.com/foaf/0.1/based_near
<http://xmlns.com/foaf/0.1/based_near> rdf:type owl:AnnotationProperty .


#################################################################
#    Object Properties
#################################################################

###  http://data.europa.eu/949/TSIMagneticFields
:TSIMagneticFields rdf:type owl:ObjectProperty ,
                            owl:FunctionalProperty ;
                   rdfs:domain :Track ;
                   rdfs:range <http://www.w3.org/2004/02/skos/core#Concept> ;
                   :rinfIndex "1.1.1.3.9.1" ;
                   <http://purl.org/dc/terms/created> "2021-08-09"^^xsd:date ;
                   <http://purl.org/dc/terms/modified> "2021-09-12"^^xsd:date ;
                   rdfs:comment "Existence and TSI compliance of rules for magnetic fields emitted by a vehicle. The allowed values for this property belong to the SKOS Concept Scheme http://data.europa.eu/949/concepts/tsi-compliances/TSICompliances."@en ;
                   rdfs:isDefinedBy <http://data.europa.eu/949/> ;
                   rdfs:label "Existence and TSI compliance of rules for magnetic fields emitted by a vehicle"@en ;
                   <http://www.w3.org/2003/06/sw-vocab-status/ns#term_status> "stable" .


###  http://data.europa.eu/949/TSITractionHarmonics
:TSITractionHarmonics rdf:type owl:ObjectProperty ,
                               owl:FunctionalProperty ;
                      rdfs:domain :Track ;
                      rdfs:range <http://www.w3.org/2004/02/skos/core#Concept> ;
                      :rinfIndex "1.1.1.3.9.2" ;
                      <http://purl.org/dc/terms/created> "2021-08-09"^^xsd:date ;
                      <http://purl.org/dc/terms/modified> "2021-09-12"^^xsd:date ;
                      rdfs:comment "Existence and TSI compliance of limits in harmonics in the traction current of vehicles. The allowed values for this property belong to the SKOS Concept Scheme http://data.europa.eu/949/concepts/tsi-compliances/TSICompliances."@en ;
                      rdfs:isDefinedBy <http://data.europa.eu/949/> ;
                      rdfs:label "Existence and TSI compliance of limits in harmonics in the traction current of vehicles"@en ;
                      <http://www.w3.org/2003/06/sw-vocab-status/ns#term_status> "stable" .


###  http://data.europa.eu/949/authorizedCountry
:authorizedCountry rdf:type owl:ObjectProperty ;
                   rdfs:domain :VehicleType ;
                   rdfs:range <http://www.w3.org/2004/02/skos/core#Concept> ;
                   <http://purl.org/dc/terms/created> "2020-09-30"^^xsd:date ;
                   <http://purl.org/dc/terms/modified> "2020-09-30"^^xsd:date ;
                   rdfs:comment "Indicates the country(ies) in where a vehicle type has been authorized to operate. The allowed values for this property belong to the SKOS Concept Scheme http://publications.europa.eu/resource/authority/country"@en ;
                   rdfs:isDefinedBy <http://data.europa.eu/949/> ;
                   rdfs:label "authorized country"@en ;
                   <http://www.w3.org/2003/06/sw-vocab-status/ns#term_status> "stable" .


###  http://data.europa.eu/949/axleBearingConditionMonitoring
:axleBearingConditionMonitoring rdf:type owl:ObjectProperty ;
                                rdfs:domain :VehicleType ;
                                rdfs:range <http://www.w3.org/2004/02/skos/core#Concept> ;
                                :eratvIndex "4.9.2" ;
                                <http://purl.org/dc/terms/created> "2020-08-24"^^xsd:date ;
                                <http://purl.org/dc/terms/modified> "2021-08-02"^^xsd:date ;
                                rdfs:comment "Axle bearing condition monitoring. The allowed values for this property belong to the SKOS Concept Scheme http://data.europa.eu/949/concepts/axle-monitoring/AxleBearingMonitoring"@en ;
                                rdfs:isDefinedBy <http://data.europa.eu/949/> ;
                                rdfs:label "axle bearing condition monitoring"@en ;
                                <http://www.w3.org/2003/06/sw-vocab-status/ns#term_status> "stable" .


###  http://data.europa.eu/949/category
:category rdf:type owl:ObjectProperty ,
                   owl:FunctionalProperty ;
          rdfs:domain :VehicleType ;
          rdfs:range <http://www.w3.org/2004/02/skos/core#Concept> ;
          :eratvIndex 1.4 ;
          <http://purl.org/dc/terms/created> "2020-07-29"^^xsd:date ;
          <http://purl.org/dc/terms/modified> "2021-08-03"^^xsd:date ;
          rdfs:comment "Vehicle category. The allowed values for this property belong to the SKOS Concept Scheme http://data.europa.eu/949/concepts/vehicle-types/Categories."@en ;
          rdfs:isDefinedBy <http://data.europa.eu/949/> ;
          rdfs:label "vehicle category"@en ;
          <http://www.w3.org/2003/06/sw-vocab-status/ns#term_status> "stable" .


###  http://data.europa.eu/949/composedOf
:composedOf rdf:type owl:ObjectProperty ;
            rdfs:domain [ rdf:type owl:Class ;
                          owl:unionOf ( :GradientCurve
                                        :SpeedSection
                                      )
                        ] ;
            rdfs:range :LinearLocation ;
            <http://purl.org/dc/terms/created> "2022-09-12"^^xsd:date ;
            rdfs:comment """The speed section and the gradient curve are composed of zero or more
linear locations."""@en ;
            rdfs:isDefinedBy "http://data.europa.eu/949/"^^xsd:anyURI ;
            rdfs:label "composed of"@en ;
            <http://www.w3.org/2003/06/sw-vocab-status/ns#term_status> "stable" .


###  http://data.europa.eu/949/contactLineSystem
:contactLineSystem rdf:type owl:ObjectProperty ;
                   rdfs:domain :Track ;
                   rdfs:range :ContactLineSystem ;
                   <http://purl.org/dc/terms/created> "2020-08-24"^^xsd:date ;
                   <http://purl.org/dc/terms/modified> "2021-09-11"^^xsd:date ;
                   rdfs:comment "Contact line system present in the section of line."@en ;
                   rdfs:isDefinedBy <http://data.europa.eu/949/> ;
                   rdfs:label "contact line system"@en ;
                   <http://www.w3.org/2003/06/sw-vocab-status/ns#term_status> "stable" .


###  http://data.europa.eu/949/contactLineSystemType
:contactLineSystemType rdf:type owl:ObjectProperty ;
                       rdfs:domain :ContactLineSystem ;
                       rdfs:range <http://www.w3.org/2004/02/skos/core#Concept> ;
                       :isCoreParameter "true"^^xsd:boolean ;
                       :rinfIndex "1.1.1.2.2.1.1" ;
                       <http://purl.org/dc/terms/created> "2021-08-06"^^xsd:date ;
                       <http://purl.org/dc/terms/modified> "2021-08-06"^^xsd:date ;
                       rdfs:comment "Indication of the type of the contact line system. The allowed values for this property belong to the SKOS Concept Scheme http://data.europa.eu/949/concepts/contact-line-systems/ContactLineSystems"@en ;
                       rdfs:isDefinedBy <http://data.europa.eu/949/> ;
                       rdfs:label "Type of contact line system"@en ;
                       <http://www.w3.org/2003/06/sw-vocab-status/ns#term_status> "stable" .


###  http://data.europa.eu/949/contactStripMaterial
:contactStripMaterial rdf:type owl:ObjectProperty ;
                      rdfs:domain [ rdf:type owl:Class ;
                                    owl:unionOf ( :Track
                                                  :VehicleType
                                                )
                                  ] ;
                      rdfs:range <http://www.w3.org/2004/02/skos/core#Concept> ;
                      :eratvIndex "4.10.10" ;
                      :rinfIndex "1.1.1.2.3.4" ;
                      <http://purl.org/dc/terms/created> "2020-08-25"^^xsd:date ;
                      <http://purl.org/dc/terms/modified> "2021-09-12"^^xsd:date ;
                      rdfs:comment "Indication of which contact strip materials are permitted to be used. The allowed values for this property belong to the SKOS Concept Scheme http://data.europa.eu/949/concepts/contact-strip-materials/ContactStripMaterials"@en ;
                      rdfs:isDefinedBy <http://data.europa.eu/949/> ;
                      rdfs:label "Permitted contact strip material"@en ;
                      <http://www.w3.org/2003/06/sw-vocab-status/ns#term_status> "stable" .


###  http://data.europa.eu/949/dataGSMRNetwork
:dataGSMRNetwork rdf:type owl:ObjectProperty ,
                          owl:FunctionalProperty ;
                 rdfs:domain :VehicleType ;
                 rdfs:range <http://www.w3.org/2004/02/skos/core#Concept> ;
                 :eratvIndex "4.13.2.11" ;
                 <http://purl.org/dc/terms/created> "2020-08-31"^^xsd:date ;
                 <http://purl.org/dc/terms/modified> "2021-08-02"^^xsd:date ;
                 rdfs:comment "Data SIM Card GSM-R Home Network. The allowed values for this property belong to the SKOS Concept Scheme http://data.europa.eu/949/concepts/gsmr-networks/GSMRNetworks"@en ;
                 rdfs:isDefinedBy <http://data.europa.eu/949/> ;
                 rdfs:label "data GSM-R network"@en ;
                 <http://www.w3.org/2003/06/sw-vocab-status/ns#term_status> "stable" .


###  http://data.europa.eu/949/dataRadioCompatible
:dataRadioCompatible rdf:type owl:ObjectProperty ;
                     rdfs:domain [ rdf:type owl:Class ;
                                   owl:unionOf ( :Track
                                                 :VehicleType
                                               )
                                 ] ;
                     rdfs:range <http://www.w3.org/2004/02/skos/core#Concept> ;
                     :eratvIndex "4.13.2.8" ;
                     :rinfIndex "1.1.1.3.3.10" ;
                     <http://purl.org/dc/terms/created> "2020-08-31"^^xsd:date ;
                     <http://purl.org/dc/terms/modified> "2021-09-12"^^xsd:date ;
                     rdfs:comment """Radio requirements used for demonstrating technical compatibility voice.
 The allowed values for this property belong to the SKOS Concept Scheme http://data.europa.eu/949/concepts/data-radio-system-compatibilities/DataRadioSystemCompatibilities. This concept scheme is temporatily non-deferenceable."""@en ;
                     rdfs:isDefinedBy <http://data.europa.eu/949/> ;
                     rdfs:label "Radio system compatibility data"@en ;
                     <http://www.w3.org/2003/06/sw-vocab-status/ns#term_status> "stable" .


###  http://data.europa.eu/949/eddyCurrentBraking
:eddyCurrentBraking rdf:type owl:ObjectProperty ,
                             owl:FunctionalProperty ;
                    rdfs:domain :Track ;
                    rdfs:range <http://www.w3.org/2004/02/skos/core#Concept> ;
                    :isCoreParameter "true"^^xsd:boolean ;
                    :rinfIndex "1.1.1.1.6.2" ;
                    <http://purl.org/dc/terms/created> "2020-08-24"^^xsd:date ;
                    <http://purl.org/dc/terms/modified> "2022-09-06"^^xsd:date ;
                    rdfs:comment """Use of eddy current brakes. The allowed values for this property belong to the SKOS Concept Scheme http://data.europa.eu/949/concepts/eddy-current-braking/EddyCurrentBraking
This property has been modified to be a RINF parameter (its eratvIndex is deleted). It is treated as a SKOS by RINF and as a boolean by ERATV. A new ERATV datatype property has been defined, eddyCurrentBrakingFitted with boolean values."""@en ;
                    rdfs:isDefinedBy <http://data.europa.eu/949/> ;
                    rdfs:label "Use of eddy current brakes"@en ;
                    <http://www.w3.org/2003/06/sw-vocab-status/ns#term_status> "stable" .


###  http://data.europa.eu/949/elementA
:elementA rdf:type owl:ObjectProperty ;
          rdfs:domain :NetRelation ;
          rdfs:range :NetElement ;
          <http://purl.org/dc/terms/created> "2021-04-01"^^xsd:date ;
          <http://purl.org/dc/terms/modified> "2021-04-01"^^xsd:date ;
          rdfs:comment "References the first topological object in an oriented relation."@en ;
          rdfs:isDefinedBy <http://data.europa.eu/949/> ;
          rdfs:label "element A"@en ;
          <http://www.w3.org/2003/06/sw-vocab-status/ns#term_status> "stable" .


###  http://data.europa.eu/949/elementB
:elementB rdf:type owl:ObjectProperty ;
          rdfs:domain :NetRelation ;
          rdfs:range :NetElement ;
          <http://purl.org/dc/terms/created> "2021-04-01"^^xsd:date ;
          <http://purl.org/dc/terms/modified> "2021-04-01"^^xsd:date ;
          rdfs:comment "References the second topological object in an oriented relation."@en ;
          rdfs:isDefinedBy <http://data.europa.eu/949/> ;
          rdfs:label "element B"@en ;
          <http://www.w3.org/2003/06/sw-vocab-status/ns#term_status> "stable" .


###  http://data.europa.eu/949/elementPart
:elementPart rdf:type owl:ObjectProperty ;
             rdfs:domain :NetElement ;
             rdfs:range :NetElement ;
             <http://purl.org/dc/terms/created> "2021-04-01"^^xsd:date ;
             <http://purl.org/dc/terms/modified> "2021-04-01"^^xsd:date ;
             rdfs:comment "References the topology object of a higher-granularity level which contains a lower-granularity topology object."@en ;
             rdfs:isDefinedBy <http://data.europa.eu/949/> ;
             rdfs:label "element part"@en ;
             <http://www.w3.org/2003/06/sw-vocab-status/ns#term_status> "stable" .


###  http://data.europa.eu/949/endCouplingType
:endCouplingType rdf:type owl:ObjectProperty ;
                 rdfs:domain :VehicleType ;
                 rdfs:range <http://www.w3.org/2004/02/skos/core#Concept> ;
                 :eratvIndex "4.9.1" ;
                 <http://purl.org/dc/terms/created> "2021-08-31"^^xsd:date ;
                 <http://purl.org/dc/terms/modified> "2021-08-31"^^xsd:date ;
                 rdfs:comment "Type of end coupling (indicating tensile and compressive forces). The allowed values for this property belong to the SKOS Concept Scheme http://data.europa.eu/949/concepts/end-coupling-type/EndCouplingType."@en ;
                 rdfs:isDefinedBy <http://data.europa.eu/949/> ;
                 rdfs:label "end coupling type"@en ;
                 <http://www.w3.org/2003/06/sw-vocab-status/ns#term_status> "stable" .


###  http://data.europa.eu/949/endLocation
:endLocation rdf:type owl:ObjectProperty ;
             rdfs:subPropertyOf <http://www.opengis.net/ont/geosparql#hasGeometry> ,
                                <http://www.w3.org/2003/01/geo/wgs84_pos#location> ;
             rdfs:domain :Tunnel ;
             rdfs:range [ rdf:type owl:Class ;
                          owl:unionOf ( <http://www.opengis.net/ont/geosparql#Geometry>
                                        <http://www.w3.org/2003/01/geo/wgs84_pos#Point>
                                      )
                        ] ;
             :isCoreParameter "true"^^xsd:boolean ;
             :rinfIndex "1.1.1.1.8.4" ;
             <http://purl.org/dc/terms/created> "2020-07-29"^^xsd:date ;
             <http://purl.org/dc/terms/modified> "2021-08-11"^^xsd:date ;
             rdfs:comment "References the geolocation of the end of a tunnel."@en ;
             rdfs:isDefinedBy <http://data.europa.eu/949/> ;
             rdfs:label "End of tunnel"@en ;
             <http://www.w3.org/2003/06/sw-vocab-status/ns#term_status> "stable" .


###  http://data.europa.eu/949/energySupplySystem
:energySupplySystem rdf:type owl:ObjectProperty ;
                    rdfs:domain [ rdf:type owl:Class ;
                                  owl:unionOf ( :ContactLineSystem
                                                :VehicleType
                                              )
                                ] ;
                    rdfs:range <http://www.w3.org/2004/02/skos/core#Concept> ;
                    :eratvIndex "4.10.1" ;
                    :isCoreParameter "true"^^xsd:boolean ;
                    :rinfIndex "1.1.1.2.2.1.2" ;
                    <http://purl.org/dc/terms/created> "2020-08-24"^^xsd:date ;
                    <http://purl.org/dc/terms/modified> "2021-08-06"^^xsd:date ;
                    rdfs:comment "Indication of the traction supply system (nominal voltage and frequency). Type of end coupling (indicating tensile and compressive forces). The allowed values for this property belong to the SKOS Concept Scheme http://data.europa.eu/949/concepts/energy-supply-systems/EnergySupplySystems"@en ;
                    rdfs:isDefinedBy <http://data.europa.eu/949/> ;
                    rdfs:label "Energy supply system"@en ;
                    <http://www.w3.org/2003/06/sw-vocab-status/ns#term_status> "stable" .


###  http://data.europa.eu/949/etcsBaseline
:etcsBaseline rdf:type owl:ObjectProperty ;
              rdfs:domain [ rdf:type owl:Class ;
                            owl:unionOf ( :ETCSLevel
                                          :VehicleType
                                        )
                          ] ;
              rdfs:range <http://www.w3.org/2004/02/skos/core#Concept> ;
              :eratvIndex "4.13.1.2" ;
              :rinfIndex "1.1.1.3.2.2" ;
              <http://purl.org/dc/terms/created> "2021-08-07"^^xsd:date ;
              <http://purl.org/dc/terms/modified> "2021-08-31"^^xsd:date ;
              rdfs:comment "ETCS baseline installed lineside/on-board. The allowed values for this property belong to the SKOS Concept Scheme http://data.europa.eu/949/concepts/etcs-baselines/ETCSBaselines"@en ;
              rdfs:isDefinedBy <http://data.europa.eu/949/> ;
              rdfs:label "ETCS baseline"@en ;
              <http://www.w3.org/2003/06/sw-vocab-status/ns#term_status> "stable" .


###  http://data.europa.eu/949/etcsDegradedSituation
:etcsDegradedSituation rdf:type owl:ObjectProperty ;
                       rdfs:domain :Track ;
                       rdfs:range <http://www.w3.org/2004/02/skos/core#Concept> ;
                       :rinfIndex "1.1.1.3.10.1" ;
                       <http://purl.org/dc/terms/created> "2021-08-09"^^xsd:date ;
                       <http://purl.org/dc/terms/modified> "2021-09-12"^^xsd:date ;
                       rdfs:comment "ERTMS / ETCS application level for degraded situation related to the track side equipment. The allowed values for this property belong to the SKOS Concept Scheme http://data.europa.eu/949/concepts/etcs-situation/ETCSSituations"@en ;
                       rdfs:isDefinedBy <http://data.europa.eu/949/> ;
                       rdfs:label "ETCS level for degraded situation"@en ;
                       <http://www.w3.org/2003/06/sw-vocab-status/ns#term_status> "stable" .


###  http://data.europa.eu/949/etcsEquipmentOnBoardLevel
:etcsEquipmentOnBoardLevel rdf:type owl:ObjectProperty ,
                                    owl:FunctionalProperty ;
                           rdfs:domain :VehicleType ;
                           rdfs:range <http://www.w3.org/2004/02/skos/core#Concept> ;
                           :eratvIndex "4.13.1.1" ;
                           <http://purl.org/dc/terms/created> "2021-08-31"^^xsd:date ;
                           <http://purl.org/dc/terms/modified> "2021-08-31"^^xsd:date ;
                           rdfs:comment "ETCS equipment on-board and its level. The allowed values for this property belong to the SKOS Concept Scheme http://data.europa.eu/949/concepts/etcs-equipment-on-board-level/ETCSEquipmentLevels."@en ;
                           rdfs:isDefinedBy <http://data.europa.eu/949/> ;
                           rdfs:label "ETCS equipment level"@en ;
                           <http://www.w3.org/2003/06/sw-vocab-status/ns#term_status> "stable" .


###  http://data.europa.eu/949/etcsInfill
:etcsInfill rdf:type owl:ObjectProperty ,
                     owl:FunctionalProperty ;
            rdfs:domain [ rdf:type owl:Class ;
                          owl:unionOf ( :Track
                                        :VehicleType
                                      )
                        ] ;
            rdfs:range <http://www.w3.org/2004/02/skos/core#Concept> ;
            :eratvIndex "4.13.1.3" ;
            :rinfIndex "1.1.1.3.2.4" ;
            <http://purl.org/dc/terms/created> "2021-08-08"^^xsd:date ;
            <http://purl.org/dc/terms/modified> "2021-09-12"^^xsd:date ;
            rdfs:comment "Information about installed trackside/on-board equipment capable to transmit infill information by loop or GSM-R for level 1 installation. The allowed values for this property belong to the SKOS Concept Scheme http://data.europa.eu/949/concepts/etcs-infills/ETCSInfills"@en ;
            rdfs:isDefinedBy <http://data.europa.eu/949/> ;
            rdfs:label "ETCS infill installed lineside"@en ;
            <http://www.w3.org/2003/06/sw-vocab-status/ns#term_status> "stable" .


###  http://data.europa.eu/949/etcsLevel
:etcsLevel rdf:type owl:ObjectProperty ;
           rdfs:domain :Track ;
           rdfs:range :ETCSLevel ;
           <http://purl.org/dc/terms/created> "2021-08-07"^^xsd:date ;
           <http://purl.org/dc/terms/modified> "2021-09-12"^^xsd:date ;
           rdfs:comment "ETCS level available in the section of line. The allowed values for this property belong to the SKOS Concept Scheme http://data.europa.eu/949/concepts/etcs-levels/ETCSLevels"@en ;
           rdfs:isDefinedBy <http://data.europa.eu/949/> ;
           rdfs:label "etcs level"@en ;
           <http://www.w3.org/2003/06/sw-vocab-status/ns#term_status> "stable" .


###  http://data.europa.eu/949/etcsLevelType
:etcsLevelType rdf:type owl:ObjectProperty ;
               rdfs:domain :ETCSLevel ;
               rdfs:range <http://www.w3.org/2004/02/skos/core#Concept> ;
               :isCoreParameter "true"^^xsd:boolean ;
               :rinfIndex "1.1.1.3.2.1" ;
               <http://purl.org/dc/terms/created> "2021-08-07"^^xsd:date ;
               <http://purl.org/dc/terms/modified> "2021-08-07"^^xsd:date ;
               rdfs:comment "ERTMS / ETCS application level which expresses the possible operating relationships between track and train. The allowed values for this property belong to the SKOS Concept Scheme http://data.europa.eu/949/concepts/etcs-levels/ETCSLevels"@en ;
               rdfs:isDefinedBy <http://data.europa.eu/949/> ;
               rdfs:label "ETCS level type"@en ;
               <http://www.w3.org/2003/06/sw-vocab-status/ns#term_status> "stable" .


###  http://data.europa.eu/949/etcsMVersion
:etcsMVersion rdf:type owl:ObjectProperty ,
                       owl:FunctionalProperty ;
              rdfs:domain :Track ;
              rdfs:range <http://www.w3.org/2004/02/skos/core#Concept> ;
              :rinfIndex "1.1.1.3.2.10" ;
              <http://purl.org/dc/terms/created> "2021-08-08"^^xsd:date ;
              <http://purl.org/dc/terms/modified> "2021-09-12"^^xsd:date ;
              rdfs:comment "ETCS M_version according to SRS 7.5.1.9. The allowed values for this property belong to the SKOS Concept Scheme http://data.europa.eu/949/concepts/etcs-m-versions/ETCSMVersions"@en ;
              rdfs:isDefinedBy <http://data.europa.eu/949/> ;
              rdfs:label "ETCS M_version"@en ;
              <http://www.w3.org/2003/06/sw-vocab-status/ns#term_status> "stable" .


###  http://data.europa.eu/949/etcsSystemCompatibility
:etcsSystemCompatibility rdf:type owl:ObjectProperty ;
                         rdfs:domain [ rdf:type owl:Class ;
                                       owl:unionOf ( :Track
                                                     :VehicleType
                                                   )
                                     ] ;
                         rdfs:range <http://www.w3.org/2004/02/skos/core#Concept> ;
                         :eratvIndex "4.13.1.8" ;
                         :isCoreParameter "true"^^xsd:boolean ;
                         :rinfIndex "1.1.1.3.2.9" ;
                         <http://purl.org/dc/terms/created> "2020-08-31"^^xsd:date ;
                         <http://purl.org/dc/terms/modified> "2021-09-12"^^xsd:date ;
                         rdfs:comment "ETCS requirements used for demonstrating technical compatibility. The allowed values for this property belong to the SKOS Concept Scheme http://data.europa.eu/949/concepts/etcs-system-compatibilities/ETCSSystemCompatibilities"@en ;
                         rdfs:isDefinedBy <http://data.europa.eu/949/> ;
                         rdfs:label "ETCS system compatibility"@en ;
                         <http://www.w3.org/2003/06/sw-vocab-status/ns#term_status> "stable" .


###  http://data.europa.eu/949/fireSafetyCategory
:fireSafetyCategory rdf:type owl:ObjectProperty ,
                             owl:FunctionalProperty ;
                    rdfs:domain :VehicleType ;
                    rdfs:range <http://www.w3.org/2004/02/skos/core#Concept> ;
                    :eratvIndex "4.4.1" ;
                    <http://purl.org/dc/terms/created> "2020-08-29"^^xsd:date ;
                    <http://purl.org/dc/terms/modified> "2021-08-03"^^xsd:date ;
                    rdfs:comment "Fire safety category for tunnels. The allowed values for this property belong to the SKOS Concept Scheme http://data.europa.eu/949/concepts/rolling-stock-fire/Categories."@en ;
                    rdfs:isDefinedBy <http://data.europa.eu/949/> ;
                    rdfs:label "fire safety category"@en ;
                    <http://www.w3.org/2003/06/sw-vocab-status/ns#term_status> "stable" .


###  http://data.europa.eu/949/freightCorridor
:freightCorridor rdf:type owl:ObjectProperty ;
                 rdfs:domain :Track ;
                 rdfs:range <http://www.w3.org/2004/02/skos/core#Concept> ;
                 :rinfIndex "1.1.1.1.2.3" ,
                            "1.2.1.0.2.3" ;
                 <http://purl.org/dc/terms/created> "2021-08-03"^^xsd:date ;
                 <http://purl.org/dc/terms/modified> "2021-08-11"^^xsd:date ;
                 rdfs:comment "Railway Freight Corridor that the line is designated to. Fire safety category for tunnels. The allowed values for this property belong to the SKOS Concept Scheme http://data.europa.eu/949/concepts/freight-corridor/FreightCorridors"@en ;
                 rdfs:isDefinedBy <http://data.europa.eu/949/> ;
                 rdfs:label "Part of a Railway freight corridor"@en ;
                 <http://www.w3.org/2003/06/sw-vocab-status/ns#term_status> "stable" .


###  http://data.europa.eu/949/frenchTrainDetectionSystemLimitation
:frenchTrainDetectionSystemLimitation rdf:type owl:ObjectProperty ;
                                      rdfs:domain :Track ;
                                      rdfs:range <http://www.w3.org/2004/02/skos/core#Concept> ;
                                      :rinfIndex "1.1.1.3.7.1.4" ;
                                      <http://purl.org/dc/terms/created> "2020-08-24"^^xsd:date ;
                                      <http://purl.org/dc/terms/modified> "2021-09-12"^^xsd:date ;
                                      rdfs:comment "Section with train detection limitation, specific for route compatibility check on French network. The allowed values for this property belong to the SKOS Concept Scheme http://data.europa.eu/949/concepts/train-detection/FrenchTrainDetectionSystemLimitations."@en ;
                                      rdfs:isDefinedBy <http://data.europa.eu/949/> ;
                                      rdfs:label "Section with train detection limitation, only for the French network"@en ;
                                      <http://www.w3.org/2003/06/sw-vocab-status/ns#term_status> "stable" .


###  http://data.europa.eu/949/gaugingProfile
:gaugingProfile rdf:type owl:ObjectProperty ;
                rdfs:domain [ rdf:type owl:Class ;
                              owl:unionOf ( :Track
                                            :VehicleType
                                          )
                            ] ;
                rdfs:range <http://www.w3.org/2004/02/skos/core#Concept> ;
                :eratvIndex "4.2.1" ;
                :isCoreParameter "true"^^xsd:boolean ;
                :rinfIndex "1.1.1.1.3.1.1" ,
                           "1.2.1.0.3.4" ;
                <http://purl.org/dc/terms/created> "2020-07-29"^^xsd:date ;
                <http://purl.org/dc/terms/modified> "2021-09-10"^^xsd:date ;
                rdfs:comment "Gauges as defined in European standard or other local gauges, including lower or upper part. The allowed values for this property belong to the SKOS Concept Scheme http://data.europa.eu/949/concepts/gaugings/GaugingProfiles"@en ;
                rdfs:isDefinedBy <http://data.europa.eu/949/> ;
                rdfs:label "Gauging"@en ;
                <http://www.w3.org/2003/06/sw-vocab-status/ns#term_status> "stable" .


###  http://data.europa.eu/949/gsmRActiveMobiles
:gsmRActiveMobiles rdf:type owl:ObjectProperty ,
                            owl:FunctionalProperty ;
                   rdfs:domain :Track ;
                   rdfs:range <http://www.w3.org/2004/02/skos/core#Concept> ;
                   :rinfIndex "1.1.1.3.3.2" ;
                   <http://purl.org/dc/terms/created> "2021-08-08"^^xsd:date ;
                   <http://purl.org/dc/terms/modified> "2021-09-12"^^xsd:date ;
                   rdfs:comment "Number of active GSM-R mobiles (EDOR) or simultaneous communication session on-board for ETCS Level 2 (or level 3) needed to perform radio block centre handovers without having an operational disruption. The allowed values for this property belong to the SKOS Concept Scheme http://data.europa.eu/949/concepts/gsmr-number-active-mobiles/NumberActiveMobiles"@en ;
                   rdfs:isDefinedBy <http://data.europa.eu/949/> ;
                   rdfs:label "Advised required number of active GSM-R mobiles (EDOR) or simultaneous communication session on-board for ETCS Level 2 (or level 3) needed to perform radio block centre handovers without having an operational disruption"@en ;
                   <http://www.w3.org/2003/06/sw-vocab-status/ns#term_status> "stable" .


###  http://data.europa.eu/949/gsmROptionalFunctions
:gsmROptionalFunctions rdf:type owl:ObjectProperty ;
                       rdfs:domain :Track ;
                       rdfs:range <http://www.w3.org/2004/02/skos/core#Concept> ;
                       :rinfIndex "1.1.1.3.3.3" ;
                       <http://purl.org/dc/terms/created> "2021-08-08"^^xsd:date ;
                       <http://purl.org/dc/terms/modified> "2021-09-12"^^xsd:date ;
                       rdfs:comment "Use of optional GSM-R functions which might improve operation on the line. They are for information only and not for network access criteria. The allowed values for this property belong to the SKOS Concept Scheme http://data.europa.eu/949/concepts/gsmr-optional-functions/OptionalFunctions"@en ;
                       rdfs:isDefinedBy <http://data.europa.eu/949/> ;
                       rdfs:label "Optional GSM-R functions"@en ;
                       <http://www.w3.org/2003/06/sw-vocab-status/ns#term_status> "stable" .


###  http://data.europa.eu/949/gsmRRadioDataCommunication
:gsmRRadioDataCommunication rdf:type owl:ObjectProperty ,
                                     owl:FunctionalProperty ;
                            rdfs:domain :VehicleType ;
                            rdfs:range <http://www.w3.org/2004/02/skos/core#Concept> ;
                            :eratvIndex "4.13.2.7" ;
                            <http://purl.org/dc/terms/created> "2021-08-31"^^xsd:date ;
                            <http://purl.org/dc/terms/modified> "2021-08-31"^^xsd:date ;
                            rdfs:comment "GSM-R Radio Data communication on board and its Baseline. The allowed values for this property belong to the SKOS Concept Scheme http://data.europa.eu/949/concepts/gsm-r-radio-data-communication/GSMRRadioDataCommunications."@en ;
                            rdfs:isDefinedBy <http://data.europa.eu/949/> ;
                            rdfs:label "GSM-R radio data communication"@en ;
                            <http://www.w3.org/2003/06/sw-vocab-status/ns#term_status> "stable" .


###  http://data.europa.eu/949/gsmRVersion
:gsmRVersion rdf:type owl:ObjectProperty ,
                      owl:FunctionalProperty ;
             rdfs:domain [ rdf:type owl:Class ;
                           owl:unionOf ( :Track
                                         :VehicleType
                                       )
                         ] ;
             rdfs:range <http://www.w3.org/2004/02/skos/core#Concept> ;
             :eratvIndex "4.13.2.1" ;
             :isCoreParameter "true"^^xsd:boolean ;
             :rinfIndex "1.1.1.3.3.1" ;
             <http://purl.org/dc/terms/created> "2021-08-08"^^xsd:date ;
             <http://purl.org/dc/terms/modified> "2021-09-12"^^xsd:date ;
             rdfs:comment "GSM-R version installed lineside/on-board. The allowed values for this property belong to the SKOS Concept Scheme http://data.europa.eu/949/concepts/gsmr-versions/GSMRVersions"@en ;
             rdfs:isDefinedBy <http://data.europa.eu/949/> ;
             rdfs:label "GSM-R version"@en ;
             <http://www.w3.org/2003/06/sw-vocab-status/ns#term_status> "stable" .


###  http://data.europa.eu/949/gsmrNetworkCoverage
:gsmrNetworkCoverage rdf:type owl:ObjectProperty ;
                     rdfs:domain :Track ;
                     rdfs:range <http://www.w3.org/2004/02/skos/core#Concept> ;
                     :rinfIndex "1.1.1.3.3.5" ;
                     <http://purl.org/dc/terms/created> "2020-08-31"^^xsd:date ;
                     <http://purl.org/dc/terms/modified> "2021-09-12"^^xsd:date ;
                     rdfs:comment "GSM-R networks covered by a roaming agreement. The allowed values for this property belong to the SKOS Concept Scheme http://data.europa.eu/949/concepts/gsmr-networks/GSMRNetworks"@en ;
                     rdfs:isDefinedBy <http://data.europa.eu/949/> ;
                     rdfs:label "GSM-R networks covered by a roaming agreement"@en ;
                     <http://www.w3.org/2003/06/sw-vocab-status/ns#term_status> "stable" .


###  http://data.europa.eu/949/hasAbstraction
:hasAbstraction rdf:type owl:ObjectProperty ;
                owl:inverseOf :hasImplementation ;
                rdfs:domain :PhysicalImplementationFeature ;
                rdfs:range :TopologicalObject ;
                <http://purl.org/dc/terms/created> "2020-07-29"^^xsd:date ;
                <http://purl.org/dc/terms/modified> "2021-04-13"^^xsd:date ;
                rdfs:comment "Property that links a physical entity with its topological abstraction representation."@en ;
                rdfs:isDefinedBy <http://data.europa.eu/949/> ;
                rdfs:label "has abstraction"@en ;
                <http://www.w3.org/2003/06/sw-vocab-status/ns#term_status> "stable" .


###  http://data.europa.eu/949/hasImplementation
:hasImplementation rdf:type owl:ObjectProperty ;
                   rdfs:domain :TopologicalObject ;
                   rdfs:range :PhysicalImplementationFeature ;
                   <http://purl.org/dc/terms/created> "2020-07-29"^^xsd:date ;
                   <http://purl.org/dc/terms/modified> "2021-04-13"^^xsd:date ;
                   rdfs:comment "Property that links a topological abstraction entity with its physical representation."@en ;
                   rdfs:isDefinedBy <http://data.europa.eu/949/> ;
                   rdfs:label "has implementation"@en ;
                   <http://www.w3.org/2003/06/sw-vocab-status/ns#term_status> "stable" .


###  http://data.europa.eu/949/hasSignal
:hasSignal rdf:type owl:ObjectProperty ;
           rdfs:domain :NetElement ;
           rdfs:range :Signal ;
           <http://purl.org/dc/terms/created> "2021-04-01"^^xsd:date ;
           <http://purl.org/dc/terms/modified> "2021-04-01"^^xsd:date ;
           rdfs:comment "References a signal associated with a topology object."@en ;
           rdfs:isDefinedBy <http://data.europa.eu/949/> ;
           rdfs:label "has signal"@en ;
           <http://www.w3.org/2003/06/sw-vocab-status/ns#term_status> "stable" .


###  http://data.europa.eu/949/hotAxleBoxDetectorDirection
:hotAxleBoxDetectorDirection rdf:type owl:ObjectProperty ;
                             rdfs:subPropertyOf owl:topObjectProperty ;
                             rdfs:domain :Track ;
                             rdfs:range <http://www.w3.org/2004/02/skos/core#Concept> ;
                             :rinfIndex "1.1.1.1.7.9" ;
                             <http://purl.org/dc/terms/created> "2022-07-08"^^xsd:date ;
                             rdfs:comment """Direction of measurement of trackside HABD. Specific for the French Italian and Swedish networks.

This property was previously a datatype property with domain Track and range string. As its values are a list of three predefined values, it is now a SKOS. The allowed values for this property belong to the SKOS Concept Scheme http://data.europa.eu/949/concepts/hot-axle/HotAxleBoxDetectorDirections"""@en ;
                             rdfs:isDefinedBy <http://data.europa.eu/949/> ;
                             rdfs:label "hot axle box detector direction"@en .


###  http://data.europa.eu/949/inCountry
:inCountry rdf:type owl:ObjectProperty ;
           rdfs:domain :PhysicalImplementationFeature ;
           rdfs:range <http://www.w3.org/2004/02/skos/core#Concept> ;
           <http://purl.org/dc/terms/created> "2020-09-01"^^xsd:date ;
           <http://purl.org/dc/terms/modified> "2020-11-20"^^xsd:date ;
           rdfs:comment "Indicates the country in which an entity resides. The allowed values for this property belong to the SKOS Concept Scheme http://publications.europa.eu/resource/authority/country"@en ;
           rdfs:isDefinedBy <http://data.europa.eu/949/> ;
           rdfs:label "in country"@en ;
           <http://www.w3.org/2003/06/sw-vocab-status/ns#term_status> "stable" .


###  http://data.europa.eu/949/infrastructureMgr
:infrastructureMgr rdf:type owl:ObjectProperty ;
                   rdfs:domain :PhysicalImplementationFeature ;
                   rdfs:range :InfrastructureManager ;
                   <http://purl.org/dc/terms/created> "2022-07-07"@en ;
                   rdfs:comment "Relates any feature implemented in the European railway infrastructure with its infrastructure manager."@en ;
                   rdfs:isDefinedBy <http://data.europa.eu/949/> ;
                   rdfs:label "infrastructure manager"@en .


###  http://data.europa.eu/949/legacyRadioSystem
:legacyRadioSystem rdf:type owl:ObjectProperty ;
                   rdfs:domain [ rdf:type owl:Class ;
                                 owl:unionOf ( :Track
                                               :VehicleType
                                             )
                               ] ;
                   rdfs:range <http://www.w3.org/2004/02/skos/core#Concept> ;
                   :eratvIndex "4.13.2.3" ;
                   :isCoreParameter "true"^^xsd:boolean ;
                   :rinfIndex "1.1.1.3.6.1" ;
                   <http://purl.org/dc/terms/created> "2020-08-31"^^xsd:date ;
                   <http://purl.org/dc/terms/modified> "2021-09-12"^^xsd:date ;
                   rdfs:comment "Indication of radio legacy systems installed. The allowed values for this property belong to the SKOS Concept Scheme http://data.europa.eu/949/concepts/legacy-radio-systems/LegacyRadioSystems"@en ;
                   rdfs:isDefinedBy <http://data.europa.eu/949/> ;
                   rdfs:label "Other radio systems installed (Radio Legacy Systems)"@en ;
                   <http://www.w3.org/2003/06/sw-vocab-status/ns#term_status> "stable" .


###  http://data.europa.eu/949/lineCategory
:lineCategory rdf:type owl:ObjectProperty ;
              rdfs:domain :NationalRailwayLine ;
              rdfs:range <http://www.w3.org/2004/02/skos/core#Concept> ;
              :isCoreParameter "true"^^xsd:boolean ;
              :rinfIndex "1.1.1.1.2.2" ,
                         "1.2.1.0.2.2" ;
              <http://purl.org/dc/terms/created> "2021-08-02"^^xsd:date ;
              <http://purl.org/dc/terms/modified> "2021-08-11"^^xsd:date ;
              rdfs:comment "Classification of a line according to the INF TSI. The allowed values for this property belong to the SKOS Concept Scheme http://data.europa.eu/949/concepts/line-category/LineCategories"@en ;
              rdfs:isDefinedBy <http://data.europa.eu/949/> ;
              rdfs:label "Category of line"@en ;
              <http://www.w3.org/2003/06/sw-vocab-status/ns#term_status> "stable" .


###  http://data.europa.eu/949/lineNationalId
:lineNationalId rdf:type owl:ObjectProperty ,
                         owl:FunctionalProperty ;
                rdfs:domain [ rdf:type owl:Class ;
                              owl:unionOf ( :LineReference
                                            :SectionOfLine
                                          )
                            ] ;
                rdfs:range :NationalRailwayLine ;
                :isCoreParameter "true"^^xsd:boolean ;
                :rinfIndex "1.1.0.0.0.2" ;
                <http://purl.org/dc/terms/created> "2020-09-30"^^xsd:date ;
                <http://purl.org/dc/terms/modified> "2021-08-11"^^xsd:date ;
                rdfs:comment "Related national railway line."@en ;
                rdfs:isDefinedBy <http://data.europa.eu/949/> ;
                rdfs:label "National line identification"@en ;
                <http://www.w3.org/2003/06/sw-vocab-status/ns#term_status> "stable" .


###  http://data.europa.eu/949/lineReference
:lineReference rdf:type owl:ObjectProperty ;
               rdfs:domain :OperationalPoint ;
               rdfs:range :LineReference ;
               :isCoreParameter "true"^^xsd:boolean ;
               :rinfIndex "1.2.0.0.0.6" ;
               <http://purl.org/dc/terms/created> "2021-01-29"^^xsd:date ;
               <http://purl.org/dc/terms/modified> "2021-08-11"^^xsd:date ;
               rdfs:comment "Indicates a relationship with a national railway line at a specific kilometer point."@en ;
               rdfs:isDefinedBy <http://data.europa.eu/949/> ;
               rdfs:label "Railway location of Operational point"@en ;
               <http://www.w3.org/2003/06/sw-vocab-status/ns#term_status> "stable" .


###  http://data.europa.eu/949/loadCapability
:loadCapability rdf:type owl:ObjectProperty ;
                rdfs:domain :Track ;
                rdfs:range <http://www.w3.org/2004/02/skos/core#Concept> ;
                :isCoreParameter "true"^^xsd:boolean ;
                :rinfIndex "1.1.1.1.2.4" ;
                <http://purl.org/dc/terms/created> "2020-08-24"^^xsd:date ;
                <http://purl.org/dc/terms/modified> "2021-09-10"^^xsd:date ;
                rdfs:comment "A combination of the line category and speed at the weakest point of the track. The allowed values for this property belong to the SKOS Concept Scheme http://data.europa.eu/949/concepts/load-capabilities/LoadCapabilities"@en ;
                rdfs:isDefinedBy <http://data.europa.eu/949/> ;
                rdfs:label "Load Capability"@en ;
                <http://www.w3.org/2003/06/sw-vocab-status/ns#term_status> "stable" .


###  http://data.europa.eu/949/magneticBraking
:magneticBraking rdf:type owl:ObjectProperty ,
                          owl:FunctionalProperty ;
                 rdfs:domain :Track ;
                 rdfs:range <http://www.w3.org/2004/02/skos/core#Concept> ;
                 :isCoreParameter "true"^^xsd:boolean ;
                 :rinfIndex "1.1.1.1.6.3" ;
                 <http://purl.org/dc/terms/created> "2020-08-24"^^xsd:date ;
                 <http://purl.org/dc/terms/modified> "2022-09-12"^^xsd:date ;
                 rdfs:comment """Use of magnetic brakes. The allowed values for this property belong to the SKOS Concept Scheme http://data.europa.eu/949/concepts/magnetic-braking/MagneticBraking.
This property has been modified to be a RINF parameter (its eratvIndex is deleted). It is treated as a SKOS by RINF and as a boolean by ERATV. A new ERATV datatype property has been defined, magneticBrakingFitted with boolean values."""@en ;
                 rdfs:isDefinedBy <http://data.europa.eu/949/> ;
                 rdfs:label "Use of magnetic brakes"@en ;
                 <http://www.w3.org/2003/06/sw-vocab-status/ns#term_status> "stable" .


###  http://data.europa.eu/949/manufacturer
:manufacturer rdf:type owl:ObjectProperty ;
              rdfs:domain :VehicleType ;
              rdfs:range :Manufacturer ;
              <http://purl.org/dc/terms/created> "2020-07-29"^^xsd:date ;
              <http://purl.org/dc/terms/modified> "2020-11-19"^^xsd:date ;
              rdfs:comment "Vehicle manufacturer company."@en ;
              rdfs:isDefinedBy <http://data.europa.eu/949/> ;
              rdfs:label "manufacturer"@en ;
              <http://www.w3.org/2003/06/sw-vocab-status/ns#term_status> "stable" .


###  http://data.europa.eu/949/manufacturingCountry
:manufacturingCountry rdf:type owl:ObjectProperty ;
                      rdfs:domain [ rdf:type owl:Class ;
                                    owl:unionOf ( :Vehicle
                                                  :VehicleType
                                                )
                                  ] ;
                      rdfs:range <http://www.w3.org/2004/02/skos/core#Concept> ;
                      <http://purl.org/dc/terms/created> "2020-09-30"^^xsd:date ;
                      <http://purl.org/dc/terms/modified> "2020-11-22"^^xsd:date ;
                      rdfs:comment "Indicates the country in which a vehicle or vehicle type is manufactured. The allowed values for this property belong to the SKOS Concept Scheme http://publications.europa.eu/resource/authority/country"@en ;
                      rdfs:isDefinedBy <http://data.europa.eu/949/> ;
                      rdfs:label "manufacturing country"@en ;
                      <http://www.w3.org/2003/06/sw-vocab-status/ns#term_status> "stable" .


###  http://data.europa.eu/949/maxSandingOutput
:maxSandingOutput rdf:type owl:ObjectProperty ;
                  rdfs:domain :TrainDetectionSystem ;
                  rdfs:range <http://www.w3.org/2004/02/skos/core#Concept> ;
                  :rinfIndex "1.1.1.3.7.17" ;
                  <http://purl.org/dc/terms/created> "2021-08-08"^^xsd:date ;
                  <http://purl.org/dc/terms/modified> "2021-08-08"^^xsd:date ;
                  rdfs:comment "Maximum amount of sand accepted on the track within value of sanding output for 30s, given in grams. The allowed values for this property belong to the SKOS Concept Scheme http://data.europa.eu/949/concepts/max-amount-sandings/MaxAmountSandings"@en ;
                  rdfs:isDefinedBy <http://data.europa.eu/949/> ;
                  rdfs:label "Maximum amount of sand"@en ;
                  <http://www.w3.org/2003/06/sw-vocab-status/ns#term_status> "stable" .


###  http://data.europa.eu/949/minAxleLoadVehicleCategory
:minAxleLoadVehicleCategory rdf:type owl:ObjectProperty ;
                            rdfs:domain :TrainDetectionSystem ;
                            rdfs:range <http://www.w3.org/2004/02/skos/core#Concept> ;
                            :rinfIndex "1.1.1.3.7.11.1" ;
                            <http://purl.org/dc/terms/created> "2021-08-08"^^xsd:date ;
                            <http://purl.org/dc/terms/modified> "2021-08-08"^^xsd:date ;
                            rdfs:comment "Minimum permitted axle load per category of Vehicle, given in tons depending of the category of vehicle. The allowed values for this property belong to the SKOS Concept Scheme http://data.europa.eu/949/concepts/min-axle-loads-per-vehicle-category/MinAxleLoadsPerVehicleCategory"@en ;
                            rdfs:isDefinedBy <http://data.europa.eu/949/> ;
                            rdfs:label "Minimum axle load by vehicle category"@en ;
                            <http://www.w3.org/2003/06/sw-vocab-status/ns#term_status> "stable" .


###  http://data.europa.eu/949/navigability
:navigability rdf:type owl:ObjectProperty ;
              rdfs:domain :NetRelation ;
              rdfs:range <http://www.w3.org/2004/02/skos/core#Concept> ;
              <http://purl.org/dc/terms/created> "2021-04-01"^^xsd:date ;
              <http://purl.org/dc/terms/modified> "2021-08-03"^^xsd:date ;
              rdfs:comment "Indicates the navigation possibilities between two related topological objects. The allowed values for this property belong to the SKOS Concept Scheme http://data.europa.eu/949/concepts/navigabilities/Navigabilities."@en ;
              rdfs:isDefinedBy <http://data.europa.eu/949/> ;
              rdfs:label "navigability"@en ;
              <http://www.w3.org/2003/06/sw-vocab-status/ns#term_status> "stable" .


###  http://data.europa.eu/949/netElement
:netElement rdf:type owl:ObjectProperty ;
            rdfs:range :NetElement ;
            <http://purl.org/dc/terms/created> "2021-04-01"^^xsd:date ;
            <http://purl.org/dc/terms/modified> "2022-09-06"^^xsd:date ;
            rdfs:comment """References an associated topological object.
The reason for deprecating this property is that it is defined as \"References an associated topological object.\" and the vocabulary has already a property \"hasAbstraction\" which relates the implementation layer with the topological layer."""@en ;
            rdfs:isDefinedBy <http://data.europa.eu/949/> ;
            rdfs:label "net element"@en ;
            owl:deprecated "true"^^xsd:boolean ;
            <http://www.w3.org/2003/06/sw-vocab-status/ns#term_status> "stable" .


###  http://data.europa.eu/949/netElementReference
:netElementReference rdf:type owl:ObjectProperty ;
                     rdfs:domain :SpotLocation ;
                     rdfs:range :NetElement ;
                     <http://purl.org/dc/terms/source> "https://wiki3.railml.org/wiki/RTM:spotLocation"^^xsd:anyURI ;
                     rdfs:isDefinedBy <http://data.europa.eu/949/> ;
                     rdfs:label "net element reference"@en ;
                     <http://www.w3.org/2004/02/skos/core#definition> "Reference to a railway topology net element."@en .


###  http://data.europa.eu/949/notApplicable
:notApplicable rdf:type owl:ObjectProperty ;
               <http://purl.org/dc/terms/created> "2021-09-13"^^xsd:date ;
               <http://purl.org/dc/terms/modified> "2021-09-13"^^xsd:date ;
               rdfs:comment "Reference to a property that is not applicable."@en ;
               rdfs:isDefinedBy <http://data.europa.eu/949/> ;
               rdfs:label "not applicable"@en ;
               <http://www.w3.org/2003/06/sw-vocab-status/ns#term_status> "unstable" .


###  http://data.europa.eu/949/notYetAvailable
:notYetAvailable rdf:type owl:ObjectProperty ;
                 <http://purl.org/dc/terms/created> "2021-09-13"^^xsd:date ;
                 <http://purl.org/dc/terms/modified> "2021-09-13"^^xsd:date ;
                 rdfs:comment "Reference to a property that is not yet available."@en ;
                 rdfs:isDefinedBy <http://data.europa.eu/949/> ;
                 rdfs:label "not yet available"@en ;
                 <http://www.w3.org/2003/06/sw-vocab-status/ns#term_status> "unstable" .


###  http://data.europa.eu/949/opEnd
:opEnd rdf:type owl:ObjectProperty ;
       rdfs:domain :SectionOfLine ;
       rdfs:range :OperationalPoint ;
       :isCoreParameter "true"^^xsd:boolean ;
       :rinfIndex "1.1.0.0.0.4" ;
       <http://purl.org/dc/terms/created> "2021-09-09"^^xsd:date ;
       <http://purl.org/dc/terms/modified> "2021-09-09"^^xsd:date ;
       rdfs:comment "Operational Point at the end of a Section of Line."@en ;
       rdfs:isDefinedBy <http://data.europa.eu/949/> ;
       rdfs:label "Operational Point at end of Section of Line"@en ;
       <http://www.w3.org/2003/06/sw-vocab-status/ns#term_status> "stable" .


###  http://data.europa.eu/949/opStart
:opStart rdf:type owl:ObjectProperty ;
         rdfs:domain :SectionOfLine ;
         rdfs:range :OperationalPoint ;
         :isCoreParameter "true"^^xsd:boolean ;
         :rinfIndex "1.1.0.0.0.3" ;
         <http://purl.org/dc/terms/created> "2021-09-09"^^xsd:date ;
         <http://purl.org/dc/terms/modified> "2021-09-09"^^xsd:date ;
         rdfs:comment "Operational Point at the start of a Section of Line."@en ;
         rdfs:isDefinedBy <http://data.europa.eu/949/> ;
         rdfs:label "Operational Point at start of Section of Line"@en ;
         <http://www.w3.org/2003/06/sw-vocab-status/ns#term_status> "stable" .


###  http://data.europa.eu/949/opType
:opType rdf:type owl:ObjectProperty ,
                 owl:FunctionalProperty ;
        rdfs:domain :OperationalPoint ;
        rdfs:range <http://www.w3.org/2004/02/skos/core#Concept> ;
        :isCoreParameter "true"^^xsd:boolean ;
        :rinfIndex "1.2.0.0.0.4" ;
        <http://purl.org/dc/terms/created> "2020-07-29"^^xsd:date ;
        <http://purl.org/dc/terms/modified> "2021-08-03"^^xsd:date ;
        rdfs:comment "Indicates the type on an operational point. The allowed values for this property belong to the SKOS Concept Scheme http://data.europa.eu/949/concepts/op-types/OperationalPointTypes."@en ;
        rdfs:isDefinedBy <http://data.europa.eu/949/> ;
        rdfs:label "Type of operational point"@en ;
        <http://www.w3.org/2003/06/sw-vocab-status/ns#term_status> "stable" .


###  http://data.europa.eu/949/operationalRestriction
:operationalRestriction rdf:type owl:ObjectProperty ;
                        rdfs:domain :Vehicle ;
                        rdfs:range <http://www.w3.org/2004/02/skos/core#Concept> ;
                        <http://purl.org/dc/terms/created> "2020-11-23"^^xsd:date ;
                        <http://purl.org/dc/terms/modified> "2021-08-03"^^xsd:date ;
                        rdfs:comment "Indicates an operational restriction of vehicle or wagon. Parking brake type (if the vehicle is fitted with it). The allowed values for this property belong to the SKOS Concept Scheme http://data.europa.eu/949/concepts/restrictions/Restrictions."@en ;
                        rdfs:isDefinedBy <http://data.europa.eu/949/> ;
                        rdfs:label "operational restriction"@en ;
                        <http://www.w3.org/2003/06/sw-vocab-status/ns#term_status> "stable" .


###  http://data.europa.eu/949/osmClass
:osmClass rdf:type owl:ObjectProperty ;
          rdfs:domain :Track ;
          rdfs:range <http://www.w3.org/2004/02/skos/core#Concept> ;
          rdfs:isDefinedBy <http://data.europa.eu/949/> ;
          <http://www.w3.org/2004/02/skos/core#definition> "Additional concept class according to OpenStreetMap. The allowed values for this property belong to the SKOS Concept Scheme http://data.europa.eu/949/concepts/osmclass/OSMClasses."@en .


###  http://data.europa.eu/949/otherPantographHead
:otherPantographHead rdf:type owl:ObjectProperty ;
                     rdfs:domain :Track ;
                     rdfs:range <http://www.w3.org/2004/02/skos/core#Concept> ;
                     :rinfIndex "1.1.1.2.3.2" ;
                     <http://purl.org/dc/terms/created> "2022-06-03"^^xsd:date ;
                     <http://purl.org/dc/terms/modified> "2022-06-03"^^xsd:date ;
                     rdfs:comment """Indication of which non-TSI compliant pantograph heads are allowed to be used.
The allowed values for this property belong to the SKOS Concept Scheme http://data.europa.eu/949/concepts/other-pantograph-heads/OtherPantographHeads."""@en ;
                     rdfs:isDefinedBy <http://data.europa.eu/949/> ;
                     rdfs:label "Accepted other pantograph heads"@en ;
                     <http://www.w3.org/2003/06/sw-vocab-status/ns#term_status> "stable" .


###  http://data.europa.eu/949/otherTrainProtection
:otherTrainProtection rdf:type owl:ObjectProperty ,
                               owl:FunctionalProperty ;
                      rdfs:domain :Track ;
                      rdfs:range <http://www.w3.org/2004/02/skos/core#Concept> ;
                      :rinfIndex "1.1.1.3.10.2" ;
                      <http://purl.org/dc/terms/created> "2021-08-09"^^xsd:date ;
                      <http://purl.org/dc/terms/modified> "2021-09-12"^^xsd:date ;
                      rdfs:comment "Other train protection, control and warning systems for degraded situation. The allowed values for this property belong to the SKOS Concept Scheme http://data.europa.eu/949/concepts/other-protection-control-warning/OtherProtectionControlWarnings"@en ;
                      rdfs:isDefinedBy <http://data.europa.eu/949/> ;
                      rdfs:label "Other train protection, control and warning systems for degraded situation"@en ;
                      <http://www.w3.org/2003/06/sw-vocab-status/ns#term_status> "stable" .


###  http://data.europa.eu/949/parkingBrakeType
:parkingBrakeType rdf:type owl:ObjectProperty ;
                  rdfs:domain :VehicleType ;
                  rdfs:range <http://www.w3.org/2004/02/skos/core#Concept> ;
                  :eratvIndex "4.7.3.2" ;
                  <http://purl.org/dc/terms/created> "2021-08-26"^^xsd:date ;
                  <http://purl.org/dc/terms/modified> "2021-08-26"^^xsd:date ;
                  rdfs:comment "Parking brake type (if the vehicle is fitted with it). The allowed values for this property belong to the SKOS Concept Scheme http://data.europa.eu/949/concepts/brake-parking-type/BrakeParkingType."@en ;
                  rdfs:isDefinedBy <http://data.europa.eu/949/> ;
                  rdfs:label "parking brake type"@en ;
                  <http://www.w3.org/2003/06/sw-vocab-status/ns#term_status> "stable" .


###  http://data.europa.eu/949/partOf
:partOf rdf:type owl:ObjectProperty ;
        rdfs:domain :LinearLocation ;
        rdfs:range :NetElement ;
        <http://purl.org/dc/terms/created> "2022-07-11"^^xsd:date ;
        rdfs:comment "Linear locations are subsections (part of) of other net elements"@en ;
        rdfs:isDefinedBy <http://data.europa.eu/949/> ;
        rdfs:label "part of"@en .


###  http://data.europa.eu/949/passesThroughTunnel
:passesThroughTunnel rdf:type owl:ObjectProperty ;
                     rdfs:domain [ rdf:type owl:Class ;
                                   owl:unionOf ( :NetElement
                                                 :Track
                                               )
                                 ] ;
                     rdfs:range :Tunnel ;
                     <http://purl.org/dc/terms/created> "2020-07-29"^^xsd:date ;
                     <http://purl.org/dc/terms/modified> "2021-08-09"^^xsd:date ;
                     rdfs:comment "References a tunnel that a track goes through."@en ;
                     rdfs:isDefinedBy <http://data.europa.eu/949/> ;
                     rdfs:label "passes through tunnel"@en ;
                     <http://www.w3.org/2003/06/sw-vocab-status/ns#term_status> "stable" .


###  http://data.europa.eu/949/platform
:platform rdf:type owl:ObjectProperty ;
          rdfs:domain :Track ;
          rdfs:range :Platform ;
          <http://purl.org/dc/terms/created> "2021-08-09"^^xsd:date ;
          <http://purl.org/dc/terms/modified> "2021-08-09"^^xsd:date ;
          rdfs:comment "Reference to a related platform."@en ;
          rdfs:isDefinedBy <http://data.europa.eu/949/> ;
          rdfs:label "platform"@en ;
          <http://www.w3.org/2003/06/sw-vocab-status/ns#term_status> "stable" .


###  http://data.europa.eu/949/platformHeight
:platformHeight rdf:type owl:ObjectProperty ,
                         owl:FunctionalProperty ;
                rdfs:domain :Platform ;
                rdfs:range <http://www.w3.org/2004/02/skos/core#Concept> ;
                :isCoreParameter "true"^^xsd:boolean ;
                :rinfIndex "1.2.1.0.6.5" ;
                <http://purl.org/dc/terms/created> "2021-08-02"^^xsd:date ;
                <http://purl.org/dc/terms/modified> "2021-08-02"^^xsd:date ;
                rdfs:comment "Distance between the upper surface of platform and running surface of the neighbouring track. It is the nominal value expressed in millimetres. The allowed values for this property belong to the SKOS Concept Scheme http://data.europa.eu/949/concepts/platform-heights/PlatformHeights"@en ;
                rdfs:isDefinedBy <http://data.europa.eu/949/> ;
                rdfs:label "Height of platform"@en ;
                <http://www.w3.org/2003/06/sw-vocab-status/ns#term_status> "stable" .


###  http://data.europa.eu/949/positionOnA
:positionOnA rdf:type owl:ObjectProperty ;
             rdfs:domain :NetRelation ;
             rdfs:range <http://www.w3.org/2004/02/skos/core#Concept> ;
             <http://purl.org/dc/terms/created> "2021-04-03"^^xsd:date ;
             <http://purl.org/dc/terms/modified> "2021-08-03"^^xsd:date ;
             rdfs:comment "Determines the position of the topological object A in a relation. The allowed values for this property belong to the SKOS Concept Scheme http://data.europa.eu/949/concepts/relation-positions/RelationPositions."@en ;
             rdfs:isDefinedBy <http://data.europa.eu/949/> ;
             rdfs:label "position on A"@en ;
             <http://www.w3.org/2003/06/sw-vocab-status/ns#term_status> "stable" .


###  http://data.europa.eu/949/positionOnB
:positionOnB rdf:type owl:ObjectProperty ;
             rdfs:domain :NetRelation ;
             rdfs:range <http://www.w3.org/2004/02/skos/core#Concept> ;
             <http://purl.org/dc/terms/created> "2021-04-03"^^xsd:date ;
             <http://purl.org/dc/terms/modified> "2021-08-03"^^xsd:date ;
             rdfs:comment "Determines the position of the topological object B in a relation. The allowed values for this property belong to the SKOS Concept Scheme http://data.europa.eu/949/concepts/relation-positions/RelationPositions."@en ;
             rdfs:isDefinedBy <http://data.europa.eu/949/> ;
             rdfs:label "position on B"@en ;
             <http://www.w3.org/2003/06/sw-vocab-status/ns#term_status> "stable" .


###  http://data.europa.eu/949/previousVehicleType
:previousVehicleType rdf:type owl:ObjectProperty ,
                              owl:FunctionalProperty ;
                     rdfs:domain :VehicleType ;
                     rdfs:range :VehicleType ;
                     <http://purl.org/dc/terms/created> "2022-06-15"^^xsd:date ;
                     <http://purl.org/dc/terms/modified> "2022-06-15"^^xsd:date ;
                     rdfs:comment "Denotes a the previous VehicleType."@en ;
                     rdfs:isDefinedBy <http://data.europa.eu/949/> ;
                     rdfs:label "previous vehicle type"@en ;
                     <http://www.w3.org/2003/06/sw-vocab-status/ns#term_status> "stable"@en .


###  http://data.europa.eu/949/profileNumberSemiTrailers
:profileNumberSemiTrailers rdf:type owl:ObjectProperty ;
                           rdfs:domain :Track ;
                           rdfs:range <http://www.w3.org/2004/02/skos/core#Concept> ;
                           :isCoreParameter "true"^^xsd:boolean ;
                           :rinfIndex "1.1.1.1.3.5" ;
                           <http://purl.org/dc/terms/created> "2021-08-03"^^xsd:date ;
                           <http://purl.org/dc/terms/modified> "2021-09-10"^^xsd:date ;
                           rdfs:comment "Coding for combined transport for semi-trailers as defined in UIC Code. The allowed values for this property belong to the SKOS Concept Scheme http://data.europa.eu/949/concepts/profile-num-semi-trailers/ProfileNumbersSemiTrailers"@en ;
                           rdfs:isDefinedBy <http://data.europa.eu/949/> ;
                           rdfs:label "Standard combined transport profile number for semi-trailers"@en ;
                           <http://www.w3.org/2003/06/sw-vocab-status/ns#term_status> "stable" .


###  http://data.europa.eu/949/profileNumberSwapBodies
:profileNumberSwapBodies rdf:type owl:ObjectProperty ;
                         rdfs:domain :Track ;
                         rdfs:range <http://www.w3.org/2004/02/skos/core#Concept> ;
                         :isCoreParameter "true"^^xsd:boolean ;
                         :rinfIndex "1.1.1.1.3.4" ;
                         <http://purl.org/dc/terms/created> "2021-08-03"^^xsd:date ;
                         <http://purl.org/dc/terms/modified> "2021-09-10"^^xsd:date ;
                         rdfs:comment "Coding for combined transport with swap bodies as defined in UIC Code. The allowed values for this property belong to the SKOS Concept Scheme http://data.europa.eu/949/concepts/profile-num-swap-bodies/ProfileNumbersSwapBodies"@en ;
                         rdfs:isDefinedBy <http://data.europa.eu/949/> ;
                         rdfs:label "Standard combined transport profile number for swap bodies"@en ;
                         <http://www.w3.org/2003/06/sw-vocab-status/ns#term_status> "stable" .


###  http://data.europa.eu/949/protectionLegacySystem
:protectionLegacySystem rdf:type owl:ObjectProperty ;
                        rdfs:domain [ rdf:type owl:Class ;
                                      owl:unionOf ( :Track
                                                    :VehicleType
                                                  )
                                    ] ;
                        rdfs:range <http://www.w3.org/2004/02/skos/core#Concept> ;
                        :eratvIndex "4.13.1.5" ;
                        :isCoreParameter "true"^^xsd:boolean ;
                        :rinfIndex "1.1.1.3.5.3" ;
                        <http://purl.org/dc/terms/created> "2020-08-31"^^xsd:date ;
                        <http://purl.org/dc/terms/modified> "2021-09-12"^^xsd:date ;
                        rdfs:comment "Indication of which class B system is installed. The allowed values for this property belong to the SKOS Concept Scheme http://data.europa.eu/949/concepts/train-protection-legacy-systems/TrainProtectionLegacySystems"@en ;
                        rdfs:isDefinedBy <http://data.europa.eu/949/> ;
                        rdfs:label "Train protection legacy system"@en ;
                        <http://www.w3.org/2003/06/sw-vocab-status/ns#term_status> "stable" .


###  http://data.europa.eu/949/quieterRoutesExemptedCountry
:quieterRoutesExemptedCountry rdf:type owl:ObjectProperty ;
                              rdfs:domain :Vehicle ;
                              rdfs:range <http://www.w3.org/2004/02/skos/core#Concept> ;
                              <http://purl.org/dc/terms/created> "2020-11-23"^^xsd:date ;
                              <http://purl.org/dc/terms/modified> "2020-11-23"^^xsd:date ;
                              rdfs:comment "Country where a vehicle may operate without noise restrictions. The allowed values for this property belong to the SKOS Concept Scheme http://publications.europa.eu/resource/authority/country"@en ;
                              rdfs:isDefinedBy <http://data.europa.eu/949/> ;
                              rdfs:label "quieter route exempted country"@en ;
                              <http://www.w3.org/2003/06/sw-vocab-status/ns#term_status> "stable" .


###  http://data.europa.eu/949/railInclination
:railInclination rdf:type owl:ObjectProperty ,
                          owl:FunctionalProperty ;
                 rdfs:domain [ rdf:type owl:Class ;
                               owl:unionOf ( :Track
                                             :VehicleType
                                           )
                             ] ;
                 rdfs:range <http://www.w3.org/2004/02/skos/core#Concept> ;
                 :eratvIndex "4.6.5" ;
                 :isCoreParameter "true"^^xsd:boolean ;
                 :rinfIndex "1.1.1.1.4.3" ;
                 <http://purl.org/dc/terms/created> "2020-08-24"^^xsd:date ;
                 <http://purl.org/dc/terms/modified> "2022-10-20"^^xsd:date ;
                 rdfs:comment """An angle defining the inclination of the head of a rail relative to the running surface. The allowed values for this property belong to the SKOS Concept Scheme http://data.europa.eu/949/concepts/rail-inclinations/RailInclinations
This property has been changed, its rinfIndex was deleted. RINF treats this parameter as an integer. A new datatype property for RINF has been defined called railInclinationMeasurement.
This change was rolled back, RINF index was again added."""@en ;
                 rdfs:isDefinedBy <http://data.europa.eu/949/> ;
                 rdfs:label "Rail inclination"@en ;
                 <http://www.w3.org/2003/06/sw-vocab-status/ns#term_status> "stable" .


###  http://data.europa.eu/949/rollingStockFireCategory
:rollingStockFireCategory rdf:type owl:ObjectProperty ,
                                   owl:FunctionalProperty ;
                          rdfs:domain :Tunnel ;
                          rdfs:range <http://www.w3.org/2004/02/skos/core#Concept> ;
                          :isCoreParameter "true"^^xsd:boolean ;
                          :rinfIndex "1.1.1.1.8.10" ,
                                     "1.2.1.0.5.7" ,
                                     "1.2.2.0.5.7" ;
                          <http://purl.org/dc/terms/created> "2020-07-29"^^xsd:date ;
                          <http://purl.org/dc/terms/modified> "2021-08-10"^^xsd:date ;
                          rdfs:comment "Applicable rolling stock fire category for a tunnel. The allowed values for this property belong to the SKOS Concept Scheme http://data.europa.eu/949/concepts/rolling-stock-fire/Categories."@en ;
                          rdfs:isDefinedBy <http://data.europa.eu/949/> ;
                          rdfs:label "Fire category of rolling stock required"@en ;
                          <http://www.w3.org/2003/06/sw-vocab-status/ns#term_status> "stable" .


###  http://data.europa.eu/949/siding
:siding rdf:type owl:ObjectProperty ;
        rdfs:domain :OperationalPoint ;
        rdfs:range :Siding ;
        <http://purl.org/dc/terms/created> "2021-08-10"^^xsd:date ;
        <http://purl.org/dc/terms/modified> "2021-08-10"^^xsd:date ;
        rdfs:comment "Reference to a related siding."@en ;
        rdfs:isDefinedBy <http://data.europa.eu/949/> ;
        rdfs:label "siding"@en ;
        <http://www.w3.org/2003/06/sw-vocab-status/ns#term_status> "stable" .


###  http://data.europa.eu/949/snowIceHailConditions
:snowIceHailConditions rdf:type owl:ObjectProperty ,
                                owl:FunctionalProperty ;
                       rdfs:domain :VehicleType ;
                       rdfs:range <http://www.w3.org/2004/02/skos/core#Concept> ;
                       :eratvIndex "4.3.3" ;
                       <http://purl.org/dc/terms/created> "2020-08-24"^^xsd:date ;
                       <http://purl.org/dc/terms/modified> "2021-08-02"^^xsd:date ;
                       rdfs:comment "Snow, ice and hail conditions. The allowed values for this property belong to the SKOS Concept Scheme http://data.europa.eu/949/concepts/ice-conditions/IceConditions"@en ;
                       rdfs:isDefinedBy <http://data.europa.eu/949/> ;
                       rdfs:label "snow ice hail conditions"@en ;
                       <http://www.w3.org/2003/06/sw-vocab-status/ns#term_status> "stable" .


###  http://data.europa.eu/949/solNature
:solNature rdf:type owl:ObjectProperty ,
                    owl:FunctionalProperty ;
           rdfs:domain :SectionOfLine ;
           rdfs:range <http://www.w3.org/2004/02/skos/core#Concept> ;
           :isCoreParameter "true"^^xsd:boolean ;
           :rinfIndex "1.1.0.0.0.6" ;
           <http://purl.org/dc/terms/created> "2021-08-08"^^xsd:date ;
           <http://purl.org/dc/terms/modified> "2021-08-08"^^xsd:date ;
           rdfs:comment "Indicates the nature of a section of line. The allowed values for this property belong to the SKOS Concept Scheme http://data.europa.eu/949/concepts/sol-natures/SoLNatures"@en ;
           rdfs:isDefinedBy <http://data.europa.eu/949/> ;
           rdfs:label "Nature of Section of Line"@en ;
           <http://www.w3.org/2003/06/sw-vocab-status/ns#term_status> "stable" .


###  http://data.europa.eu/949/startLocation
:startLocation rdf:type owl:ObjectProperty ;
               rdfs:subPropertyOf <http://www.opengis.net/ont/geosparql#hasGeometry> ,
                                  <http://www.w3.org/2003/01/geo/wgs84_pos#location> ;
               rdfs:domain :Tunnel ;
               rdfs:range [ rdf:type owl:Class ;
                            owl:unionOf ( <http://www.opengis.net/ont/geosparql#Geometry>
                                          <http://www.w3.org/2003/01/geo/wgs84_pos#Point>
                                        )
                          ] ;
               :isCoreParameter "true"^^xsd:boolean ;
               :rinfIndex "1.1.1.1.8.3" ;
               <http://purl.org/dc/terms/created> "2020-07-29"^^xsd:date ;
               <http://purl.org/dc/terms/modified> "2021-08-11"^^xsd:date ;
               rdfs:comment "References the geolocation of the start of a tunnel."@en ;
               rdfs:isDefinedBy <http://data.europa.eu/949/> ;
               rdfs:label "Start of tunnel"@en ;
               <http://www.w3.org/2003/06/sw-vocab-status/ns#term_status> "stable" .


###  http://data.europa.eu/949/state
:state rdf:type owl:ObjectProperty ,
                owl:FunctionalProperty ;
       rdfs:domain :Certificate ;
       rdfs:range <http://www.w3.org/2004/02/skos/core#Concept> ;
       <http://purl.org/dc/terms/created> "2022-06-15"^^xsd:date ;
       <http://purl.org/dc/terms/modified> "2022-06-15"^^xsd:date ;
       rdfs:comment "Denoting the state of the certificate and range the following instances. The allowed values for this property belong to the SKOS Concept Scheme http://data.europa.eu/949/concepts/states/States. This concept scheme is temporarily non-dereferenceable."@en ;
       rdfs:label "state"@en ;
       <http://www.w3.org/2003/06/sw-vocab-status/ns#term_status> "stable"@en .


###  http://data.europa.eu/949/subCategory
:subCategory rdf:type owl:ObjectProperty ,
                      owl:FunctionalProperty ;
             rdfs:domain :VehicleType ;
             rdfs:range <http://www.w3.org/2004/02/skos/core#Concept> ;
             :eratvIndex 1.5 ;
             <http://purl.org/dc/terms/created> "2020-07-29"^^xsd:date ;
             <http://purl.org/dc/terms/modified> "2021-08-03"^^xsd:date ;
             rdfs:comment "Vehicle subcategory. The allowed values for this property belong to the SKOS Concept Scheme http://data.europa.eu/949/concepts/vehicle-types/Categories."@en ;
             rdfs:isDefinedBy <http://data.europa.eu/949/> ;
             rdfs:label "vehicle subcategory"@en ;
             <http://www.w3.org/2003/06/sw-vocab-status/ns#term_status> "stable" .


###  http://data.europa.eu/949/supportedPlatformHeight
:supportedPlatformHeight rdf:type owl:ObjectProperty ;
                         rdfs:domain :VehicleType ;
                         rdfs:range <http://www.w3.org/2004/02/skos/core#Concept> ;
                         :eratvIndex "4.12.3.1" ;
                         <http://purl.org/dc/terms/created> "2020-07-29"^^xsd:date ;
                         <http://purl.org/dc/terms/modified> "2021-08-02"^^xsd:date ;
                         rdfs:comment "Platform height for which the vehicle is deÂ­signed. The allowed values for this property belong to the SKOS Concept Scheme http://data.europa.eu/949/concepts/platform-heights/PlatformHeights"@en ;
                         rdfs:isDefinedBy <http://data.europa.eu/949/> ;
                         rdfs:label "supported platform height"@en ;
                         <http://www.w3.org/2003/06/sw-vocab-status/ns#term_status> "stable" .


###  http://data.europa.eu/949/tenClassification
:tenClassification rdf:type owl:ObjectProperty ;
                   rdfs:domain [ rdf:type owl:Class ;
                                 owl:unionOf ( :Platform
                                               :Track
                                             )
                               ] ;
                   rdfs:range <http://www.w3.org/2004/02/skos/core#Concept> ;
                   :isCoreParameter "true"^^xsd:boolean ;
                   :rinfIndex "1.1.1.1.2.1" ,
                              "1.2.1.0.2.1" ,
                              "1.2.1.0.6.3" ,
                              "1.2.2.0.0.3" ;
                   <http://purl.org/dc/terms/created> "2021-08-02"^^xsd:date ;
                   <http://purl.org/dc/terms/modified> "2021-09-10"^^xsd:date ;
                   rdfs:comment "Indicates the related TEN (trans-European network). The allowed values for this property belong to the SKOS Concept Scheme http://data.europa.eu/949/concepts/ten-classifications/TENClassifications."@en ;
                   rdfs:isDefinedBy <http://data.europa.eu/949/> ;
                   rdfs:label "TEN classification (of track, of platform, of siding)"@en ;
                   <http://www.w3.org/2003/06/sw-vocab-status/ns#term_status> "stable" .


###  http://data.europa.eu/949/thermalCapacityTSIReference
:thermalCapacityTSIReference rdf:type owl:ObjectProperty ,
                                      owl:FunctionalProperty ;
                             rdfs:domain :VehicleType ;
                             rdfs:range <http://www.w3.org/2004/02/skos/core#Concept> ;
                             :eratvIndex "4.7.2.1.1" ;
                             <http://purl.org/dc/terms/created> "2020-08-24"^^xsd:date ;
                             <http://purl.org/dc/terms/modified> "2021-08-02"^^xsd:date ;
                             rdfs:comment "Reference case of a TSI thermal capacity. The allowed values for this property belong to the SKOS Concept Scheme http://data.europa.eu/949/concepts/thermal-capacity/ThermalCapacityTSIReferences"@en ;
                             rdfs:isDefinedBy <http://data.europa.eu/949/> ;
                             rdfs:label "thermal capacity TSI reference"@en ;
                             <http://www.w3.org/2003/06/sw-vocab-status/ns#term_status> "stable" .


###  http://data.europa.eu/949/track
:track rdf:type owl:ObjectProperty ;
       rdfs:domain [ rdf:type owl:Class ;
                     owl:unionOf ( :OperationalPoint
                                   :SectionOfLine
                                 )
                   ] ;
       rdfs:range :Track ;
       <http://purl.org/dc/terms/created> "2021-08-09"^^xsd:date ;
       <http://purl.org/dc/terms/modified> "2021-09-09"^^xsd:date ;
       rdfs:comment "Reference to a related railway track."@en ;
       rdfs:isDefinedBy <http://data.europa.eu/949/> ;
       rdfs:label "track"@en ;
       <http://www.w3.org/2003/06/sw-vocab-status/ns#term_status> "stable" .


###  http://data.europa.eu/949/trackDirection
:trackDirection rdf:type owl:ObjectProperty ,
                         owl:FunctionalProperty ;
                rdfs:domain :Track ;
                rdfs:range <http://www.w3.org/2004/02/skos/core#Concept> ;
                :isCoreParameter "true"^^xsd:boolean ;
                :rinfIndex "1.1.1.0.0.2" ;
                <http://purl.org/dc/terms/created> "2021-09-09"^^xsd:date ;
                <http://purl.org/dc/terms/modified> "2021-09-09"^^xsd:date ;
                rdfs:comment "Track normal running direction. The allowed values for this property belong to the SKOS Concept Scheme http://data.europa.eu/949/concepts/track-running-directions/TrackRunningDirections."@en ;
                rdfs:isDefinedBy <http://data.europa.eu/949/> ;
                rdfs:label "Normal running direction"@en ;
                <http://www.w3.org/2003/06/sw-vocab-status/ns#term_status> "stable" .


###  http://data.europa.eu/949/trainDetectionSystem
:trainDetectionSystem rdf:type owl:ObjectProperty ;
                      rdfs:domain :Track ;
                      rdfs:range :TrainDetectionSystem ;
                      <http://purl.org/dc/terms/created> "2020-07-29"^^xsd:date ;
                      <http://purl.org/dc/terms/modified> "2021-09-12"^^xsd:date ;
                      rdfs:comment "Train detection systems installed in the section of line."@en ;
                      rdfs:isDefinedBy <http://data.europa.eu/949/> ;
                      rdfs:label "train detection system"@en ;
                      <http://www.w3.org/2003/06/sw-vocab-status/ns#term_status> "stable" .


###  http://data.europa.eu/949/trainDetectionSystemSpecificCheck
:trainDetectionSystemSpecificCheck rdf:type owl:ObjectProperty ;
                                   rdfs:domain :TrainDetectionSystem ;
                                   rdfs:range <http://www.w3.org/2004/02/skos/core#Concept> ;
                                   :rinfIndex "1.1.1.3.7.1.2" ;
                                   <http://purl.org/dc/terms/created> "2020-08-24"^^xsd:date ;
                                   <http://purl.org/dc/terms/modified> "2021-08-08"^^xsd:date ;
                                   rdfs:comment "Type of track circuits or axle counter to which specific checks are needed. The allowed values for this property belong to the SKOS Concept Scheme http://data.europa.eu/949/concepts/train-detection-specific-checks/TrainDetectionSystemsSpecificChecks"@en ;
                                   rdfs:isDefinedBy <http://data.europa.eu/949/> ;
                                   rdfs:label "Type of track circuits to which specific checks are needed"@en ;
                                   <http://www.w3.org/2003/06/sw-vocab-status/ns#term_status> "stable" .


###  http://data.europa.eu/949/trainDetectionSystemType
:trainDetectionSystemType rdf:type owl:ObjectProperty ;
                          rdfs:domain [ rdf:type owl:Class ;
                                        owl:unionOf ( :TrainDetectionSystem
                                                      :VehicleType
                                                    )
                                      ] ;
                          rdfs:range <http://www.w3.org/2004/02/skos/core#Concept> ;
                          :eratvIndex "4.14.1" ;
                          :isCoreParameter "true"^^xsd:boolean ;
                          :rinfIndex "1.1.1.3.7.1.1" ;
                          <http://purl.org/dc/terms/created> "2021-08-07"^^xsd:date ;
                          <http://purl.org/dc/terms/modified> "2021-08-07"^^xsd:date ;
                          rdfs:comment "Indication of supported types of train detection systems. The allowed values for this property belong to the SKOS Concept Scheme http://data.europa.eu/949/concepts/train-detection/TrainDetectionSystems"@en ;
                          rdfs:isDefinedBy <http://data.europa.eu/949/> ;
                          rdfs:label "Type of train detection system"@en ;
                          <http://www.w3.org/2003/06/sw-vocab-status/ns#term_status> "stable" .


###  http://data.europa.eu/949/tsiCompliantCompositeBrakeBlocks
:tsiCompliantCompositeBrakeBlocks rdf:type owl:ObjectProperty ;
                                  rdfs:domain :TrainDetectionSystem ;
                                  rdfs:range <http://www.w3.org/2004/02/skos/core#Concept> ;
                                  :rinfIndex "1.1.1.3.7.21" ;
                                  <http://purl.org/dc/terms/created> "2021-08-08"^^xsd:date ;
                                  <http://purl.org/dc/terms/modified> "2021-08-09"^^xsd:date ;
                                  rdfs:comment "TSI compliance of rules on the use of composite brake blocks. The allowed values for this property belong to the SKOS Concept Scheme http://data.europa.eu/949/concepts/tsi-compliances/TSICompliances."@en ;
                                  rdfs:isDefinedBy <http://data.europa.eu/949/> ;
                                  rdfs:label "TSI compliance of rules on the use of composite brake blocks"@en ;
                                  <http://www.w3.org/2003/06/sw-vocab-status/ns#term_status> "stable" .


###  http://data.europa.eu/949/tsiCompliantFerromagneticWheel
:tsiCompliantFerromagneticWheel rdf:type owl:ObjectProperty ;
                                rdfs:domain :TrainDetectionSystem ;
                                rdfs:range <http://www.w3.org/2004/02/skos/core#Concept> ;
                                :rinfIndex "1.1.1.3.7.14" ;
                                <http://purl.org/dc/terms/created> "2021-08-08"^^xsd:date ;
                                <http://purl.org/dc/terms/modified> "2021-08-08"^^xsd:date ;
                                rdfs:comment """TSI compliance of Ferromagnetic characteristics of wheel material required. The allowed values for this property belong to the SKOS Concept Scheme http://data.europa.eu/949/concepts/tsi-compliances/TSICompliances.

The concept scheme is temporarily non-deferenceable."""@en ;
                                rdfs:isDefinedBy <http://data.europa.eu/949/> ;
                                rdfs:label "TSI compliance of Ferromagnetic characteristics of wheel material required"@en ;
                                <http://www.w3.org/2003/06/sw-vocab-status/ns#term_status> "stable" .


###  http://data.europa.eu/949/tsiCompliantMaxDistConsecutiveAxles
:tsiCompliantMaxDistConsecutiveAxles rdf:type owl:ObjectProperty ;
                                     rdfs:domain :TrainDetectionSystem ;
                                     rdfs:range <http://www.w3.org/2004/02/skos/core#Concept> ;
                                     :isCoreParameter "true"^^xsd:boolean ;
                                     :rinfIndex "1.1.1.3.7.2.1" ;
                                     <http://purl.org/dc/terms/created> "2021-08-07"^^xsd:date ;
                                     <http://purl.org/dc/terms/modified> "2021-08-09"^^xsd:date ;
                                     rdfs:comment "Indication whether required distance between two consecutive axles is compliant with the TSI. The allowed values for this property belong to the SKOS Concept Scheme http://data.europa.eu/949/concepts/tsi-compliances/TSICompliances."@en ;
                                     rdfs:isDefinedBy <http://data.europa.eu/949/> ;
                                     rdfs:label "TSI compliance of maximum permitted distance between two consecutive axles"@en ;
                                     <http://www.w3.org/2003/06/sw-vocab-status/ns#term_status> "stable" .


###  http://data.europa.eu/949/tsiCompliantMaxImpedanceWheelset
:tsiCompliantMaxImpedanceWheelset rdf:type owl:ObjectProperty ;
                                  rdfs:domain :TrainDetectionSystem ;
                                  rdfs:range <http://www.w3.org/2004/02/skos/core#Concept> ;
                                  :rinfIndex "1.1.1.3.7.15.1" ;
                                  <http://purl.org/dc/terms/created> "2021-08-08"^^xsd:date ;
                                  <http://purl.org/dc/terms/modified> "2021-08-09"^^xsd:date ;
                                  rdfs:comment "TSI compliance of maximum permitted impedance between opposite wheels of a wheelset. The allowed values for this property belong to the SKOS Concept Scheme http://data.europa.eu/949/concepts/tsi-compliances/TSICompliances."@en ;
                                  rdfs:isDefinedBy <http://data.europa.eu/949/> ;
                                  rdfs:label "TSI compliance of maximum permitted impedance between opposite wheels of a wheelset"@en ;
                                  <http://www.w3.org/2003/06/sw-vocab-status/ns#term_status> "stable" .


###  http://data.europa.eu/949/tsiCompliantMetalConstruction
:tsiCompliantMetalConstruction rdf:type owl:ObjectProperty ;
                               rdfs:domain :TrainDetectionSystem ;
                               rdfs:range <http://www.w3.org/2004/02/skos/core#Concept> ;
                               :rinfIndex "1.1.1.3.7.13" ;
                               <http://purl.org/dc/terms/created> "2021-08-08"^^xsd:date ;
                               <http://purl.org/dc/terms/modified> "2021-08-09"^^xsd:date ;
                               rdfs:comment "TSI compliance of rules for vehicle metal construction. The allowed values for this property belong to the SKOS Concept Scheme http://data.europa.eu/949/concepts/tsi-compliances/TSICompliances."@en ;
                               rdfs:isDefinedBy <http://data.europa.eu/949/> ;
                               rdfs:label "TSI compliance of rules for vehicle metal construction"@en ;
                               <http://www.w3.org/2003/06/sw-vocab-status/ns#term_status> "stable" .


###  http://data.europa.eu/949/tsiCompliantMetalFreeSpace
:tsiCompliantMetalFreeSpace rdf:type owl:ObjectProperty ;
                            rdfs:domain :TrainDetectionSystem ;
                            rdfs:range <http://www.w3.org/2004/02/skos/core#Concept> ;
                            :rinfIndex "1.1.1.3.7.12" ;
                            <http://purl.org/dc/terms/created> "2021-08-08"^^xsd:date ;
                            <http://purl.org/dc/terms/modified> "2021-08-09"^^xsd:date ;
                            rdfs:comment "TSI compliance of rules for metal-free space around wheels. The allowed values for this property belong to the SKOS Concept Scheme http://data.europa.eu/949/concepts/tsi-compliances/TSICompliances."@en ;
                            rdfs:isDefinedBy <http://data.europa.eu/949/> ;
                            rdfs:label "TSI compliance of rules for metal-free space around wheels"@en ;
                            <http://www.w3.org/2003/06/sw-vocab-status/ns#term_status> "stable" .


###  http://data.europa.eu/949/tsiCompliantRSTShuntImpedance
:tsiCompliantRSTShuntImpedance rdf:type owl:ObjectProperty ;
                               rdfs:domain :TrainDetectionSystem ;
                               rdfs:range <http://www.w3.org/2004/02/skos/core#Concept> ;
                               :rinfIndex "1.1.1.3.7.23" ;
                               <http://purl.org/dc/terms/created> "2021-08-08"^^xsd:date ;
                               <http://purl.org/dc/terms/modified> "2021-08-09"^^xsd:date ;
                               rdfs:comment "TSI compliance of rules on combination of RST characteristics influencing shunting impedance. The allowed values for this property belong to the SKOS Concept Scheme http://data.europa.eu/949/concepts/tsi-compliances/TSICompliances."@en ;
                               rdfs:isDefinedBy <http://data.europa.eu/949/> ;
                               rdfs:label "TSI compliance of rules on combination of RST characteristics influencing shunting impedance"@en ;
                               <http://www.w3.org/2003/06/sw-vocab-status/ns#term_status> "stable" .


###  http://data.europa.eu/949/tsiCompliantSandCharacteristics
:tsiCompliantSandCharacteristics rdf:type owl:ObjectProperty ;
                                 rdfs:domain :TrainDetectionSystem ;
                                 rdfs:range <http://www.w3.org/2004/02/skos/core#Concept> ;
                                 :rinfIndex "1.1.1.3.7.19" ;
                                 <http://purl.org/dc/terms/created> "2021-08-08"^^xsd:date ;
                                 <http://purl.org/dc/terms/modified> "2021-08-09"^^xsd:date ;
                                 rdfs:comment "TSI Compliance of rules on sand characteristics. The allowed values for this property belong to the SKOS Concept Scheme http://data.europa.eu/949/concepts/tsi-compliances/TSICompliances."@en ;
                                 rdfs:isDefinedBy <http://data.europa.eu/949/> ;
                                 rdfs:label "TSI Compliance of rules on sand characteristics"@en ;
                                 <http://www.w3.org/2003/06/sw-vocab-status/ns#term_status> "stable" .


###  http://data.europa.eu/949/tsiCompliantSanding
:tsiCompliantSanding rdf:type owl:ObjectProperty ;
                     rdfs:domain :TrainDetectionSystem ;
                     rdfs:range <http://www.w3.org/2004/02/skos/core#Concept> ;
                     :rinfIndex "1.1.1.3.7.16" ;
                     <http://purl.org/dc/terms/created> "2021-08-08"^^xsd:date ;
                     <http://purl.org/dc/terms/modified> "2021-08-09"^^xsd:date ;
                     rdfs:comment "TSI compliance of sanding rules to allow compatibility with track circuits. Too much sand brings the risk of not detecting trains in tracks equipped with track circuits. The allowed values for this property belong to the SKOS Concept Scheme http://data.europa.eu/949/concepts/tsi-compliances/TSICompliances."@en ;
                     rdfs:isDefinedBy <http://data.europa.eu/949/> ;
                     rdfs:label "TSI compliance of sanding"@en ;
                     <http://www.w3.org/2003/06/sw-vocab-status/ns#term_status> "unstable" .


###  http://data.europa.eu/949/tsiCompliantShuntDevices
:tsiCompliantShuntDevices rdf:type owl:ObjectProperty ;
                          rdfs:domain :TrainDetectionSystem ;
                          rdfs:range <http://www.w3.org/2004/02/skos/core#Concept> ;
                          :rinfIndex "1.1.1.3.7.22" ;
                          <http://purl.org/dc/terms/created> "2021-08-08"^^xsd:date ;
                          <http://purl.org/dc/terms/modified> "2021-08-09"^^xsd:date ;
                          rdfs:comment "TSI compliance of rules on shunt assisting devices. The allowed values for this property belong to the SKOS Concept Scheme http://data.europa.eu/949/concepts/tsi-compliances/TSICompliances."@en ;
                          rdfs:isDefinedBy <http://data.europa.eu/949/> ;
                          rdfs:label "TSI compliance of rules on shunt assisting devices"@en ;
                          <http://www.w3.org/2003/06/sw-vocab-status/ns#term_status> "stable" .


###  http://data.europa.eu/949/tsiPantographHead
:tsiPantographHead rdf:type owl:ObjectProperty ;
                   rdfs:domain :Track ;
                   rdfs:range <http://www.w3.org/2004/02/skos/core#Concept> ;
                   :rinfIndex "1.1.1.2.3.1" ;
                   <http://purl.org/dc/terms/created> "2020-08-25"^^xsd:date ;
                   <http://purl.org/dc/terms/modified> "2021-09-11"^^xsd:date ;
                   rdfs:comment "Indication of which TSI compliant pantograph heads are allowed to be used. The allowed values for this property belong to the SKOS Concept Scheme http://data.europa.eu/949/concepts/compliant-pantograph-heads/CompliantPantographHeads."@en ;
                   rdfs:isDefinedBy <http://data.europa.eu/949/> ;
                   rdfs:label "Accepted TSI compliant pantograph heads"@en ;
                   <http://www.w3.org/2003/06/sw-vocab-status/ns#term_status> "stable" .


###  http://data.europa.eu/949/typeVersionId
:typeVersionId rdf:type owl:ObjectProperty ;
               rdfs:domain :VehicleType ;
               rdfs:range <http://www.w3.org/2004/02/skos/core#Concept> ;
               <http://purl.org/dc/terms/created> "2022-11-03"^^xsd:date ;
               rdf:label "type version id"@en ;
               rdfs:comment """Indicates the registrationVersion with Ids 10,20 and 30 indicating registration according to Directive 2008/57/EC and implementing Decision 2011/665/EU, and 40 and 50 indicating registration according to regime described in Directive 2008/57/EC.
The allowed values for this property belong to the SKOS Concept Scheme http://data.europa.eu/949/concepts/version-ids/VehicleTypeVersionIds."""@en ;
               rdfs:isDefinedBy <http://data.europa.eu/949/> ;
               <http://www.w3.org/2003/06/sw-vocab-status/ns#term_status> "stable" .


###  http://data.europa.eu/949/validityPeriod
:validityPeriod rdf:type owl:ObjectProperty ;
                rdfs:domain :EraFeature ;
                rdfs:range :ValidityPeriod ;
                <http://purl.org/dc/terms/created> "2022-10-21"^^xsd:date ;
                rdfs:comment "Resltionship among an object of the infrastructure and its period of validity"@en ;
                rdfs:isDefinedBy "http://data.europa.eu/949/"^^xsd:anyURI ;
                rdfs:label "validity period"@en ;
                <http://www.w3.org/2003/06/sw-vocab-status/ns#term_status> "stable" .


###  http://data.europa.eu/949/vehicleKeeper
:vehicleKeeper rdf:type owl:ObjectProperty ;
               rdfs:domain :Vehicle ;
               rdfs:range :VehicleKeeper ;
               <http://purl.org/dc/terms/created> "2020-11-23"^^xsd:date ;
               <http://purl.org/dc/terms/modified> "2020-11-23"^^xsd:date ;
               rdfs:comment "Indicates the organization that owns/operated a vehicle or wagon. http://data.europa.eu/949/concepts/tsi-compliances/TSICompliances"@en ;
               rdfs:isDefinedBy <http://data.europa.eu/949/> ;
               rdfs:label "vehicle keeper"@en ;
               <http://www.w3.org/2003/06/sw-vocab-status/ns#term_status> "stable" .


###  http://data.europa.eu/949/vehicleType
:vehicleType rdf:type owl:ObjectProperty ;
             rdfs:domain :Vehicle ;
             rdfs:range :VehicleType ;
             <http://purl.org/dc/terms/created> "2020-11-22"^^xsd:date ;
             <http://purl.org/dc/terms/modified> "2020-11-22"^^xsd:date ;
             rdfs:comment "Indicates the vehicle type of a specific vehicle or wagon."@en ;
             rdfs:isDefinedBy <http://data.europa.eu/949/> ;
             rdfs:label "vehicle type"@en ;
             <http://www.w3.org/2003/06/sw-vocab-status/ns#term_status> "stable" .


###  http://data.europa.eu/949/voiceGSMRNetwork
:voiceGSMRNetwork rdf:type owl:ObjectProperty ,
                           owl:FunctionalProperty ;
                  rdfs:domain :VehicleType ;
                  rdfs:range <http://www.w3.org/2004/02/skos/core#Concept> ;
                  :eratvIndex "4.13.2.10" ;
                  <http://purl.org/dc/terms/created> "2020-08-31"^^xsd:date ;
                  <http://purl.org/dc/terms/modified> "2021-08-02"^^xsd:date ;
                  rdfs:comment "Voice SIM Card GSM-R Home Network. The allowed values for this property belong to the SKOS Concept Scheme http://data.europa.eu/949/concepts/gsmr-networks/GSMRNetworks"@en ;
                  rdfs:isDefinedBy <http://data.europa.eu/949/> ;
                  rdfs:label "voice GSM-R network"@en ;
                  <http://www.w3.org/2003/06/sw-vocab-status/ns#term_status> "stable" .


###  http://data.europa.eu/949/voiceRadioCompatible
:voiceRadioCompatible rdf:type owl:ObjectProperty ;
                      rdfs:domain [ rdf:type owl:Class ;
                                    owl:unionOf ( :Track
                                                  :VehicleType
                                                )
                                  ] ;
                      rdfs:range <http://www.w3.org/2004/02/skos/core#Concept> ;
                      :eratvIndex "4.13.2.5" ;
                      :rinfIndex "1.1.1.3.3.9" ;
                      <http://purl.org/dc/terms/created> "2020-08-31"^^xsd:date ;
                      <http://purl.org/dc/terms/modified> "2021-09-12"^^xsd:date ;
                      rdfs:comment """Radio requirements used for demonstrating technical compatibility voice.
 The allowed values for this property belong to the SKOS Concept Scheme http://data.europa.eu/949/concepts/voice-radio-system-compatibilities/VoiceRadioSystemCompatibilities. This concept scheme is temporatily non-deferenceable."""@en ;
                      rdfs:isDefinedBy <http://data.europa.eu/949/> ;
                      rdfs:label "Radio system compatibility voice"@en ;
                      <http://www.w3.org/2003/06/sw-vocab-status/ns#term_status> "stable" .


###  http://data.europa.eu/949/wheelSetGauge
:wheelSetGauge rdf:type owl:ObjectProperty ,
                        owl:FunctionalProperty ;
               rdfs:domain [ rdf:type owl:Class ;
                             owl:unionOf ( :Track
                                           :VehicleType
                                         )
                           ] ;
               rdfs:range <http://www.w3.org/2004/02/skos/core#Concept> ;
               :eratvIndex "4.1.3" ;
               :isCoreParameter "true"^^xsd:boolean ;
               :rinfIndex "1.1.1.1.4.1" ,
                          "1.2.1.0.4.1" ;
               <http://purl.org/dc/terms/created> "2020-07-29"^^xsd:date ;
               <http://purl.org/dc/terms/modified> "2021-09-10"^^xsd:date ;
               rdfs:comment "A single value expressed in millimetres that identifies the track and vehicle wheel set gauge. The allowed values for this property belong to the SKOS Concept Scheme http://data.europa.eu/949/concepts/nominal-track-gauges/NominalTrackGauges"@en ;
               rdfs:isDefinedBy <http://data.europa.eu/949/> ;
               rdfs:label "Nominal track gauge"@en ;
               <http://www.w3.org/2003/06/sw-vocab-status/ns#term_status> "stable" .


###  http://data.europa.eu/949/wheelSetGaugeChangeoverFacility
:wheelSetGaugeChangeoverFacility rdf:type owl:ObjectProperty ,
                                          owl:FunctionalProperty ;
                                 rdfs:domain :VehicleType ;
                                 rdfs:range <http://www.w3.org/2004/02/skos/core#Concept> ;
                                 :eratvIndex "4.1.11" ;
                                 <http://purl.org/dc/terms/created> "2020-09-01"^^xsd:date ;
                                 <http://purl.org/dc/terms/modified> "2021-08-25"^^xsd:date ;
                                 rdfs:comment "Wheelset gauge changeover facility. The allowed values for this property belong to the SKOS Concept Scheme http://data.europa.eu/949/concepts/gauge-changeover-facilities/GaugeChangeoverFacilities"@en ;
                                 rdfs:isDefinedBy <http://data.europa.eu/949/> ;
                                 rdfs:label "wheelset gauge changeover facility"@en ;
                                 <http://www.w3.org/2003/06/sw-vocab-status/ns#term_status> "stable" .


###  http://www.w3.org/2003/01/geo/wgs84_pos#location
<http://www.w3.org/2003/01/geo/wgs84_pos#location> rdf:type owl:ObjectProperty .


#################################################################
#    Data properties
#################################################################

###  http://data.europa.eu/949/accelerationLevelCrossing
:accelerationLevelCrossing rdf:type owl:DatatypeProperty ,
                                    owl:FunctionalProperty ;
                           rdfs:domain :Track ;
                           rdfs:range xsd:string ;
                           :rinfIndex "1.1.1.1.7.3" ;
                           <http://purl.org/dc/terms/created> "2021-08-03"^^xsd:date ;
                           <http://purl.org/dc/terms/modified> "2021-09-11"^^xsd:date ;
                           rdfs:comment "Existence of limit for acceleration of train if stopping or recovering speed close to a level crossing expressed in a specific reference acceleration curve."@en ;
                           rdfs:isDefinedBy <http://data.europa.eu/949/> ;
                           rdfs:label "Acceleration allowed at level crossing"@en ;
                           <http://www.w3.org/2003/06/sw-vocab-status/ns#term_status> "stable" .


###  http://data.europa.eu/949/additionalBrakingInformationDocument
:additionalBrakingInformationDocument rdf:type owl:DatatypeProperty ;
                                      rdfs:domain :Track ;
                                      rdfs:range xsd:string ;
                                      :rinfIndex "1.1.1.3.11.3" ;
                                      <http://purl.org/dc/terms/created> "2020-08-24"^^xsd:date ;
                                      <http://purl.org/dc/terms/modified> "2021-09-12"^^xsd:date ;
                                      rdfs:comment "Electronic document available in two EU languages from the IM stored by the Agency providing additional information as defined in point (2) of point 4.2.2.6.2 of the Annex to Regulation XXX - OPE TSI."@en ;
                                      rdfs:isDefinedBy <http://data.europa.eu/949/> ;
                                      rdfs:label "Documents available by the IM relating to braking performance"@en ;
                                      <http://www.w3.org/2003/06/sw-vocab-status/ns#term_status> "stable" .


###  http://data.europa.eu/949/alternativeName
:alternativeName rdf:type owl:DatatypeProperty ,
                          owl:FunctionalProperty ;
                 rdfs:domain :VehicleType ;
                 rdfs:range xsd:string ;
                 :eratvIndex 1.2 ;
                 <http://purl.org/dc/terms/created> "2020-07-29"^^xsd:date ;
                 <http://purl.org/dc/terms/modified> "2020-07-29"^^xsd:date ;
                 rdfs:comment "Alternative name of a vehicle."@en ;
                 rdfs:isDefinedBy <http://data.europa.eu/949/> ;
                 rdfs:label "alternative name"@en ;
                 <http://www.w3.org/2003/06/sw-vocab-status/ns#term_status> "stable" .


###  http://data.europa.eu/949/altitudeRange
:altitudeRange rdf:type owl:DatatypeProperty ;
               rdfs:domain :VehicleType ;
               rdfs:range xsd:string ;
               :eratvIndex "4.3.2" ;
               <http://purl.org/dc/terms/created> "2021-08-26"^^xsd:date ;
               <http://purl.org/dc/terms/modified> "2021-08-26"^^xsd:date ;
               rdfs:comment "Altitude range."@en ;
               rdfs:isDefinedBy <http://data.europa.eu/949/> ;
               rdfs:label "altitude range"@en ;
               <http://www.w3.org/2003/06/sw-vocab-status/ns#term_status> "stable" .


###  http://data.europa.eu/949/altitudeRangeDetail
:altitudeRangeDetail rdf:type owl:DatatypeProperty ;
                     rdfs:domain :VehicleType ;
                     rdfs:range xsd:integer ;
                     :eratvIndex "4.3.2.1" ;
                     <http://purl.org/dc/terms/created> "2021-08-26"^^xsd:date ;
                     <http://purl.org/dc/terms/modified> "2021-08-26"^^xsd:date ;
                     rdfs:comment "Altitude range value for 'X' if value 'AX' is selected in altitude range."@en ;
                     rdfs:isDefinedBy <http://data.europa.eu/949/> ;
                     rdfs:label "altitude range detail"@en ;
                     <http://www.w3.org/2003/06/sw-vocab-status/ns#term_status> "stable" .


###  http://data.europa.eu/949/areaBoardingAid
:areaBoardingAid rdf:type owl:DatatypeProperty ,
                          owl:FunctionalProperty ;
                 rdfs:domain :Platform ;
                 rdfs:range xsd:integer ;
                 :isCoreParameter "true"^^xsd:boolean ;
                 :rinfIndex "1.2.1.0.6.7" ;
                 <http://purl.org/dc/terms/created> "2021-08-02"^^xsd:date ;
                 <http://purl.org/dc/terms/modified> "2021-08-02"^^xsd:date ;
                 rdfs:comment "Information of the train access level for which the boarding aid can be used. Data is presented as the vertical difference that is overcome by the platform boarding aid in millimetres. The value â0â means that the platform is not equipped with a platform boarding aid."@en ;
                 rdfs:isDefinedBy <http://data.europa.eu/949/> ;
                 rdfs:label "Areas of use of the platform boarding aid"@en ;
                 <http://www.w3.org/2003/06/sw-vocab-status/ns#term_status> "stable" .


###  http://data.europa.eu/949/assistanceStartingTrain
:assistanceStartingTrain rdf:type owl:DatatypeProperty ,
                                  owl:FunctionalProperty ;
                         rdfs:domain :Platform ;
                         rdfs:range xsd:boolean ;
                         :isCoreParameter "true"^^xsd:boolean ;
                         :rinfIndex "1.2.1.0.6.6" ;
                         <http://purl.org/dc/terms/created> "2021-08-02"^^xsd:date ;
                         <http://purl.org/dc/terms/modified> "2021-08-02"^^xsd:date ;
                         rdfs:comment "Indication of existence of equipment or staff supporting the train crew in starting the train."@en ;
                         rdfs:isDefinedBy <http://data.europa.eu/949/> ;
                         rdfs:label "Existence of platform assistance for starting train"@en ;
                         <http://www.w3.org/2003/06/sw-vocab-status/ns#term_status> "stable" .


###  http://data.europa.eu/949/automaticDroppingDeviceRequired
:automaticDroppingDeviceRequired rdf:type owl:DatatypeProperty ,
                                          owl:FunctionalProperty ;
                                 rdfs:domain :Track ;
                                 rdfs:range xsd:boolean ;
                                 :rinfIndex "1.1.1.2.5.3" ;
                                 <http://purl.org/dc/terms/created> "2020-08-25"^^xsd:date ;
                                 <http://purl.org/dc/terms/modified> "2021-09-12"^^xsd:date ;
                                 rdfs:comment "Indication of whether an automatic dropping device (ADD) required on the vehicle."@en ;
                                 rdfs:isDefinedBy <http://data.europa.eu/949/> ;
                                 rdfs:label "Automatic dropping device required"@en ;
                                 <http://www.w3.org/2003/06/sw-vocab-status/ns#term_status> "stable" .


###  http://data.europa.eu/949/axleSpacing
:axleSpacing rdf:type owl:DatatypeProperty ,
                      owl:FunctionalProperty ;
             rdfs:domain :VehicleType ;
             rdfs:range xsd:string ;
             :eratvIndex "4.5.3.4" ;
             <http://purl.org/dc/terms/created> "2020-08-24"^^xsd:date ;
             <http://purl.org/dc/terms/modified> "2021-08-26"^^xsd:date ;
             rdfs:comment "Position of the axles along the unit. a: Distance between axles; b: Distance from end axle to the end of the nearest coupling plane; c: distance between two inside axles."@en ;
             rdfs:isDefinedBy <http://data.europa.eu/949/> ;
             rdfs:label "axle spacing"@en ;
             <http://www.w3.org/2003/06/sw-vocab-status/ns#term_status> "stable" .


###  http://data.europa.eu/949/boardingAids
:boardingAids rdf:type owl:DatatypeProperty ;
              rdfs:domain :VehicleType ;
              rdfs:range xsd:string ;
              :eratvIndex "4.12.3.2" ;
              <http://purl.org/dc/terms/created> "2021-08-31"^^xsd:date ;
              <http://purl.org/dc/terms/modified> "2021-08-31"^^xsd:date ;
              rdfs:comment "Description of any integrated boarding aids (if provided)."@en ;
              rdfs:isDefinedBy <http://data.europa.eu/949/> ;
              rdfs:label "boarding aids"@en ;
              <http://www.w3.org/2003/06/sw-vocab-status/ns#term_status> "stable" .


###  http://data.europa.eu/949/brakeWeightPercentage
:brakeWeightPercentage rdf:type owl:DatatypeProperty ,
                                owl:FunctionalProperty ;
                       rdfs:domain :VehicleType ;
                       rdfs:range xsd:string ;
                       :eratvIndex "4.7.6" ;
                       <http://purl.org/dc/terms/created> "2020-08-24"^^xsd:date ;
                       <http://purl.org/dc/terms/modified> "2021-08-26"^^xsd:date ;
                       rdfs:comment "Brake weight percentage (lambda) or Braked mass."@en ;
                       rdfs:isDefinedBy <http://data.europa.eu/949/> ;
                       rdfs:label "brake weight percentage"@en ;
                       <http://www.w3.org/2003/06/sw-vocab-status/ns#term_status> "stable" .


###  http://data.europa.eu/949/bridge
:bridge rdf:type owl:DatatypeProperty ;
        rdfs:domain :Track ;
        rdfs:range xsd:boolean ;
        rdfs:isDefinedBy <http://data.europa.eu/949/> ;
        rdfs:label "is bridge"@en ;
        <http://www.w3.org/2004/02/skos/core#definition> "Whether or not a track is associated with a bridge."@en .


###  http://data.europa.eu/949/cantDefficiency
:cantDefficiency rdf:type owl:DatatypeProperty ;
                 rdfs:domain :VehicleType ;
                 rdfs:range xsd:integer ;
                 :eratvIndex "4.6.1" ;
                 <http://purl.org/dc/terms/created> "2021-08-26"^^xsd:date ;
                 <http://purl.org/dc/terms/modified> "2021-08-26"^^xsd:date ;
                 rdfs:comment "Cant deficiency (maximum uncompensated lateral acceleration) for which the vehicle has been assessed. For dual gauge vehicles values for each gauge have to be indicated."@en ;
                 rdfs:isDefinedBy <http://data.europa.eu/949/> ;
                 rdfs:label "cant defficiency"@en ;
                 <http://www.w3.org/2003/06/sw-vocab-status/ns#term_status> "stable" .


###  http://data.europa.eu/949/cantDeficiency
:cantDeficiency rdf:type owl:DatatypeProperty ,
                         owl:FunctionalProperty ;
                rdfs:domain :Track ;
                rdfs:range xsd:integer ;
                :isCoreParameter "true"^^xsd:boolean ;
                :rinfIndex "1.1.1.1.4.2" ;
                <http://purl.org/dc/terms/created> "2020-08-24"^^xsd:date ;
                <http://purl.org/dc/terms/modified> "2021-09-10"^^xsd:date ;
                rdfs:comment "Maximum cant deficiency expressed in millimetres defined as difference between the applied cant and a higher equilibrium cant the line has been designed for."@en ;
                rdfs:isDefinedBy <http://data.europa.eu/949/> ;
                rdfs:label "Cant deficiency"@en ;
                <http://www.w3.org/2003/06/sw-vocab-status/ns#term_status> "stable" .


###  http://data.europa.eu/949/catenaryMaxRatedCurrent
:catenaryMaxRatedCurrent rdf:type owl:DatatypeProperty ;
                         rdfs:domain :VehicleType ;
                         rdfs:range xsd:double ;
                         :eratvIndex "4.10.3" ;
                         <http://purl.org/dc/terms/created> "2021-08-31"^^xsd:date ;
                         <http://purl.org/dc/terms/modified> "2021-08-31"^^xsd:date ;
                         rdfs:comment "Maximum rated current from the catenary (to be indicated for each electrical energy supply system the vehicle is equipped for), given in A."@en ;
                         rdfs:isDefinedBy <http://data.europa.eu/949/> ;
                         rdfs:label "catenary max rated current"@en ;
                         <http://www.w3.org/2003/06/sw-vocab-status/ns#term_status> "stable" .


###  http://data.europa.eu/949/certificate
:certificate rdf:type owl:DatatypeProperty ;
             rdfs:domain :VehicleType ;
             rdfs:range xsd:string ;
             <http://purl.org/dc/terms/created> "2022-06-15"^^xsd:date ;
             <http://purl.org/dc/terms/modified> "2022-06-15"^^xsd:date ;
             rdfs:comment "Denotes a certificate for this particular vehicleType."@en ;
             rdfs:isDefinedBy <http://data.europa.eu/949/> ;
             rdfs:label "certificate"@en ;
             <http://www.w3.org/2003/06/sw-vocab-status/ns#term_status> "stable"@en .


###  http://data.europa.eu/949/compatibilityProcedureDocument
:compatibilityProcedureDocument rdf:type owl:DatatypeProperty ;
                                rdfs:domain :Track ;
                                rdfs:range xsd:string ;
                                :rinfIndex "1.1.1.1.2.4.4" ;
                                <http://purl.org/dc/terms/created> "2020-08-24"^^xsd:date ;
                                <http://purl.org/dc/terms/modified> "2021-09-10"^^xsd:date ;
                                rdfs:comment "Document with the procedure(s) for static and dynamic route compatibility checks."@en ;
                                rdfs:isDefinedBy <http://data.europa.eu/949/> ;
                                rdfs:label "Document with the procedure(s) for static and dynamic route compatibility checks"@en ;
                                <http://www.w3.org/2003/06/sw-vocab-status/ns#term_status> "stable" .


###  http://data.europa.eu/949/complianceInfTsi
:complianceInfTsi rdf:type owl:DatatypeProperty ,
                           owl:FunctionalProperty ;
                  rdfs:domain :Tunnel ;
                  rdfs:range xsd:boolean ;
                  :isCoreParameter "true"^^xsd:boolean ;
                  :rinfIndex "1.1.1.1.8.8.1" ;
                  <http://purl.org/dc/terms/created> "2021-08-03"^^xsd:date ;
                  <http://purl.org/dc/terms/modified> "2021-08-03"^^xsd:date ;
                  rdfs:comment "Compliance of the tunnel with INF TSI at the maximum permitted speed."@en ;
                  rdfs:isDefinedBy <http://data.europa.eu/949/> ;
                  rdfs:label "Compliance of the tunnel with INF TSI"@en ;
                  <http://www.w3.org/2003/06/sw-vocab-status/ns#term_status> "stable" .


###  http://data.europa.eu/949/compositeBrakeBlockRetrofitted
:compositeBrakeBlockRetrofitted rdf:type owl:DatatypeProperty ;
                                rdfs:domain :Vehicle ;
                                rdfs:range xsd:boolean ;
                                <http://purl.org/dc/terms/created> "2020-11-23"^^xsd:date ;
                                <http://purl.org/dc/terms/modified> "2020-11-23"^^xsd:date ;
                                rdfs:comment "Indicates if a vehicle's composite brake block is retrofitted"@en ;
                                rdfs:isDefinedBy <http://data.europa.eu/949/> ;
                                rdfs:label "composite brake block retrofitted"@en ;
                                <http://www.w3.org/2003/06/sw-vocab-status/ns#term_status> "stable" .


###  http://data.europa.eu/949/conditionalRegenerativeBrake
:conditionalRegenerativeBrake rdf:type owl:DatatypeProperty ;
                              rdfs:domain :ContactLineSystem ;
                              rdfs:range xsd:boolean ;
                              :rinfIndex "1.1.1.2.2.4" ;
                              <http://purl.org/dc/terms/created> "2020-08-24"^^xsd:date ;
                              <http://purl.org/dc/terms/modified> "2021-09-12"^^xsd:date ;
                              rdfs:comment "Regenerative braking allowed under certain conditions."@en ;
                              rdfs:isDefinedBy <http://data.europa.eu/949/> ;
                              rdfs:label "conditional regenerative brake"@en ;
                              <http://www.w3.org/2003/06/sw-vocab-status/ns#term_status> "stable" .


###  http://data.europa.eu/949/conditionsTrainFormation
:conditionsTrainFormation rdf:type owl:DatatypeProperty ;
                          rdfs:domain :VehicleType ;
                          rdfs:range xsd:string ;
                          :eratvIndex "4.1.4" ;
                          <http://purl.org/dc/terms/created> "2021-08-25"^^xsd:date ;
                          <http://purl.org/dc/terms/modified> "2021-08-25"^^xsd:date ;
                          rdfs:comment "Conditions of use regarding train formation."@en ;
                          rdfs:isDefinedBy <http://data.europa.eu/949/> ;
                          rdfs:label "conditions train formation"@en ;
                          <http://www.w3.org/2003/06/sw-vocab-status/ns#term_status> "stable" .


###  http://data.europa.eu/949/crossSectionArea
:crossSectionArea rdf:type owl:DatatypeProperty ,
                           owl:FunctionalProperty ;
                  rdfs:domain :Tunnel ;
                  rdfs:range xsd:integer ;
                  :rinfIndex "1.1.1.1.8.8" ;
                  <http://purl.org/dc/terms/created> "2021-08-03"^^xsd:date ;
                  <http://purl.org/dc/terms/modified> "2021-08-03"^^xsd:date ;
                  rdfs:comment "Smallest cross section area in square metres of the tunnel."@en ;
                  rdfs:isDefinedBy <http://data.europa.eu/949/> ;
                  rdfs:label "Cross section area"@en ;
                  <http://www.w3.org/2003/06/sw-vocab-status/ns#term_status> "stable" .


###  http://data.europa.eu/949/currentLimitationRequired
:currentLimitationRequired rdf:type owl:DatatypeProperty ;
                           rdfs:domain :ContactLineSystem ;
                           rdfs:range xsd:boolean ;
                           :rinfIndex "1.1.1.2.5.1" ;
                           <http://purl.org/dc/terms/created> "2020-08-25"^^xsd:date ;
                           <http://purl.org/dc/terms/modified> "2021-09-12"^^xsd:date ;
                           rdfs:comment "Indication of whether an on board current or power limitation function on vehicles is required."@en ;
                           rdfs:isDefinedBy <http://data.europa.eu/949/> ;
                           rdfs:label "Current or power limitation on board required"@en ;
                           <http://www.w3.org/2003/06/sw-vocab-status/ns#term_status> "stable" .


###  http://data.europa.eu/949/dangerousGoodsTankCode
:dangerousGoodsTankCode rdf:type owl:DatatypeProperty ;
                        rdfs:domain :VehicleType ;
                        rdfs:range xsd:string ;
                        :eratvIndex "4.1.9" ;
                        <http://purl.org/dc/terms/created> "2021-08-25"^^xsd:date ;
                        <http://purl.org/dc/terms/modified> "2021-08-25"^^xsd:date ;
                        rdfs:comment "Dangerous goods for which the vehicle is suitable (tank code)."@en ;
                        rdfs:isDefinedBy <http://data.europa.eu/949/> ;
                        rdfs:label "dangerous goods tank code"@en ;
                        <http://www.w3.org/2003/06/sw-vocab-status/ns#term_status> "stable" .


###  http://data.europa.eu/949/demonstrationENE
:demonstrationENE rdf:type owl:DatatypeProperty ;
                  rdfs:domain :Track ;
                  rdfs:range xsd:string ;
                  :rinfIndex "1.1.1.2.1.2" ;
                  <http://purl.org/dc/terms/created> "2021-08-08"^^xsd:date ;
                  <http://purl.org/dc/terms/modified> "2021-09-11"^^xsd:date ;
                  rdfs:comment "Unique number for EI declarations concerning requirements of ENE (ENErgy subsytem) on the specific track."@en ;
                  rdfs:isDefinedBy <http://data.europa.eu/949/> ;
                  rdfs:label "EI declaration of demonstration for track (ENE)"@en ;
                  <http://www.w3.org/2003/06/sw-vocab-status/ns#term_status> "stable" .


###  http://data.europa.eu/949/demonstrationINF
:demonstrationINF rdf:type owl:DatatypeProperty ;
                  rdfs:domain [ rdf:type owl:Class ;
                                owl:unionOf ( :Siding
                                              :Track
                                            )
                              ] ;
                  rdfs:range xsd:string ;
                  :rinfIndex "1.1.1.1.1.2" ,
                             "1.2.1.0.1.2" ,
                             "1.2.2.0.1.2" ;
                  <http://purl.org/dc/terms/created> "2021-08-03"^^xsd:date ;
                  <http://purl.org/dc/terms/modified> "2021-09-10"^^xsd:date ;
                  rdfs:comment "Unique number for EI declarations concerning requirements of INF (INFrastructure) TSI."@en ;
                  rdfs:isDefinedBy <http://data.europa.eu/949/> ;
                  rdfs:label "EI declaration of demonstration for track/siding [INF]"@en ;
                  <http://www.w3.org/2003/06/sw-vocab-status/ns#term_status> "stable" .


###  http://data.europa.eu/949/demonstrationSRT
:demonstrationSRT rdf:type owl:DatatypeProperty ;
                  rdfs:domain :Tunnel ;
                  rdfs:range xsd:string ;
                  :rinfIndex "1.1.1.1.8.6" ,
                             "1.2.1.0.5.4" ,
                             "1.2.2.0.5.4" ;
                  <http://purl.org/dc/terms/created> "2021-08-03"^^xsd:date ;
                  <http://purl.org/dc/terms/modified> "2021-08-11"^^xsd:date ;
                  rdfs:comment "Unique number for EI declarations concerning requirements of SRT (Safety in Railway Tunnels) TSI for infrastructure system."@en ;
                  rdfs:isDefinedBy <http://data.europa.eu/949/> ;
                  rdfs:label "EI declaration of demonstration for tunnel (SRT)"@en ;
                  <http://www.w3.org/2003/06/sw-vocab-status/ns#term_status> "stable" .


###  http://data.europa.eu/949/designMassExceptionalPayload
:designMassExceptionalPayload rdf:type owl:DatatypeProperty ,
                                       owl:FunctionalProperty ;
                              rdfs:domain :VehicleType ;
                              rdfs:range xsd:integer ;
                              :eratvIndex "4.5.2.3" ;
                              <http://purl.org/dc/terms/created> "2020-08-24"^^xsd:date ;
                              <http://purl.org/dc/terms/modified> "2020-11-03"^^xsd:date ;
                              rdfs:comment "Design mass under exceptional payload."@en ;
                              rdfs:isDefinedBy <http://data.europa.eu/949/> ;
                              rdfs:label "design mass under exceptional payload"@en ;
                              <http://www.w3.org/2003/06/sw-vocab-status/ns#term_status> "stable" .


###  http://data.europa.eu/949/designMassNormalPayload
:designMassNormalPayload rdf:type owl:DatatypeProperty ,
                                  owl:FunctionalProperty ;
                         rdfs:domain :VehicleType ;
                         rdfs:range xsd:integer ;
                         :eratvIndex "4.5.2.2" ;
                         <http://purl.org/dc/terms/created> "2020-08-24"^^xsd:date ;
                         <http://purl.org/dc/terms/modified> "2020-11-03"^^xsd:date ;
                         rdfs:comment "Design mass under normal payload."@en ;
                         rdfs:isDefinedBy <http://data.europa.eu/949/> ;
                         rdfs:label "design mass under normal payload"@en ;
                         <http://www.w3.org/2003/06/sw-vocab-status/ns#term_status> "stable" .


###  http://data.europa.eu/949/designMassWorkingOrder
:designMassWorkingOrder rdf:type owl:DatatypeProperty ,
                                 owl:FunctionalProperty ;
                        rdfs:domain :VehicleType ;
                        rdfs:range xsd:integer ;
                        :eratvIndex "4.5.2.1" ;
                        <http://purl.org/dc/terms/created> "2020-08-24"^^xsd:date ;
                        <http://purl.org/dc/terms/modified> "2020-11-03"^^xsd:date ;
                        rdfs:comment "Design mass in working order."@en ;
                        rdfs:isDefinedBy <http://data.europa.eu/949/> ;
                        rdfs:label "design mass in working order"@en ;
                        <http://www.w3.org/2003/06/sw-vocab-status/ns#term_status> "stable" .


###  http://data.europa.eu/949/dieselThermalAllowed
:dieselThermalAllowed rdf:type owl:DatatypeProperty ,
                               owl:FunctionalProperty ;
                      rdfs:domain :Tunnel ;
                      rdfs:range xsd:boolean ;
                      :rinfIndex "1.2.1.0.5.9" ;
                      <http://purl.org/dc/terms/created> "2021-08-09"^^xsd:date ;
                      <http://purl.org/dc/terms/modified> "2021-08-09"^^xsd:date ;
                      rdfs:comment "Indication whether it is allowed to use diesel or other thermal traction in the tunnel."@en ;
                      rdfs:isDefinedBy <http://data.europa.eu/949/> ;
                      rdfs:label "Diesel or other thermal traction allowed"@en ;
                      <http://www.w3.org/2003/06/sw-vocab-status/ns#term_status> "stable" .


###  http://data.europa.eu/949/distSignToPhaseEnd
:distSignToPhaseEnd rdf:type owl:DatatypeProperty ,
                             owl:FunctionalProperty ;
                    rdfs:domain :Track ;
                    rdfs:range xsd:integer ;
                    :rinfIndex "1.1.1.2.4.3" ;
                    <http://purl.org/dc/terms/created> "2021-08-08"^^xsd:date ;
                    <http://purl.org/dc/terms/modified> "2021-09-12"^^xsd:date ;
                    rdfs:comment "Distance between the signboard authorizing the driver to âraise pantographâ or âclose the circuit breakerâ after passing the phase separation and the end of the phase separation section. Specific for route compatibility check on French network."@en ;
                    rdfs:isDefinedBy <http://data.europa.eu/949/> ;
                    rdfs:label "Distance between signboard and phase separation ending"@en ;
                    <http://www.w3.org/2003/06/sw-vocab-status/ns#term_status> "stable" .


###  http://data.europa.eu/949/drivingCabs
:drivingCabs rdf:type owl:DatatypeProperty ,
                      owl:FunctionalProperty ;
             rdfs:domain :VehicleType ;
             rdfs:range xsd:integer ;
             :eratvIndex "4.1.1" ;
             <http://purl.org/dc/terms/created> "2021-08-24"^^xsd:date ;
             <http://purl.org/dc/terms/modified> "2021-08-24"^^xsd:date ;
             rdfs:comment "Number of driving cabs. For wagons the number of driving cabs is to be set to zero (0)."@en ;
             rdfs:isDefinedBy <http://data.europa.eu/949/> ;
             rdfs:label "driving cabs"@en ;
             <http://www.w3.org/2003/06/sw-vocab-status/ns#term_status> "stable" .


###  http://data.europa.eu/949/eddyCurrentBrakePrevention
:eddyCurrentBrakePrevention rdf:type owl:DatatypeProperty ,
                                     owl:FunctionalProperty ;
                            rdfs:domain :VehicleType ;
                            rdfs:range xsd:boolean ;
                            :eratvIndex "4.7.4.1.2" ;
                            <http://purl.org/dc/terms/created> "2020-08-24"^^xsd:date ;
                            <http://purl.org/dc/terms/modified> "2020-11-03"^^xsd:date ;
                            rdfs:comment "Possibility of preventing the use of the eddy current track brake (only if fitted with eddy current brake)"@en ;
                            rdfs:isDefinedBy <http://data.europa.eu/949/> ;
                            rdfs:label "eddy current brake prevention"@en ;
                            <http://www.w3.org/2003/06/sw-vocab-status/ns#term_status> "stable" .


###  http://data.europa.eu/949/eddyCurrentBrakingConditionsDocument
:eddyCurrentBrakingConditionsDocument rdf:type owl:DatatypeProperty ;
                                      rdfs:domain :Track ;
                                      rdfs:range xsd:string ;
                                      :rinfIndex "1.1.1.1.6.4" ;
                                      <http://purl.org/dc/terms/created> "2020-08-24"^^xsd:date ;
                                      <http://purl.org/dc/terms/modified> "2021-09-10"^^xsd:date ;
                                      rdfs:comment "Document with the conditions for the use of eddy current brakes."@en ;
                                      rdfs:isDefinedBy <http://data.europa.eu/949/> ;
                                      rdfs:label "Document with the conditions for the use of eddy current brakes"@en ;
                                      <http://www.w3.org/2003/06/sw-vocab-status/ns#term_status> "stable" .


###  http://data.europa.eu/949/eddyCurrentBrakingFitted
:eddyCurrentBrakingFitted rdf:type owl:DatatypeProperty ,
                                   owl:FunctionalProperty ;
                          rdfs:domain :VehicleType ;
                          rdfs:range xsd:boolean ;
                          :eratvIndex "4.7.4.1.1" ;
                          :isCoreParameter "true"^^xsd:boolean ;
                          <http://purl.org/dc/terms/created> "2022-09-06"^^xsd:date ;
                          rdfs:comment "Eddy current track brake fitted. New property defined to distinghish it from eddyCurrentBraking which is a RINF SKOS property."@en ;
                          rdfs:isDefinedBy "http://data.europa.eu/949/"^^xsd:anyURI ;
                          rdfs:label "eddy current braking fitted"@en .


###  http://data.europa.eu/949/emergencyBrake
:emergencyBrake rdf:type owl:DatatypeProperty ,
                         owl:FunctionalProperty ;
                rdfs:domain :VehicleType ;
                rdfs:range xsd:string ;
                :eratvIndex "4.7.5" ;
                <http://purl.org/dc/terms/created> "2020-08-24"^^xsd:date ;
                <http://purl.org/dc/terms/modified> "2021-08-26"^^xsd:date ;
                rdfs:comment "Stopping distance and deceleration profile for each load condition per design maximum speed."@en ;
                rdfs:isDefinedBy <http://data.europa.eu/949/> ;
                rdfs:label "emergency braking"@en ;
                <http://www.w3.org/2003/06/sw-vocab-status/ns#term_status> "stable" .


###  http://data.europa.eu/949/endIntrinsicCoordinate
:endIntrinsicCoordinate rdf:type owl:DatatypeProperty ;
                        rdfs:domain :NetElement ;
                        rdfs:range xsd:double ;
                        <http://purl.org/dc/terms/created> "2021-04-01"^^xsd:date ;
                        <http://purl.org/dc/terms/modified> "2021-04-01"^^xsd:date ;
                        rdfs:comment "Indicates the coordinate point where a linear object ends."@en ;
                        rdfs:isDefinedBy <http://data.europa.eu/949/> ;
                        rdfs:label "end intrinsic coordinate"@en ;
                        <http://www.w3.org/2003/06/sw-vocab-status/ns#term_status> "stable" .


###  http://data.europa.eu/949/energyMeterInstalled
:energyMeterInstalled rdf:type owl:DatatypeProperty ;
                      rdfs:domain :VehicleType ;
                      rdfs:range xsd:boolean ;
                      :eratvIndex "4.10.12" ;
                      <http://purl.org/dc/terms/created> "2021-08-31"^^xsd:date ;
                      <http://purl.org/dc/terms/modified> "2021-08-31"^^xsd:date ;
                      rdfs:comment "TSI conform energy meter for billing purposes installed on board."@en ;
                      rdfs:isDefinedBy <http://data.europa.eu/949/> ;
                      rdfs:label "energy meter installed"@en ;
                      <http://www.w3.org/2003/06/sw-vocab-status/ns#term_status> "stable" .


###  http://data.europa.eu/949/energySupplyMaxPower
:energySupplyMaxPower rdf:type owl:DatatypeProperty ;
                      rdfs:domain :VehicleType ;
                      rdfs:range xsd:double ;
                      :eratvIndex "4.10.2" ;
                      <http://purl.org/dc/terms/created> "2021-08-31"^^xsd:date ;
                      <http://purl.org/dc/terms/modified> "2021-08-31"^^xsd:date ;
                      rdfs:comment "Maximum power (to be indicated for each energy supply system the vehicle is equipped for), given in kW."@en ;
                      rdfs:isDefinedBy <http://data.europa.eu/949/> ;
                      rdfs:label "energy supply max power"@en ;
                      <http://www.w3.org/2003/06/sw-vocab-status/ns#term_status> "stable" .


###  http://data.europa.eu/949/energySupplySystemTSICompliant
:energySupplySystemTSICompliant rdf:type owl:DatatypeProperty ;
                                rdfs:domain :ContactLineSystem ;
                                rdfs:range xsd:boolean ;
                                :rinfIndex "1.1.1.2.2.1.2.1" ;
                                <http://purl.org/dc/terms/created> "2020-08-24"^^xsd:date ;
                                <http://purl.org/dc/terms/modified> "2021-08-06"^^xsd:date ;
                                rdfs:comment "Indication if the traction supply system (nominal voltage and frequency) is fully compliant with TSI."@en ;
                                rdfs:isDefinedBy <http://data.europa.eu/949/> ;
                                rdfs:label "Energy supply system TSI compliant"@en ;
                                <http://www.w3.org/2003/06/sw-vocab-status/ns#term_status> "stable" .


###  http://data.europa.eu/949/etcsDataCommApp
:etcsDataCommApp rdf:type owl:DatatypeProperty ,
                          owl:FunctionalProperty ;
                 rdfs:domain :VehicleType ;
                 rdfs:range xsd:string ;
                 :eratvIndex "4.13.2.9" ;
                 <http://purl.org/dc/terms/created> "2021-08-31"^^xsd:date ;
                 <http://purl.org/dc/terms/modified> "2021-08-31"^^xsd:date ;
                 rdfs:comment "Data communication application for ETCS implementation."@en ;
                 rdfs:isDefinedBy <http://data.europa.eu/949/> ;
                 rdfs:label "ETCS data communication application"@en ;
                 <http://www.w3.org/2003/06/sw-vocab-status/ns#term_status> "stable" .


###  http://data.europa.eu/949/etcsInfillLineAccess
:etcsInfillLineAccess rdf:type owl:DatatypeProperty ,
                               owl:FunctionalProperty ;
                      rdfs:domain :Track ;
                      rdfs:range xsd:boolean ;
                      :isCoreParameter "true"^^xsd:boolean ;
                      :rinfIndex "1.1.1.3.2.3" ;
                      <http://purl.org/dc/terms/created> "2021-08-08"^^xsd:date ;
                      <http://purl.org/dc/terms/modified> "2021-09-12"^^xsd:date ;
                      rdfs:comment "Indication whether infill is required to access the line for safety reasons."@en ;
                      rdfs:isDefinedBy <http://data.europa.eu/949/> ;
                      rdfs:label "ETCS infill necessary for line access"@en ;
                      <http://www.w3.org/2003/06/sw-vocab-status/ns#term_status> "stable" .


###  http://data.europa.eu/949/etcsNationalApplications
:etcsNationalApplications rdf:type owl:DatatypeProperty ;
                          rdfs:domain :VehicleType ;
                          rdfs:range xsd:string ;
                          :eratvIndex "4.13.1.4" ;
                          <http://purl.org/dc/terms/created> "2021-08-31"^^xsd:date ;
                          <http://purl.org/dc/terms/modified> "2021-08-31"^^xsd:date ;
                          rdfs:comment "ETCS national applications implemented (NID_XUSER of Packet 44)."@en ;
                          rdfs:isDefinedBy <http://data.europa.eu/949/> ;
                          rdfs:label "ETCS national applications"@en ;
                          <http://www.w3.org/2003/06/sw-vocab-status/ns#term_status> "stable" .


###  http://data.europa.eu/949/etcsNationalPacket44
:etcsNationalPacket44 rdf:type owl:DatatypeProperty ,
                               owl:FunctionalProperty ;
                      rdfs:domain :Track ;
                      rdfs:range xsd:boolean ;
                      :rinfIndex "1.1.1.3.2.5" ;
                      <http://purl.org/dc/terms/created> "2021-08-08"^^xsd:date ;
                      <http://purl.org/dc/terms/modified> "2021-09-12"^^xsd:date ;
                      rdfs:comment "Indication whether data for national packet 44 applications is transmitted between track and train."@en ;
                      rdfs:isDefinedBy <http://data.europa.eu/949/> ;
                      rdfs:label "ETCS national packet 44 application implemented"@en ;
                      <http://www.w3.org/2003/06/sw-vocab-status/ns#term_status> "stable" .


###  http://data.europa.eu/949/etcsOnBoardImplementation
:etcsOnBoardImplementation rdf:type owl:DatatypeProperty ,
                                    owl:FunctionalProperty ;
                           rdfs:domain :VehicleType ;
                           rdfs:range xsd:string ;
                           :eratvIndex "4.13.1.7" ;
                           <http://purl.org/dc/terms/created> "2021-08-31"^^xsd:date ;
                           <http://purl.org/dc/terms/modified> "2021-08-31"^^xsd:date ;
                           rdfs:comment "ETCS on-board implementation."@en ;
                           rdfs:isDefinedBy <http://data.europa.eu/949/> ;
                           rdfs:label "ETCS on-board implementation"@en ;
                           <http://www.w3.org/2003/06/sw-vocab-status/ns#term_status> "stable" .


###  http://data.europa.eu/949/etcsOptionalFunctions
:etcsOptionalFunctions rdf:type owl:DatatypeProperty ;
                       rdfs:domain :Track ;
                       rdfs:range xsd:string ;
                       :rinfIndex "1.1.1.3.2.7" ;
                       <http://purl.org/dc/terms/created> "2021-08-08"^^xsd:date ;
                       <http://purl.org/dc/terms/modified> "2021-09-12"^^xsd:date ;
                       rdfs:comment "Optional ETCS functions which might improve operation on the line."@en ;
                       rdfs:isDefinedBy <http://data.europa.eu/949/> ;
                       rdfs:label "ETCS optional functions"@en ;
                       <http://www.w3.org/2003/06/sw-vocab-status/ns#term_status> "unstable" .


###  http://data.europa.eu/949/ferromagneticWheelMaterial
:ferromagneticWheelMaterial rdf:type owl:DatatypeProperty ;
                            rdfs:domain :VehicleType ;
                            rdfs:range xsd:boolean ;
                            :eratvIndex "4.14.2.12" ;
                            <http://purl.org/dc/terms/created> "2021-09-01"^^xsd:date ;
                            <http://purl.org/dc/terms/modified> "2021-09-01"^^xsd:date ;
                            rdfs:comment "Wheel material is ferromagnetic."@en ;
                            rdfs:isDefinedBy <http://data.europa.eu/949/> ;
                            rdfs:label "ferromagnetic wheel material"@en ;
                            <http://www.w3.org/2003/06/sw-vocab-status/ns#term_status> "stable" .


###  http://data.europa.eu/949/fixedSeats
:fixedSeats rdf:type owl:DatatypeProperty ;
            rdfs:domain :VehicleType ;
            rdfs:range xsd:string ;
            :eratvIndex "4.12.1.1" ;
            <http://purl.org/dc/terms/created> "2021-08-31"^^xsd:date ;
            <http://purl.org/dc/terms/modified> "2021-08-31"^^xsd:date ;
            rdfs:comment "Number of fixed seats."@en ;
            rdfs:isDefinedBy <http://data.europa.eu/949/> ;
            rdfs:label "fixed seats"@en ;
            <http://www.w3.org/2003/06/sw-vocab-status/ns#term_status> "stable" .


###  http://data.europa.eu/949/flangeLubeForbidden
:flangeLubeForbidden rdf:type owl:DatatypeProperty ,
                              owl:FunctionalProperty ;
                     rdfs:domain :Track ;
                     rdfs:range xsd:boolean ;
                     :isCoreParameter "true"^^xsd:boolean ;
                     :rinfIndex "1.1.1.1.7.1" ;
                     <http://purl.org/dc/terms/created> "2021-08-08"^^xsd:date ;
                     <http://purl.org/dc/terms/modified> "2021-09-11"^^xsd:date ;
                     rdfs:comment "Indication whether the use of on-board device for flange lubrication is forbidden"@en ;
                     rdfs:isDefinedBy <http://data.europa.eu/949/> ;
                     rdfs:label "Use of flange lubrication forbidden"@en ;
                     <http://www.w3.org/2003/06/sw-vocab-status/ns#term_status> "stable" .


###  http://data.europa.eu/949/flangeLubeRules
:flangeLubeRules rdf:type owl:DatatypeProperty ;
                 rdfs:domain :TrainDetectionSystem ;
                 rdfs:range xsd:boolean ;
                 :rinfIndex "1.1.1.3.7.20" ;
                 <http://purl.org/dc/terms/created> "2021-08-08"^^xsd:date ;
                 <http://purl.org/dc/terms/modified> "2021-08-08"^^xsd:date ;
                 rdfs:comment "Indication whether rules for activation or deactivation of flange lubrication exist."@en ;
                 rdfs:isDefinedBy <http://data.europa.eu/949/> ;
                 rdfs:label "Existence of rules on on-board flange lubrication"@en ;
                 <http://www.w3.org/2003/06/sw-vocab-status/ns#term_status> "stable" .


###  http://data.europa.eu/949/flangeLubricationFitted
:flangeLubricationFitted rdf:type owl:DatatypeProperty ;
                         rdfs:domain :VehicleType ;
                         rdfs:range xsd:boolean ;
                         :eratvIndex "4.9.3.1" ;
                         <http://purl.org/dc/terms/created> "2021-08-31"^^xsd:date ;
                         <http://purl.org/dc/terms/modified> "2021-08-31"^^xsd:date ;
                         rdfs:comment "Indicates if the vehicle type is fitted for flange lubrication."@en ;
                         rdfs:isDefinedBy <http://data.europa.eu/949/> ;
                         rdfs:label "flange lubrication fitted"@en ;
                         <http://www.w3.org/2003/06/sw-vocab-status/ns#term_status> "stable" .


###  http://data.europa.eu/949/gaugingCheckLocation
:gaugingCheckLocation rdf:type owl:DatatypeProperty ;
                      rdfs:domain :Track ;
                      rdfs:range xsd:string ;
                      :rinfIndex "1.1.1.1.3.1.2" ,
                                 "1.2.1.0.3.5" ;
                      <http://purl.org/dc/terms/created> "2020-07-29"^^xsd:date ;
                      <http://purl.org/dc/terms/modified> "2021-09-10"^^xsd:date ;
                      rdfs:comment "Location of particular points requiring specific checks due to deviations from gauging. The location (generally the distance from the origin of the line to the centre) on a line is given in kilometres with decimals (precision of 0.001)."@en ;
                      rdfs:isDefinedBy <http://data.europa.eu/949/> ;
                      rdfs:label "Railway location of particular points requiring specific checks"@en ;
                      <http://www.w3.org/2003/06/sw-vocab-status/ns#term_status> "stable" .


###  http://data.europa.eu/949/gaugingTransversalDocument
:gaugingTransversalDocument rdf:type owl:DatatypeProperty ;
                            rdfs:domain :Track ;
                            rdfs:range xsd:string ;
                            :rinfIndex "1.1.1.1.3.1.3" ,
                                       "1.2.1.0.3.6" ;
                            <http://purl.org/dc/terms/created> "2020-08-24"^^xsd:date ;
                            <http://purl.org/dc/terms/modified> "2021-09-10"^^xsd:date ;
                            rdfs:comment "Document with the transversal section of the particular points requiring specific checks."@en ;
                            rdfs:isDefinedBy <http://data.europa.eu/949/> ;
                            rdfs:label "Document with the transversal section of the particular points requiring specific checks"@en ;
                            <http://www.w3.org/2003/06/sw-vocab-status/ns#term_status> "stable" .


###  http://data.europa.eu/949/gprsForETCS
:gprsForETCS rdf:type owl:DatatypeProperty ,
                      owl:FunctionalProperty ;
             rdfs:domain :Track ;
             rdfs:range xsd:boolean ;
             :rinfIndex "1.1.1.3.3.3.2" ;
             <http://purl.org/dc/terms/created> "2021-08-08"^^xsd:date ;
             <http://purl.org/dc/terms/modified> "2021-09-12"^^xsd:date ;
             rdfs:comment "Indication if GPRS can be used for ETCS."@en ;
             rdfs:isDefinedBy <http://data.europa.eu/949/> ;
             rdfs:label "GPRS for ETCS"@en ;
             <http://www.w3.org/2003/06/sw-vocab-status/ns#term_status> "stable" .


###  http://data.europa.eu/949/gprsImplementationArea
:gprsImplementationArea rdf:type owl:DatatypeProperty ;
                        rdfs:domain :Track ;
                        rdfs:range xsd:string ;
                        :rinfIndex "1.1.1.3.3.3.3" ;
                        <http://purl.org/dc/terms/created> "2021-08-09"^^xsd:date ;
                        <http://purl.org/dc/terms/modified> "2021-09-12"^^xsd:date ;
                        rdfs:comment "Indication of the area in which GPRS can be used for ETCS."@en ;
                        rdfs:isDefinedBy <http://data.europa.eu/949/> ;
                        rdfs:label "GPRS implementation area"@en ;
                        <http://www.w3.org/2003/06/sw-vocab-status/ns#term_status> "stable" .


###  http://data.europa.eu/949/gradient
:gradient rdf:type owl:DatatypeProperty ,
                   owl:FunctionalProperty ;
          rdfs:domain [ rdf:type owl:Class ;
                        owl:unionOf ( :GradientCurve
                                      :Siding
                                    )
                      ] ;
          rdfs:range xsd:double ;
          :rinfIndex "1.2.2.0.3.1" ;
          <http://purl.org/dc/terms/created> "2021-08-10"^^xsd:date ;
          <http://purl.org/dc/terms/modified> "2021-08-10"^^xsd:date ;
          rdfs:comment "Maximum value of the gradient for stabling tracks expressed in millimetres per metre."@en ;
          rdfs:isDefinedBy <http://data.europa.eu/949/> ;
          rdfs:label "Gradient for stabling tracks"@en ;
          <http://www.w3.org/2003/06/sw-vocab-status/ns#term_status> "stable" .


###  http://data.europa.eu/949/gradientProfile
:gradientProfile rdf:type owl:DatatypeProperty ;
                 rdfs:domain :Track ;
                 rdfs:range xsd:string ;
                 :isCoreParameter "true"^^xsd:boolean ;
                 :rinfIndex "1.1.1.1.3.6" ;
                 <http://purl.org/dc/terms/created> "2020-08-24"^^xsd:date ;
                 <http://purl.org/dc/terms/modified> "2021-09-10"^^xsd:date ;
                 rdfs:comment "Sequence of gradient values and locations of change in gradient."@en ;
                 rdfs:isDefinedBy <http://data.europa.eu/949/> ;
                 rdfs:label "Gradient profile"@en ;
                 <http://www.w3.org/2003/06/sw-vocab-status/ns#term_status> "stable" .


###  http://data.europa.eu/949/gsmRAdditionalInfo
:gsmRAdditionalInfo rdf:type owl:DatatypeProperty ;
                    rdfs:domain :Track ;
                    rdfs:range xsd:string ;
                    :rinfIndex "1.1.1.3.3.3.1" ;
                    <http://purl.org/dc/terms/created> "2021-08-08"^^xsd:date ;
                    <http://purl.org/dc/terms/modified> "2021-09-12"^^xsd:date ;
                    rdfs:comment "Any additional information on network characteristics or corresponding document available from the IM and stored by the Agency, e.g.; interference level, leading to the recommendation of additional on-board protection."@en ;
                    rdfs:isDefinedBy <http://data.europa.eu/949/> ;
                    rdfs:label "Additional information on network characteristics"@en ;
                    <http://www.w3.org/2003/06/sw-vocab-status/ns#term_status> "stable" .


###  http://data.europa.eu/949/gsmRNoCoverage
:gsmRNoCoverage rdf:type owl:DatatypeProperty ,
                         owl:FunctionalProperty ;
                rdfs:domain :Track ;
                rdfs:range xsd:boolean ;
                :isCoreParameter "true"^^xsd:boolean ;
                :rinfIndex "1.1.1.3.3.8" ;
                <http://purl.org/dc/terms/created> "2021-08-09"^^xsd:date ;
                <http://purl.org/dc/terms/modified> "2021-09-12"^^xsd:date ;
                rdfs:comment "Indication if there is no GSMR coverage."@en ;
                rdfs:isDefinedBy <http://data.europa.eu/949/> ;
                rdfs:label "No GSM-R coverage"@en ;
                <http://www.w3.org/2003/06/sw-vocab-status/ns#term_status> "stable" .


###  http://data.europa.eu/949/gsmRSetsInDrivingCab
:gsmRSetsInDrivingCab rdf:type owl:DatatypeProperty ;
                      rdfs:domain :VehicleType ;
                      rdfs:range xsd:integer ;
                      :eratvIndex "4.13.2.2" ;
                      <http://purl.org/dc/terms/created> "2021-08-31"^^xsd:date ;
                      <http://purl.org/dc/terms/modified> "2021-08-31"^^xsd:date ;
                      rdfs:comment "Number of GSM-R mobile sets in driving cab for data transmission."@en ;
                      rdfs:isDefinedBy <http://data.europa.eu/949/> ;
                      rdfs:label "GSM-R sets in driving cab"@en ;
                      <http://www.w3.org/2003/06/sw-vocab-status/ns#term_status> "stable" .


###  http://data.europa.eu/949/hasAdditionalBrakingInformation
:hasAdditionalBrakingInformation rdf:type owl:DatatypeProperty ,
                                          owl:FunctionalProperty ;
                                 rdfs:domain :Track ;
                                 rdfs:range xsd:boolean ;
                                 :isCoreParameter "true"^^xsd:boolean ;
                                 :rinfIndex "1.1.1.3.11.2" ;
                                 <http://purl.org/dc/terms/created> "2020-08-24"^^xsd:date ;
                                 <http://purl.org/dc/terms/modified> "2021-09-12"^^xsd:date ;
                                 rdfs:comment "Availability by the IM of additional information as defined in 4.2.2.6.2 (2) Regulation XXX - OPE TSI."@en ;
                                 rdfs:isDefinedBy <http://data.europa.eu/949/> ;
                                 rdfs:label "Availability by the IM of additional information"@en ;
                                 <http://www.w3.org/2003/06/sw-vocab-status/ns#term_status> "stable" .


###  http://data.europa.eu/949/hasAutomaticDroppingDevice
:hasAutomaticDroppingDevice rdf:type owl:DatatypeProperty ,
                                     owl:FunctionalProperty ;
                            rdfs:domain :VehicleType ;
                            rdfs:range xsd:boolean ;
                            :eratvIndex "4.10.11" ;
                            <http://purl.org/dc/terms/created> "2020-08-25"^^xsd:date ;
                            <http://purl.org/dc/terms/modified> "2020-11-03"^^xsd:date ;
                            rdfs:comment "Automatic dropping device (ADD) fitted (to be indicated for each energy supply system the vehicle is equipped for)."@en ;
                            rdfs:isDefinedBy <http://data.europa.eu/949/> ;
                            rdfs:label "has automatic dropping device"@en ;
                            <http://www.w3.org/2003/06/sw-vocab-status/ns#term_status> "stable" .


###  http://data.europa.eu/949/hasBallast
:hasBallast rdf:type owl:DatatypeProperty ,
                     owl:FunctionalProperty ;
            rdfs:domain :Track ;
            rdfs:range xsd:boolean ;
            :rinfIndex "1.1.1.1.4.4" ;
            <http://purl.org/dc/terms/created> "2021-08-03"^^xsd:date ;
            <http://purl.org/dc/terms/modified> "2021-09-10"^^xsd:date ;
            rdfs:comment "Specifies whether track construction is with sleepers embedded in ballast or not.."@en ;
            rdfs:isDefinedBy <http://data.europa.eu/949/> ;
            rdfs:label "Existence of ballast"@en ;
            <http://www.w3.org/2003/06/sw-vocab-status/ns#term_status> "stable" .


###  http://data.europa.eu/949/hasCantDefficiencyCompensation
:hasCantDefficiencyCompensation rdf:type owl:DatatypeProperty ;
                                rdfs:domain :VehicleType ;
                                rdfs:range xsd:boolean ;
                                :eratvIndex "4.6.2" ;
                                <http://purl.org/dc/terms/created> "2021-08-26"^^xsd:date ;
                                <http://purl.org/dc/terms/modified> "2021-08-26"^^xsd:date ;
                                rdfs:comment "Vehicle equipped with a cant deficiency compensation system (tilting vehicle)."@en ;
                                rdfs:isDefinedBy <http://data.europa.eu/949/> ;
                                rdfs:label "has cant defficiency compensation"@en ;
                                <http://www.w3.org/2003/06/sw-vocab-status/ns#term_status> "stable" .


###  http://data.europa.eu/949/hasCurrentLimitation
:hasCurrentLimitation rdf:type owl:DatatypeProperty ,
                               owl:FunctionalProperty ;
                      rdfs:domain :VehicleType ;
                      rdfs:range xsd:boolean ;
                      :eratvIndex "4.10.14" ;
                      <http://purl.org/dc/terms/created> "2020-08-24"^^xsd:date ;
                      <http://purl.org/dc/terms/modified> "2020-11-03"^^xsd:date ;
                      rdfs:comment "Electric units equipped with power or current limitation function."@en ;
                      rdfs:isDefinedBy <http://data.europa.eu/949/> ;
                      rdfs:label "has current limitation"@en ;
                      <http://www.w3.org/2003/06/sw-vocab-status/ns#term_status> "stable" .


###  http://data.europa.eu/949/hasETCSRestrictionsConditions
:hasETCSRestrictionsConditions rdf:type owl:DatatypeProperty ,
                                        owl:FunctionalProperty ;
                               rdfs:domain :Track ;
                               rdfs:range xsd:boolean ;
                               :rinfIndex "1.1.1.3.2.6" ;
                               <http://purl.org/dc/terms/created> "2021-08-08"^^xsd:date ;
                               <http://purl.org/dc/terms/modified> "2021-09-12"^^xsd:date ;
                               rdfs:comment "Indication whether restrictions or conditions due to partial compliance with the CCS TSI exist."@en ;
                               rdfs:isDefinedBy <http://data.europa.eu/949/> ;
                               rdfs:label "Existence of operating restrictions or conditions"@en ;
                               <http://www.w3.org/2003/06/sw-vocab-status/ns#term_status> "stable" .


###  http://data.europa.eu/949/hasElectricShoreSupply
:hasElectricShoreSupply rdf:type owl:DatatypeProperty ,
                                 owl:FunctionalProperty ;
                        rdfs:domain :Siding ;
                        rdfs:range xsd:boolean ;
                        :isCoreParameter "true"^^xsd:boolean ;
                        :rinfIndex "1.2.2.0.4.6" ;
                        <http://purl.org/dc/terms/created> "2021-08-10"^^xsd:date ;
                        <http://purl.org/dc/terms/modified> "2021-08-10"^^xsd:date ;
                        rdfs:comment "Indication whether an installation for electric shore supply exists (fixed installation for servicing trains)."@en ;
                        rdfs:isDefinedBy <http://data.europa.eu/949/> ;
                        rdfs:label "Existence of electric shore supply"@en ;
                        <http://www.w3.org/2003/06/sw-vocab-status/ns#term_status> "stable" .


###  http://data.europa.eu/949/hasEmergencyPlan
:hasEmergencyPlan rdf:type owl:DatatypeProperty ,
                           owl:FunctionalProperty ;
                  rdfs:domain :Tunnel ;
                  rdfs:range xsd:boolean ;
                  :rinfIndex "1.1.1.1.8.9" ,
                             "1.2.1.0.5.6" ,
                             "1.2.2.0.5.6" ;
                  <http://purl.org/dc/terms/created> "2021-08-03"^^xsd:date ;
                  <http://purl.org/dc/terms/modified> "2021-08-10"^^xsd:date ;
                  rdfs:comment "Indication whether emergency plan exists."@en ;
                  rdfs:isDefinedBy <http://data.europa.eu/949/> ;
                  rdfs:label "Existence of emergency plan"@en ;
                  <http://www.w3.org/2003/06/sw-vocab-status/ns#term_status> "stable" .


###  http://data.europa.eu/949/hasExternalCleaning
:hasExternalCleaning rdf:type owl:DatatypeProperty ,
                              owl:FunctionalProperty ;
                     rdfs:domain :Siding ;
                     rdfs:range xsd:boolean ;
                     :isCoreParameter "true"^^xsd:boolean ;
                     :rinfIndex "1.2.2.0.4.2" ;
                     <http://purl.org/dc/terms/created> "2021-08-10"^^xsd:date ;
                     <http://purl.org/dc/terms/modified> "2021-08-10"^^xsd:date ;
                     rdfs:comment "Indication whether exists an installation for external cleaning facility (fixed installation for servicing trains) as defined in INF TSIs."@en ;
                     rdfs:isDefinedBy <http://data.europa.eu/949/> ;
                     rdfs:label "Existence of external cleaning facilities"@en ;
                     <http://www.w3.org/2003/06/sw-vocab-status/ns#term_status> "stable" .


###  http://data.europa.eu/949/hasHotAxleBoxDetector
:hasHotAxleBoxDetector rdf:type owl:DatatypeProperty ,
                                owl:FunctionalProperty ;
                       rdfs:domain :Track ;
                       rdfs:range xsd:boolean ;
                       :isCoreParameter "true"^^xsd:boolean ;
                       :rinfIndex "1.1.1.1.7.4" ;
                       <http://purl.org/dc/terms/created> "2020-08-24"^^xsd:date ;
                       <http://purl.org/dc/terms/modified> "2021-09-11"^^xsd:date ;
                       rdfs:comment "Existence of trackside hot axle box detector (HABD)."@en ;
                       rdfs:isDefinedBy <http://data.europa.eu/949/> ;
                       rdfs:label "Existence of trackside hot axle box detector (HABD)"@en ;
                       <http://www.w3.org/2003/06/sw-vocab-status/ns#term_status> "stable" .


###  http://data.europa.eu/949/hasLevelCrossings
:hasLevelCrossings rdf:type owl:DatatypeProperty ,
                            owl:FunctionalProperty ;
                   rdfs:domain :Track ;
                   rdfs:range xsd:boolean ;
                   :isCoreParameter "true"^^xsd:boolean ;
                   :rinfIndex "1.1.1.1.7.2" ;
                   <http://purl.org/dc/terms/created> "2021-08-03"^^xsd:date ;
                   <http://purl.org/dc/terms/modified> "2021-09-11"^^xsd:date ;
                   rdfs:comment "Indication whether level crossings (including pedestrian track crossing) exist on the section of line."@en ;
                   rdfs:isDefinedBy <http://data.europa.eu/949/> ;
                   rdfs:label "Existence of level crossings"@en ;
                   <http://www.w3.org/2003/06/sw-vocab-status/ns#term_status> "stable" .


###  http://data.europa.eu/949/hasLubricationDevicePrevention
:hasLubricationDevicePrevention rdf:type owl:DatatypeProperty ;
                                rdfs:domain :VehicleType ;
                                rdfs:range xsd:boolean ;
                                :eratvIndex "4.9.3.2" ;
                                <http://purl.org/dc/terms/created> "2021-08-31"^^xsd:date ;
                                <http://purl.org/dc/terms/modified> "2021-08-31"^^xsd:date ;
                                rdfs:comment "Possibility of preventing the use of the lubrication device (only if fitted with flange lubrication)."@en ;
                                rdfs:isDefinedBy <http://data.europa.eu/949/> ;
                                rdfs:label "has lubrication device prevention"@en ;
                                <http://www.w3.org/2003/06/sw-vocab-status/ns#term_status> "stable" .


###  http://data.europa.eu/949/hasOtherTrainProtection
:hasOtherTrainProtection rdf:type owl:DatatypeProperty ,
                                  owl:FunctionalProperty ;
                         rdfs:domain :Track ;
                         rdfs:range xsd:boolean ;
                         :rinfIndex "1.1.1.3.5.1" ;
                         <http://purl.org/dc/terms/created> "2021-08-09"^^xsd:date ;
                         <http://purl.org/dc/terms/modified> "2021-09-12"^^xsd:date ;
                         rdfs:comment "Indication if other train protection, control and warning systems in normal operation are installed lineside."@en ;
                         rdfs:isDefinedBy <http://data.europa.eu/949/> ;
                         rdfs:label "Existence of other train protection, control and warning systems installed"@en ;
                         <http://www.w3.org/2003/06/sw-vocab-status/ns#term_status> "unstable" .


###  http://data.europa.eu/949/hasParkingBrake
:hasParkingBrake rdf:type owl:DatatypeProperty ,
                          owl:FunctionalProperty ;
                 rdfs:domain :VehicleType ;
                 rdfs:range xsd:boolean ;
                 :eratvIndex "4.7.3.4" ;
                 <http://purl.org/dc/terms/created> "2021-08-26"^^xsd:date ;
                 <http://purl.org/dc/terms/modified> "2021-08-26"^^xsd:date ;
                 rdfs:comment "Indicates if a vehicle type has parking brake."@en ;
                 rdfs:isDefinedBy <http://data.europa.eu/949/> ;
                 rdfs:label "has parking brake"@en ;
                 <http://www.w3.org/2003/06/sw-vocab-status/ns#term_status> "stable" .


###  http://data.europa.eu/949/hasRefuelling
:hasRefuelling rdf:type owl:DatatypeProperty ,
                        owl:FunctionalProperty ;
               rdfs:domain :Siding ;
               rdfs:range xsd:boolean ;
               :isCoreParameter "true"^^xsd:boolean ;
               :rinfIndex "1.2.2.0.4.4" ;
               <http://purl.org/dc/terms/created> "2021-08-10"^^xsd:date ;
               <http://purl.org/dc/terms/modified> "2021-08-10"^^xsd:date ;
               rdfs:comment "Indication whether exists an installation for refuelling (fixed installation for servicing trains) as defined in INF TSIs."@en ;
               rdfs:isDefinedBy <http://data.europa.eu/949/> ;
               rdfs:label "Existence of refuelling"@en ;
               <http://www.w3.org/2003/06/sw-vocab-status/ns#term_status> "stable" .


###  http://data.europa.eu/949/hasRegenerativeBrake
:hasRegenerativeBrake rdf:type owl:DatatypeProperty ,
                               owl:FunctionalProperty ;
                      rdfs:domain :VehicleType ;
                      rdfs:range xsd:boolean ;
                      :eratvIndex "4.7.4.3.1" ;
                      <http://purl.org/dc/terms/created> "2020-08-24"^^xsd:date ;
                      <http://purl.org/dc/terms/modified> "2021-08-06"^^xsd:date ;
                      rdfs:comment "Indication whether regenerative braking is permitted or not."@en ;
                      rdfs:isDefinedBy <http://data.europa.eu/949/> ;
                      rdfs:label "Permission for regenerative braking"@en ;
                      <http://www.w3.org/2003/06/sw-vocab-status/ns#term_status> "stable" .


###  http://data.europa.eu/949/hasSandRestocking
:hasSandRestocking rdf:type owl:DatatypeProperty ,
                            owl:FunctionalProperty ;
                   rdfs:domain :Siding ;
                   rdfs:range xsd:boolean ;
                   :isCoreParameter "true"^^xsd:boolean ;
                   :rinfIndex "1.2.2.0.4.5" ;
                   <http://purl.org/dc/terms/created> "2021-08-10"^^xsd:date ;
                   <http://purl.org/dc/terms/modified> "2021-08-10"^^xsd:date ;
                   rdfs:comment "Indication whether an installation for sand restocking exists (fixed installation for servicing trains)."@en ;
                   rdfs:isDefinedBy <http://data.europa.eu/949/> ;
                   rdfs:label "Existence of sand restocking"@en ;
                   <http://www.w3.org/2003/06/sw-vocab-status/ns#term_status> "stable" .


###  http://data.europa.eu/949/hasSandingPrevention
:hasSandingPrevention rdf:type owl:DatatypeProperty ;
                      rdfs:domain :VehicleType ;
                      rdfs:range xsd:boolean ;
                      :eratvIndex "4.14.2.12" ;
                      <http://purl.org/dc/terms/created> "2021-09-01"^^xsd:date ;
                      <http://purl.org/dc/terms/modified> "2021-09-01"^^xsd:date ;
                      rdfs:comment "Possibility of preventing the use of sanding."@en ;
                      rdfs:isDefinedBy <http://data.europa.eu/949/> ;
                      rdfs:label "has sanding prevention"@en ;
                      <http://www.w3.org/2003/06/sw-vocab-status/ns#term_status> "stable" .


###  http://data.europa.eu/949/hasSevereWeatherConditions
:hasSevereWeatherConditions rdf:type owl:DatatypeProperty ,
                                     owl:FunctionalProperty ;
                            rdfs:domain :Track ;
                            rdfs:range xsd:boolean ;
                            :isCoreParameter "true"^^xsd:boolean ;
                            :rinfIndex "1.1.1.1.2.8" ;
                            <http://purl.org/dc/terms/created> "2020-08-24"^^xsd:date ;
                            <http://purl.org/dc/terms/modified> "2021-09-10"^^xsd:date ;
                            rdfs:comment "Climatic conditions on the line are severe according to European standard."@en ;
                            rdfs:isDefinedBy <http://data.europa.eu/949/> ;
                            rdfs:label "Existence of severe climatic conditions"@en ;
                            <http://www.w3.org/2003/06/sw-vocab-status/ns#term_status> "stable" .


###  http://data.europa.eu/949/hasShuntingRestrictions
:hasShuntingRestrictions rdf:type owl:DatatypeProperty ,
                                  owl:FunctionalProperty ;
                         rdfs:domain :VehicleType ;
                         rdfs:range xsd:boolean ;
                         :eratvIndex "4.8.3" ;
                         <http://purl.org/dc/terms/created> "2021-08-31"^^xsd:date ;
                         <http://purl.org/dc/terms/modified> "2021-08-31"^^xsd:date ;
                         rdfs:comment "Indicates the presence of shunting restrictions."@en ;
                         rdfs:isDefinedBy <http://data.europa.eu/949/> ;
                         rdfs:label "has shunting restrictions"@en ;
                         <http://www.w3.org/2003/06/sw-vocab-status/ns#term_status> "stable" .


###  http://data.europa.eu/949/hasSystemSeparation
:hasSystemSeparation rdf:type owl:DatatypeProperty ,
                              owl:FunctionalProperty ;
                     rdfs:domain :Track ;
                     rdfs:range xsd:boolean ;
                     :rinfIndex "1.1.1.2.4.2.1" ;
                     <http://purl.org/dc/terms/created> "2021-08-08"^^xsd:date ;
                     <http://purl.org/dc/terms/modified> "2021-09-12"^^xsd:date ;
                     rdfs:comment "Indication of existence of system separation."@en ;
                     rdfs:isDefinedBy <http://data.europa.eu/949/> ;
                     rdfs:label "System separation"@en ;
                     <http://www.w3.org/2003/06/sw-vocab-status/ns#term_status> "stable" .


###  http://data.europa.eu/949/hasTSITrainDetection
:hasTSITrainDetection rdf:type owl:DatatypeProperty ;
                      rdfs:domain :Track ;
                      rdfs:range xsd:boolean ;
                      :isCoreParameter "true"^^xsd:boolean ;
                      :rinfIndex "1.1.1.3.4.1" ;
                      <http://purl.org/dc/terms/created> "2021-08-09"^^xsd:date ;
                      <http://purl.org/dc/terms/modified> "2021-09-12"^^xsd:date ;
                      rdfs:comment "Indication if there is any train detection system installed and fully compliant with the CCS TSI requirements."@en ;
                      rdfs:isDefinedBy <http://data.europa.eu/949/> ;
                      rdfs:label "Existence of train detection system fully compliant with the TSI"@en ;
                      <http://www.w3.org/2003/06/sw-vocab-status/ns#term_status> "stable" .


###  http://data.europa.eu/949/hasToiletDischarge
:hasToiletDischarge rdf:type owl:DatatypeProperty ,
                             owl:FunctionalProperty ;
                    rdfs:domain :Siding ;
                    rdfs:range xsd:boolean ;
                    :isCoreParameter "true"^^xsd:boolean ;
                    :rinfIndex "1.2.2.0.4.1" ;
                    <http://purl.org/dc/terms/created> "2021-08-10"^^xsd:date ;
                    <http://purl.org/dc/terms/modified> "2021-08-10"^^xsd:date ;
                    rdfs:comment "Indication whether exists an installation for toilet discharge (fixed installation for servicing trains) as defined in INF TSIs."@en ;
                    rdfs:isDefinedBy <http://data.europa.eu/949/> ;
                    rdfs:label "Existence of toilet discharge"@en ;
                    <http://www.w3.org/2003/06/sw-vocab-status/ns#term_status> "stable" .


###  http://data.europa.eu/949/hasTrainIntegrityConfirmation
:hasTrainIntegrityConfirmation rdf:type owl:DatatypeProperty ,
                                        owl:FunctionalProperty ;
                               rdfs:domain :VehicleType ;
                               rdfs:range xsd:boolean ;
                               :eratvIndex "4.13.1.9" ;
                               <http://purl.org/dc/terms/created> "2020-08-31"^^xsd:date ;
                               <http://purl.org/dc/terms/modified> "2021-09-12"^^xsd:date ;
                               rdfs:comment "Indication of on-board management system about completeness of the train information."@en ;
                               rdfs:isDefinedBy <http://data.europa.eu/949/> ;
                               rdfs:label "has train integrity confirmation"@en ;
                               <http://www.w3.org/2003/06/sw-vocab-status/ns#term_status> "stable" .


###  http://data.europa.eu/949/hasWaterRestocking
:hasWaterRestocking rdf:type owl:DatatypeProperty ,
                             owl:FunctionalProperty ;
                    rdfs:domain :Siding ;
                    rdfs:range xsd:boolean ;
                    :isCoreParameter "true"^^xsd:boolean ;
                    :rinfIndex "1.2.2.0.4.3" ;
                    <http://purl.org/dc/terms/created> "2021-08-10"^^xsd:date ;
                    <http://purl.org/dc/terms/modified> "2021-08-10"^^xsd:date ;
                    rdfs:comment "Indication whether exists an installation for water restocking (fixed installation for servicing trains) as defined in INF TSIs."@en ;
                    rdfs:isDefinedBy <http://data.europa.eu/949/> ;
                    rdfs:label "Existence of water restocking"@en ;
                    <http://www.w3.org/2003/06/sw-vocab-status/ns#term_status> "stable" .


###  http://data.europa.eu/949/hasWheelSlideProtectionSystem
:hasWheelSlideProtectionSystem rdf:type owl:DatatypeProperty ,
                                        owl:FunctionalProperty ;
                               rdfs:domain :VehicleType ;
                               rdfs:range xsd:boolean ;
                               :eratvIndex "4.7.8" ;
                               <http://purl.org/dc/terms/created> "2021-08-31"^^xsd:date ;
                               <http://purl.org/dc/terms/modified> "2021-08-31"^^xsd:date ;
                               rdfs:comment "Indicates the presence of a wheel slide protection system."@en ;
                               rdfs:isDefinedBy <http://data.europa.eu/949/> ;
                               rdfs:label "has wheel slide protection system"@en ;
                               <http://www.w3.org/2003/06/sw-vocab-status/ns#term_status> "stable" .


###  http://data.europa.eu/949/highSpeedLoadModelCompliance
:highSpeedLoadModelCompliance rdf:type owl:DatatypeProperty ,
                                       owl:FunctionalProperty ;
                              rdfs:domain :Track ;
                              rdfs:range xsd:boolean ;
                              :rinfIndex "1.1.1.1.2.4.2" ;
                              <http://purl.org/dc/terms/created> "2020-08-24"^^xsd:date ;
                              <http://purl.org/dc/terms/modified> "2021-09-10"^^xsd:date ;
                              rdfs:comment "Compliance of structures with the High Speed Load Model (HSLM)."@en ;
                              rdfs:isDefinedBy <http://data.europa.eu/949/> ;
                              rdfs:label "Compliance of structures with the High Speed Load Model (HSLM) dynamic load model"@en ;
                              <http://www.w3.org/2003/06/sw-vocab-status/ns#term_status> "stable" .


###  http://data.europa.eu/949/hotAxleBoxDetectorGeneration
:hotAxleBoxDetectorGeneration rdf:type owl:DatatypeProperty ,
                                       owl:FunctionalProperty ;
                              rdfs:domain :Track ;
                              rdfs:range xsd:string ;
                              :rinfIndex "1.1.1.1.7.7" ;
                              <http://purl.org/dc/terms/created> "2020-08-24"^^xsd:date ;
                              <http://purl.org/dc/terms/modified> "2021-09-11"^^xsd:date ;
                              rdfs:comment "Generation of trackside HABD. Specific for the French Italian and Swedish networks."@en ;
                              rdfs:isDefinedBy <http://data.europa.eu/949/> ;
                              rdfs:label "Generation of trackside HABD"@en ;
                              <http://www.w3.org/2003/06/sw-vocab-status/ns#term_status> "stable" .


###  http://data.europa.eu/949/hotAxleBoxDetectorIdentification
:hotAxleBoxDetectorIdentification rdf:type owl:DatatypeProperty ,
                                           owl:FunctionalProperty ;
                                  rdfs:domain :Track ;
                                  rdfs:range xsd:string ;
                                  :rinfIndex "1.1.1.1.7.6" ;
                                  <http://purl.org/dc/terms/created> "2020-08-24"^^xsd:date ;
                                  <http://purl.org/dc/terms/modified> "2021-09-11"^^xsd:date ;
                                  rdfs:comment "Identification of trackside HABD. Applicable if trackside HABD is not TSI compliant."@en ;
                                  rdfs:isDefinedBy <http://data.europa.eu/949/> ;
                                  rdfs:label "Identification of trackside HABD"@en ;
                                  <http://www.w3.org/2003/06/sw-vocab-status/ns#term_status> "stable" .


###  http://data.europa.eu/949/hotAxleBoxDetectorLocation
:hotAxleBoxDetectorLocation rdf:type owl:DatatypeProperty ;
                            rdfs:domain :Track ;
                            rdfs:range xsd:double ;
                            :rinfIndex "1.1.1.1.7.8" ;
                            <http://purl.org/dc/terms/created> "2020-08-24"^^xsd:date ;
                            <http://purl.org/dc/terms/modified> "2021-09-11"^^xsd:date ;
                            rdfs:comment "Railway location of trackside HABD. Applicable if trackside HABD is not TSI compliant."@en ;
                            rdfs:isDefinedBy <http://data.europa.eu/949/> ;
                            rdfs:label "Railway location of trackside HABD"@en ;
                            <http://www.w3.org/2003/06/sw-vocab-status/ns#term_status> "stable" .


###  http://data.europa.eu/949/hotAxleBoxDetectorTSICompliant
:hotAxleBoxDetectorTSICompliant rdf:type owl:DatatypeProperty ,
                                         owl:FunctionalProperty ;
                                rdfs:domain :Track ;
                                rdfs:range xsd:boolean ;
                                :rinfIndex "1.1.1.1.7.5" ;
                                <http://purl.org/dc/terms/created> "2020-08-24"^^xsd:date ;
                                <http://purl.org/dc/terms/modified> "2021-09-11"^^xsd:date ;
                                rdfs:comment "Trackside HABD TSI compliant. Specific for the French, Italian and Swedish networks."@en ;
                                rdfs:isDefinedBy <http://data.europa.eu/949/> ;
                                rdfs:label "Trackside HABD TSI compliant"@en ;
                                <http://www.w3.org/2003/06/sw-vocab-status/ns#term_status> "stable" .


###  http://data.europa.eu/949/imCode
:imCode rdf:type owl:DatatypeProperty ;
        rdfs:subPropertyOf <http://purl.org/dc/terms/identifier> ;
        rdf:type owl:FunctionalProperty ;
        rdfs:domain :InfrastructureManager ;
        rdfs:range xsd:string ;
        :isCoreParameter "true"^^xsd:boolean ;
        :rinfIndex "1.1.0.0.0.1" ,
                   "1.1.1.1.8.1" ,
                   "1.2.1.0.0.1" ,
                   "1.2.1.0.5.1" ,
                   "1.2.1.0.6.1" ,
                   "1.2.2.0.0.1" ,
                   "1.2.2.0.5.1" ;
        <http://purl.org/dc/terms/created> "2021-08-02"^^xsd:date ;
        <http://purl.org/dc/terms/modified> "2022-07-07"^^xsd:date ;
        rdfs:comment "Infrastructure Manager means any body or undertaking that is responsible in particular for establishing and maintaining railway infrastructure or a part thereof. The Code is a unique identifier for the Infrastructure Manager and it shall be verified on national level."@en ;
        rdfs:isDefinedBy <http://data.europa.eu/949/> ;
        rdfs:label "IM's code"@en ;
        <http://www.w3.org/2003/06/sw-vocab-status/ns#term_status> "stable" .


###  http://data.europa.eu/949/isQuietRoute
:isQuietRoute rdf:type owl:DatatypeProperty ,
                       owl:FunctionalProperty ;
              rdfs:domain :Track ;
              rdfs:range xsd:boolean ;
              :isCoreParameter "true"^^xsd:boolean ;
              :rinfIndex "1.1.1.1.7.11" ;
              <http://purl.org/dc/terms/created> "2020-11-04"^^xsd:date ;
              <http://purl.org/dc/terms/modified> "2021-09-12"^^xsd:date ;
              rdfs:comment "Indication of a track being part of a route with noise restrictions"@en ;
              rdfs:isDefinedBy <http://data.europa.eu/949/> ;
              rdfs:label "Belonging to a quieter route"@en ;
              <http://www.w3.org/2003/06/sw-vocab-status/ns#term_status> "stable" .


###  http://data.europa.eu/949/isSwitchable
:isSwitchable rdf:type owl:DatatypeProperty ;
              rdfs:domain :Signal ;
              rdfs:range xsd:boolean ;
              <http://purl.org/dc/terms/created> "2021-04-01"^^xsd:date ;
              <http://purl.org/dc/terms/modified> "2021-04-01"^^xsd:date ;
              rdfs:comment "Indicates if a signal can be switched to show different messages or if it is a static panel."@en ;
              rdfs:isDefinedBy <http://data.europa.eu/949/> ;
              rdfs:label "is switchable"@en ;
              <http://www.w3.org/2003/06/sw-vocab-status/ns#term_status> "stable" .


###  http://data.europa.eu/949/kilometer
:kilometer rdf:type owl:DatatypeProperty ;
           rdfs:domain [ rdf:type owl:Class ;
                         owl:unionOf ( :LineReference
                                       :SpotLocation
                                     )
                       ] ;
           rdfs:range xsd:double ;
           <http://purl.org/dc/terms/created> "2021-01-29"^^xsd:date ;
           <http://purl.org/dc/terms/modified> "2021-01-29"^^xsd:date ;
           rdfs:comment "Distance measured in kilometers from the origin of a national railway line."@en ;
           rdfs:isDefinedBy <http://data.europa.eu/949/> ;
           rdfs:label "kilometer"@en ;
           <http://www.w3.org/2003/06/sw-vocab-status/ns#term_status> "stable" .


###  http://data.europa.eu/949/length
:length rdf:type owl:DatatypeProperty ,
                 owl:FunctionalProperty ;
        rdfs:domain :EraFeature ;
        rdfs:range xsd:double ;
        :eratvIndex "4.8.1" ;
        :isCoreParameter "true"^^xsd:boolean ;
        :rinfIndex "1.1.0.0.0.5" ,
                   "1.1.1.1.8.7" ,
                   "1.2.1.0.5.5" ,
                   "1.2.1.0.6.4" ,
                   "1.2.2.0.2.1" ,
                   "1.2.2.0.5.5" ;
        <http://purl.org/dc/terms/created> "2021-04-01"^^xsd:date ;
        <http://purl.org/dc/terms/modified> "2021-08-11"^^xsd:date ;
        rdfs:comment "Length of a physical object, which can be a section of line, a tunnel, a platform, etc."@en ;
        rdfs:isDefinedBy <http://data.europa.eu/949/> ;
        rdfs:label "Length (of Section of Line, of Tunnel, of Siding, Usable lenght of Platform)"@en ;
        <http://www.w3.org/2003/06/sw-vocab-status/ns#term_status> "stable" .


###  http://data.europa.eu/949/letterMarking
:letterMarking rdf:type owl:DatatypeProperty ;
               rdfs:domain :VehicleType ;
               rdfs:range xsd:string ;
               :eratvIndex "4.1.7" ;
               <http://purl.org/dc/terms/created> "2021-08-25"^^xsd:date ;
               <http://purl.org/dc/terms/modified> "2021-08-25"^^xsd:date ;
               rdfs:comment "letter marking"@en ;
               rdfs:isDefinedBy <http://data.europa.eu/949/> ;
               rdfs:label "letter marking"@en ;
               <http://www.w3.org/2003/06/sw-vocab-status/ns#term_status> "stable" .


###  http://data.europa.eu/949/linearCoordinate
:linearCoordinate rdf:type owl:DatatypeProperty ;
                  rdfs:range xsd:double ;
                  <http://purl.org/dc/terms/created> "2021-04-01"^^xsd:date ;
                  <http://purl.org/dc/terms/modified> "2021-04-01"^^xsd:date ;
                  rdfs:comment "Indicates the position of an object within a linear positioning system. For example, relative to a national railway line."@en ;
                  rdfs:isDefinedBy <http://data.europa.eu/949/> ;
                  rdfs:label "linear coordinate"@en ;
                  <http://www.w3.org/2003/06/sw-vocab-status/ns#term_status> "stable" .


###  http://data.europa.eu/949/loadingPlatformHeight
:loadingPlatformHeight rdf:type owl:DatatypeProperty ;
                       rdfs:domain :VehicleType ;
                       rdfs:range xsd:integer ;
                       :eratvIndex "4.8.7" ;
                       <http://purl.org/dc/terms/created> "2021-08-31"^^xsd:date ;
                       <http://purl.org/dc/terms/modified> "2021-08-31"^^xsd:date ;
                       rdfs:comment "Height of loading platform (for flat wagons and combined transport), given in mm."@en ;
                       rdfs:isDefinedBy <http://data.europa.eu/949/> ;
                       rdfs:label "loading platform height"@en ;
                       <http://www.w3.org/2003/06/sw-vocab-status/ns#term_status> "stable" .


###  http://data.europa.eu/949/localRulesOrRestrictions
:localRulesOrRestrictions rdf:type owl:DatatypeProperty ;
                          rdfs:domain [ rdf:type owl:Class ;
                                        owl:unionOf ( :OperationalPoint
                                                      :Track
                                                    )
                                      ] ;
                          rdfs:range xsd:boolean ;
                          :rinfIndex "1.1.1.4.1" ,
                                     "1.2.3.1" ;
                          <http://purl.org/dc/terms/created> "2021-08-09"^^xsd:date ;
                          <http://purl.org/dc/terms/modified> "2021-09-12"^^xsd:date ;
                          rdfs:comment "Existence of rules and restrictions of a strictly local nature."@en ;
                          rdfs:isDefinedBy <http://data.europa.eu/949/> ;
                          rdfs:label "Existence of rules and restrictions of a strictly local nature"@en ;
                          <http://www.w3.org/2003/06/sw-vocab-status/ns#term_status> "stable" .


###  http://data.europa.eu/949/localRulesOrRestrictionsDoc
:localRulesOrRestrictionsDoc rdf:type owl:DatatypeProperty ;
                             rdfs:domain [ rdf:type owl:Class ;
                                           owl:unionOf ( :OperationalPoint
                                                         :Track
                                                       )
                                         ] ;
                             rdfs:range xsd:string ;
                             :rinfIndex "1.1.1.4.2" ,
                                        "1.2.3.2" ;
                             <http://purl.org/dc/terms/created> "2021-08-09"^^xsd:date ;
                             <http://purl.org/dc/terms/modified> "2021-09-12"^^xsd:date ;
                             rdfs:comment "Documents regarding the rules or restrictions of a strictly local nature available by the IM."@en ;
                             rdfs:isDefinedBy <http://data.europa.eu/949/> ;
                             rdfs:label "Reference of the documents regarding the rules or restrictions of a strictly local nature available by the IM"@en ;
                             <http://www.w3.org/2003/06/sw-vocab-status/ns#term_status> "stable" .


###  http://data.europa.eu/949/magneticBrakePrevention
:magneticBrakePrevention rdf:type owl:DatatypeProperty ,
                                  owl:FunctionalProperty ;
                         rdfs:domain :VehicleType ;
                         rdfs:range xsd:boolean ;
                         :eratvIndex "4.7.4.2.2" ;
                         <http://purl.org/dc/terms/created> "2020-08-24"^^xsd:date ;
                         <http://purl.org/dc/terms/modified> "2021-04-13"^^xsd:date ;
                         rdfs:comment "Possibility of preventing the use of the magnetic track brake (only if fitted with magnetic brake)"@en ;
                         rdfs:isDefinedBy <http://data.europa.eu/949/> ;
                         rdfs:label "magnetic brake prevention"@en ;
                         <http://www.w3.org/2003/06/sw-vocab-status/ns#term_status> "stable" .


###  http://data.europa.eu/949/magneticBrakingConditionsDocument
:magneticBrakingConditionsDocument rdf:type owl:DatatypeProperty ;
                                   rdfs:domain :Track ;
                                   rdfs:range xsd:string ;
                                   :rinfIndex "1.1.1.1.6.5" ;
                                   <http://purl.org/dc/terms/created> "2020-08-24"^^xsd:date ;
                                   <http://purl.org/dc/terms/modified> "2021-09-11"^^xsd:date ;
                                   rdfs:comment "Document with the conditions for the use of magnetic brakes."@en ;
                                   rdfs:isDefinedBy <http://data.europa.eu/949/> ;
                                   rdfs:label "Document with the conditions for the use of magnetic brakes"@en ;
                                   <http://www.w3.org/2003/06/sw-vocab-status/ns#term_status> "stable" .


###  http://data.europa.eu/949/magneticBrakingFitted
:magneticBrakingFitted rdf:type owl:DatatypeProperty ;
                       rdfs:domain :VehicleType ;
                       rdfs:range xsd:boolean ;
                       :eratvIndex "4.7.4.2.1" ;
                       :isCoreParameter "true"^^xsd:boolean ;
                       <http://purl.org/dc/terms/created> "2022-09-12"^^xsd:date ;
                       rdfs:comment "Magnetic track brake fitted. New property defined to distinguish it from magneticBraking which is a RINF SKOS property."@en ;
                       rdfs:isDefinedBy "http://data.europa.eu/949/"^^xsd:anyURI ;
                       rdfs:label "magnetic braking fitted"@en .


###  http://data.europa.eu/949/massPerWheel
:massPerWheel rdf:type owl:DatatypeProperty ,
                       owl:FunctionalProperty ;
              rdfs:domain :VehicleType ;
              rdfs:range xsd:integer ;
              :eratvIndex "4.5.6" ;
              <http://purl.org/dc/terms/created> "2021-08-26"^^xsd:date ;
              <http://purl.org/dc/terms/modified> "2021-08-26"^^xsd:date ;
              rdfs:comment "Mass per wheel, given in kg."@en ;
              rdfs:isDefinedBy <http://data.europa.eu/949/> ;
              rdfs:label "mass per wheel"@en ;
              <http://www.w3.org/2003/06/sw-vocab-status/ns#term_status> "stable" .


###  http://data.europa.eu/949/maxCurrentStandstillPantograph
:maxCurrentStandstillPantograph rdf:type owl:DatatypeProperty ,
                                         owl:FunctionalProperty ;
                                rdfs:domain [ rdf:type owl:Class ;
                                              owl:unionOf ( :ContactLineSystem
                                                            :Siding
                                                            :VehicleType
                                                          )
                                            ] ;
                                rdfs:range xsd:double ;
                                :eratvIndex "4.10.4" ;
                                :rinfIndex "1.1.1.2.2.3" ,
                                           "1.2.2.0.6.1" ;
                                <http://purl.org/dc/terms/created> "2020-08-25"^^xsd:date ;
                                <http://purl.org/dc/terms/modified> "2021-09-12"^^xsd:date ;
                                rdfs:comment "Indication of the maximum allowable train current at standstill for DC systems expressed in amperes."@en ;
                                rdfs:isDefinedBy <http://data.europa.eu/949/> ;
                                rdfs:label "Maximum current at standstill per pantograph"@en ;
                                <http://www.w3.org/2003/06/sw-vocab-status/ns#term_status> "stable" .


###  http://data.europa.eu/949/maxDistConsecutiveAxles
:maxDistConsecutiveAxles rdf:type owl:DatatypeProperty ;
                         rdfs:domain [ rdf:type owl:Class ;
                                       owl:unionOf ( :TrainDetectionSystem
                                                     :VehicleType
                                                   )
                                     ] ;
                         rdfs:range xsd:integer ;
                         :eratvIndex "4.14.2.1" ;
                         :rinfIndex "1.1.1.3.7.2.2" ;
                         <http://purl.org/dc/terms/created> "2021-08-08"^^xsd:date ;
                         <http://purl.org/dc/terms/modified> "2021-09-01"^^xsd:date ;
                         rdfs:comment "Indication of maximum permitted distance between two consecutive axles in case of TSI non-compliance, given in millimetres."@en ;
                         rdfs:isDefinedBy <http://data.europa.eu/949/> ;
                         rdfs:label "Maximum permitted distance between two consecutive axles in case of TSI non-compliance"@en ;
                         <http://www.w3.org/2003/06/sw-vocab-status/ns#term_status> "stable" .


###  http://data.europa.eu/949/maxDistEndTrainFirstAxle
:maxDistEndTrainFirstAxle rdf:type owl:DatatypeProperty ;
                          rdfs:domain :TrainDetectionSystem ;
                          rdfs:range xsd:integer ;
                          :rinfIndex "1.1.1.3.7.5" ;
                          <http://purl.org/dc/terms/created> "2021-08-08"^^xsd:date ;
                          <http://purl.org/dc/terms/modified> "2021-08-08"^^xsd:date ;
                          rdfs:comment "Indication of maximum distance between end of train and first axle, given in millimetres, applicable for both sides (front and rear) of a vehicle or train."@en ;
                          rdfs:isDefinedBy <http://data.europa.eu/949/> ;
                          rdfs:label "Maximum distance between end of train and first axle"@en ;
                          <http://www.w3.org/2003/06/sw-vocab-status/ns#term_status> "stable" .


###  http://data.europa.eu/949/maxFlangeHeight
:maxFlangeHeight rdf:type owl:DatatypeProperty ;
                 rdfs:domain [ rdf:type owl:Class ;
                               owl:unionOf ( :TrainDetectionSystem
                                             :VehicleType
                                           )
                             ] ;
                 rdfs:range xsd:double ;
                 :eratvIndex "4.14.2.9" ;
                 :rinfIndex "1.1.1.3.7.10" ;
                 <http://purl.org/dc/terms/created> "2021-08-08"^^xsd:date ;
                 <http://purl.org/dc/terms/modified> "2021-09-01"^^xsd:date ;
                 rdfs:comment "Maximum permitted flange height, given in millimiters."@en ;
                 rdfs:isDefinedBy <http://data.europa.eu/949/> ;
                 rdfs:label "Maximum permitted height of the flange"@en ;
                 <http://www.w3.org/2003/06/sw-vocab-status/ns#term_status> "stable" .


###  http://data.europa.eu/949/maxImpedanceWheelset
:maxImpedanceWheelset rdf:type owl:DatatypeProperty ;
                      rdfs:domain [ rdf:type owl:Class ;
                                    owl:unionOf ( :TrainDetectionSystem
                                                  :VehicleType
                                                )
                                  ] ;
                      rdfs:range xsd:double ;
                      :eratvIndex "4.14.2.16" ;
                      :rinfIndex "1.1.1.3.7.15.2" ;
                      <http://purl.org/dc/terms/created> "2021-08-08"^^xsd:date ;
                      <http://purl.org/dc/terms/modified> "2021-08-08"^^xsd:date ;
                      rdfs:comment "The value of maximum permitted impedance given in ohm in case of TSI non-compliance."@en ;
                      rdfs:isDefinedBy <http://data.europa.eu/949/> ;
                      rdfs:label "Maximum permitted impedance between opposite wheels of a wheelset when not TSI compliant"@en ;
                      <http://www.w3.org/2003/06/sw-vocab-status/ns#term_status> "stable" .


###  http://data.europa.eu/949/maxLengthVehicleNose
:maxLengthVehicleNose rdf:type owl:DatatypeProperty ;
                      rdfs:domain :VehicleType ;
                      rdfs:range xsd:integer ;
                      :eratvIndex "4.14.2.4" ;
                      <http://purl.org/dc/terms/created> "2021-09-01"^^xsd:date ;
                      <http://purl.org/dc/terms/modified> "2021-09-01"^^xsd:date ;
                      rdfs:comment "Maximum length of the vehicle nose."@en ;
                      rdfs:isDefinedBy <http://data.europa.eu/949/> ;
                      rdfs:label "maximum length vehicle nose"@en ;
                      <http://www.w3.org/2003/06/sw-vocab-status/ns#term_status> "stable" .


###  http://data.europa.eu/949/maxSpeed
:maxSpeed rdf:type owl:DatatypeProperty ;
          rdfs:domain :SpeedSection ;
          rdfs:range xsd:double ;
          rdfs:isDefinedBy <http://data.europa.eu/949/> ;
          rdfs:label "maximum permissible speed"@en .


###  http://data.europa.eu/949/maxTrainCurrent
:maxTrainCurrent rdf:type owl:DatatypeProperty ;
                 rdfs:domain :ContactLineSystem ;
                 rdfs:range xsd:integer ;
                 :rinfIndex "1.1.1.2.2.2" ;
                 <http://purl.org/dc/terms/created> "2021-08-06"^^xsd:date ;
                 <http://purl.org/dc/terms/modified> "2021-08-06"^^xsd:date ;
                 <http://purl.org/dc/terms/source> "https://wiki2.railml.org/wiki/IS:maxTrainCurrent_electrification"^^xsd:anyURI ;
                 rdfs:comment "Maximum current taken by the complete train (composition of one or more units) expressed in amperes."@en ;
                 rdfs:isDefinedBy <http://data.europa.eu/949/> ;
                 rdfs:label "Maximum train current"@en ;
                 <http://www.w3.org/2003/06/sw-vocab-status/ns#term_status> "stable" .


###  http://data.europa.eu/949/maximumAltitude
:maximumAltitude rdf:type owl:DatatypeProperty ,
                          owl:FunctionalProperty ;
                 rdfs:domain :Track ;
                 rdfs:range xsd:double ;
                 :isCoreParameter "true"^^xsd:boolean ;
                 :rinfIndex "1.1.1.1.2.7" ;
                 <http://purl.org/dc/terms/created> "2021-08-03"^^xsd:date ;
                 <http://purl.org/dc/terms/modified> "2022-10-20"^^xsd:date ;
                 rdfs:comment "Highest point of the section of line above sea level in reference to Normal Amsterdamâs Peil (NAP). The value of the parameter shall be given in metres, with tolerance of +/-100m."@en ;
                 rdfs:isDefinedBy <http://data.europa.eu/949/> ;
                 rdfs:label "Maximum altitude"@en ;
                 <http://www.w3.org/2003/06/sw-vocab-status/ns#term_status> "stable" .


###  http://data.europa.eu/949/maximumAverageDeceleration
:maximumAverageDeceleration rdf:type owl:DatatypeProperty ,
                                     owl:FunctionalProperty ;
                            rdfs:domain :VehicleType ;
                            rdfs:range xsd:double ;
                            :eratvIndex "4.7.1" ;
                            <http://purl.org/dc/terms/created> "2021-08-26"^^xsd:date ;
                            <http://purl.org/dc/terms/modified> "2021-08-26"^^xsd:date ;
                            rdfs:comment "Maximum train deceleration given in m/sÂ²."@en ;
                            rdfs:isDefinedBy <http://data.europa.eu/949/> ;
                            rdfs:label "maximum average deceleration"@en ;
                            <http://www.w3.org/2003/06/sw-vocab-status/ns#term_status> "stable" .


###  http://data.europa.eu/949/maximumBrakeThermalEnergyCapacity
:maximumBrakeThermalEnergyCapacity rdf:type owl:DatatypeProperty ,
                                            owl:FunctionalProperty ;
                                   rdfs:domain :VehicleType ;
                                   rdfs:range xsd:integer ;
                                   :eratvIndex "4.7.2.1.6" ;
                                   <http://purl.org/dc/terms/created> "2021-08-26"^^xsd:date ;
                                   <http://purl.org/dc/terms/modified> "2021-08-26"^^xsd:date ;
                                   rdfs:comment "Maximum brake thermal energy capacity given in kJ"@en ;
                                   rdfs:isDefinedBy <http://data.europa.eu/949/> ;
                                   rdfs:label "maximum brake thermal energy capacity"@en ;
                                   <http://www.w3.org/2003/06/sw-vocab-status/ns#term_status> "stable" .


###  http://data.europa.eu/949/maximumBrakingDistance
:maximumBrakingDistance rdf:type owl:DatatypeProperty ,
                                 owl:FunctionalProperty ;
                        rdfs:domain :Track ;
                        rdfs:range xsd:integer ;
                        :isCoreParameter "true"^^xsd:boolean ;
                        :rinfIndex "1.1.1.3.11.1" ;
                        <http://purl.org/dc/terms/created> "2020-08-24"^^xsd:date ;
                        <http://purl.org/dc/terms/modified> "2021-09-12"^^xsd:date ;
                        rdfs:comment "The maximum value of the braking distance [in meters] of a train shall be given for the maximum line speed."@en ;
                        rdfs:isDefinedBy <http://data.europa.eu/949/> ;
                        rdfs:label "Maximum braking distance requested"@en ;
                        <http://www.w3.org/2003/06/sw-vocab-status/ns#term_status> "stable" .


###  http://data.europa.eu/949/maximumContactWireHeight
:maximumContactWireHeight rdf:type owl:DatatypeProperty ,
                                   owl:FunctionalProperty ;
                          rdfs:domain [ rdf:type owl:Class ;
                                        owl:unionOf ( :Track
                                                      :VehicleType
                                                    )
                                      ] ;
                          rdfs:range xsd:double ;
                          :eratvIndex "4.10.5" ;
                          :rinfIndex "1.1.1.2.2.5" ;
                          <http://purl.org/dc/terms/created> "2020-08-25"^^xsd:date ;
                          <http://purl.org/dc/terms/modified> "2021-09-11"^^xsd:date ;
                          rdfs:comment "Indication of the maximum contact wire height expressed in metres."@en ;
                          rdfs:isDefinedBy <http://data.europa.eu/949/> ;
                          rdfs:label "Maximum contact wire height"@en ;
                          <http://www.w3.org/2003/06/sw-vocab-status/ns#term_status> "stable" .


###  http://data.europa.eu/949/maximumDesignSpeed
:maximumDesignSpeed rdf:type owl:DatatypeProperty ,
                             owl:FunctionalProperty ;
                    rdfs:domain :VehicleType ;
                    rdfs:range xsd:integer ;
                    :eratvIndex "4.1.2.1" ;
                    <http://purl.org/dc/terms/created> "2020-08-24"^^xsd:date ;
                    <http://purl.org/dc/terms/modified> "2020-11-03"^^xsd:date ;
                    rdfs:comment "Maximum design speed."@en ;
                    rdfs:isDefinedBy <http://data.europa.eu/949/> ;
                    rdfs:label "maximum design speed"@en ;
                    <http://www.w3.org/2003/06/sw-vocab-status/ns#term_status> "stable" .


###  http://data.europa.eu/949/maximumLocomotivesCoupled
:maximumLocomotivesCoupled rdf:type owl:DatatypeProperty ,
                                    owl:FunctionalProperty ;
                           rdfs:domain :VehicleType ;
                           rdfs:range xsd:integer ;
                           :eratvIndex "4.1.5" ;
                           <http://purl.org/dc/terms/created> "2021-08-25"^^xsd:date ;
                           <http://purl.org/dc/terms/modified> "2021-08-25"^^xsd:date ;
                           rdfs:comment "Maximum number of trainsets or locomotives coupled together in multiple operation."@en ;
                           rdfs:isDefinedBy <http://data.europa.eu/949/> ;
                           rdfs:label "maximum locomotives coupled"@en ;
                           <http://www.w3.org/2003/06/sw-vocab-status/ns#term_status> "stable" .


###  http://data.europa.eu/949/maximumPermittedSpeed
:maximumPermittedSpeed rdf:type owl:DatatypeProperty ,
                                owl:FunctionalProperty ;
                       rdfs:domain :Track ;
                       rdfs:range xsd:integer ;
                       :isCoreParameter "true"^^xsd:boolean ;
                       :rinfIndex "1.1.1.1.2.5" ;
                       <http://purl.org/dc/terms/created> "2020-08-24"^^xsd:date ;
                       <http://purl.org/dc/terms/modified> "2021-09-10"^^xsd:date ;
                       rdfs:comment "Nominal maximum operational speed on the line as a result of INF, ENE and CCS subsystem characteristics expressed in kilometres/hour."@en ;
                       rdfs:isDefinedBy <http://data.europa.eu/949/> ;
                       rdfs:label "Maximum permitted speed"@en ;
                       <http://www.w3.org/2003/06/sw-vocab-status/ns#term_status> "stable" .


###  http://data.europa.eu/949/maximumServiceBrake
:maximumServiceBrake rdf:type owl:DatatypeProperty ,
                              owl:FunctionalProperty ;
                     rdfs:domain :VehicleType ;
                     rdfs:range xsd:string ;
                     :eratvIndex "4.7.7" ;
                     <http://purl.org/dc/terms/created> "2021-08-26"^^xsd:date ;
                     <http://purl.org/dc/terms/modified> "2021-08-26"^^xsd:date ;
                     rdfs:comment "At maximum service brake: Stopping distance, Maximum deceleration, for the load condition 'design mass under normal payload' at the design maximum speed."@en ;
                     rdfs:isDefinedBy <http://data.europa.eu/949/> ;
                     rdfs:label "maximum service break"@en ;
                     <http://www.w3.org/2003/06/sw-vocab-status/ns#term_status> "stable" .


###  http://data.europa.eu/949/maximumSpeedAndCantDeficiency
:maximumSpeedAndCantDeficiency rdf:type owl:DatatypeProperty ,
                                        owl:FunctionalProperty ;
                               rdfs:domain :VehicleType ;
                               rdfs:range xsd:string ;
                               :eratvIndex "4.6.4" ;
                               <http://purl.org/dc/terms/created> "2020-08-24"^^xsd:date ;
                               <http://purl.org/dc/terms/modified> "2021-08-02"^^xsd:date ;
                               rdfs:comment """Combination of maximum speed and maximum cant deficiency for which the vehicle was assessed.

This property was before an object skos property. The values for this property do not come from a list of predefined values. Thus, the original object property was replaced by this datatype property with range xsd:string."""@en ;
                               rdfs:isDefinedBy <http://data.europa.eu/949/> ;
                               rdfs:label "maximum speed and cant deficiency"@en ;
                               <http://www.w3.org/2003/06/sw-vocab-status/ns#term_status> "stable" .


###  http://data.europa.eu/949/maximumSpeedEmpty
:maximumSpeedEmpty rdf:type owl:DatatypeProperty ;
                   rdfs:domain :VehicleType ;
                   rdfs:range xsd:integer ;
                   :eratvIndex "4.1.2.2" ;
                   <http://purl.org/dc/terms/created> "2021-08-24"^^xsd:date ;
                   <http://purl.org/dc/terms/modified> "2021-08-24"^^xsd:date ;
                   rdfs:comment "Maximum speed when empty."@en ;
                   rdfs:isDefinedBy <http://data.europa.eu/949/> ;
                   rdfs:label "maximum speed empty"@en ;
                   <http://www.w3.org/2003/06/sw-vocab-status/ns#term_status> "stable" .


###  http://data.europa.eu/949/maximumTemperature
:maximumTemperature rdf:type owl:DatatypeProperty ;
                    rdfs:domain [ rdf:type owl:Class ;
                                  owl:unionOf ( :Track
                                                :VehicleType
                                              )
                                ] ;
                    rdfs:range xsd:integer ;
                    :eratvIndex "4.3.1" ;
                    :isCoreParameter "true"^^xsd:boolean ;
                    :rinfIndex "1.1.1.1.2.6" ;
                    <http://purl.org/dc/terms/created> "2020-08-24"^^xsd:date ;
                    <http://purl.org/dc/terms/modified> "2021-09-10"^^xsd:date ;
                    rdfs:comment "Maximum tempertaure allowed for unrestricted operation access, according to European standard."@en ;
                    rdfs:isDefinedBy <http://data.europa.eu/949/> ;
                    rdfs:label "Temperature range (maximum)"@en ;
                    <http://www.w3.org/2003/06/sw-vocab-status/ns#term_status> "stable" .


###  http://data.europa.eu/949/maximumTrainDeceleration
:maximumTrainDeceleration rdf:type owl:DatatypeProperty ,
                                   owl:FunctionalProperty ;
                          rdfs:domain :Track ;
                          rdfs:range xsd:double ;
                          :isCoreParameter "true"^^xsd:boolean ;
                          :rinfIndex "1.1.1.1.6.1" ;
                          <http://purl.org/dc/terms/created> "2020-08-24"^^xsd:date ;
                          <http://purl.org/dc/terms/modified> "2021-09-10"^^xsd:date ;
                          rdfs:comment "Limit for longitudinal track resistance given as a maximum allowed train deceleration and expressed in metres per square second."@en ;
                          rdfs:isDefinedBy <http://data.europa.eu/949/> ;
                          rdfs:label "Maximum train deceleration"@en ;
                          <http://www.w3.org/2003/06/sw-vocab-status/ns#term_status> "stable" .


###  http://data.europa.eu/949/meetsRequirementVehicleAuthorisation
:meetsRequirementVehicleAuthorisation rdf:type owl:DatatypeProperty ;
                                      rdfs:domain :VehicleType ;
                                      rdfs:range xsd:string ;
                                      :eratvIndex "4.1.8" ;
                                      <http://purl.org/dc/terms/created> "2021-08-25"^^xsd:date ;
                                      <http://purl.org/dc/terms/modified> "2021-08-25"^^xsd:date ;
                                      rdfs:comment "Type meets the requirements necessary for validity of the vehicle authorisation granted by one Member State in other MSs."@en ;
                                      rdfs:isDefinedBy <http://data.europa.eu/949/> ;
                                      rdfs:label "meets requirement vehicle authorization"@en ;
                                      <http://www.w3.org/2003/06/sw-vocab-status/ns#term_status> "stable" .


###  http://data.europa.eu/949/minAxleLoad
:minAxleLoad rdf:type owl:DatatypeProperty ,
                      owl:FunctionalProperty ;
             rdfs:domain [ rdf:type owl:Class ;
                           owl:unionOf ( :TrainDetectionSystem
                                         :VehicleType
                                       )
                         ] ;
             rdfs:range xsd:double ;
             :eratvIndex "4.14.2.10" ;
             :rinfIndex "1.1.1.3.7.11" ;
             <http://purl.org/dc/terms/created> "2021-08-08"^^xsd:date ;
             <http://purl.org/dc/terms/modified> "2021-08-08"^^xsd:date ;
             rdfs:comment "Minimum permitted axle load, given in tons."@en ;
             rdfs:isDefinedBy <http://data.europa.eu/949/> ;
             rdfs:label "Minimum permitted axle load"@en ;
             <http://www.w3.org/2003/06/sw-vocab-status/ns#term_status> "unstable" .


###  http://data.europa.eu/949/minDistConsecutiveAxles
:minDistConsecutiveAxles rdf:type owl:DatatypeProperty ;
                         rdfs:domain :TrainDetectionSystem ;
                         rdfs:range xsd:integer ;
                         :eratvIndex "4.14.2.2" ;
                         :rinfIndex "1.1.1.3.7.3" ;
                         <http://purl.org/dc/terms/created> "2021-08-08"^^xsd:date ;
                         <http://purl.org/dc/terms/modified> "2021-09-01"^^xsd:date ;
                         rdfs:comment "Indication of minimum permitted distance between two consecutive axles, given in millimetres."@en ;
                         rdfs:isDefinedBy <http://data.europa.eu/949/> ;
                         rdfs:label "Minimum permitted distance between two consecutive axles"@en ;
                         <http://www.w3.org/2003/06/sw-vocab-status/ns#term_status> "stable" .


###  http://data.europa.eu/949/minDistFirstLastAxle
:minDistFirstLastAxle rdf:type owl:DatatypeProperty ;
                      rdfs:domain [ rdf:type owl:Class ;
                                    owl:unionOf ( :TrainDetectionSystem
                                                  :VehicleType
                                                )
                                  ] ;
                      rdfs:range xsd:integer ;
                      :eratvIndex "4.14.2.3" ;
                      :rinfIndex "1.1.1.3.7.4" ;
                      <http://purl.org/dc/terms/created> "2021-08-08"^^xsd:date ;
                      <http://purl.org/dc/terms/modified> "2021-08-08"^^xsd:date ;
                      rdfs:comment "Indication of minimum permitted distance between first and last axles, given in millimetres."@en ;
                      rdfs:isDefinedBy <http://data.europa.eu/949/> ;
                      rdfs:label "Minimum permitted distance between first and last axle"@en ;
                      <http://www.w3.org/2003/06/sw-vocab-status/ns#term_status> "stable" .


###  http://data.europa.eu/949/minFlangeHeight
:minFlangeHeight rdf:type owl:DatatypeProperty ;
                 rdfs:domain [ rdf:type owl:Class ;
                               owl:unionOf ( :TrainDetectionSystem
                                             :VehicleType
                                           )
                             ] ;
                 rdfs:range xsd:double ;
                 :eratvIndex "4.14.2.8" ;
                 :rinfIndex "1.1.1.3.7.9" ;
                 <http://purl.org/dc/terms/created> "2021-08-08"^^xsd:date ;
                 <http://purl.org/dc/terms/modified> "2021-09-01"^^xsd:date ;
                 rdfs:comment "Minimum permitted flange height, given in millimiters."@en ;
                 rdfs:isDefinedBy <http://data.europa.eu/949/> ;
                 rdfs:label "Minimum permitted height of the flange"@en ;
                 <http://www.w3.org/2003/06/sw-vocab-status/ns#term_status> "stable" .


###  http://data.europa.eu/949/minFlangeThickness
:minFlangeThickness rdf:type owl:DatatypeProperty ;
                    rdfs:domain [ rdf:type owl:Class ;
                                  owl:unionOf ( :TrainDetectionSystem
                                                :VehicleType
                                              )
                                ] ;
                    rdfs:range xsd:double ;
                    :eratvIndex "4.14.2.7" ;
                    :rinfIndex "1.1.1.3.7.8" ;
                    <http://purl.org/dc/terms/created> "2021-08-08"^^xsd:date ;
                    <http://purl.org/dc/terms/modified> "2021-09-01"^^xsd:date ;
                    rdfs:comment "Minimum permitted flange thickness, given in millimiters."@en ;
                    rdfs:isDefinedBy <http://data.europa.eu/949/> ;
                    rdfs:label "Minimum permitted thickness of the flange"@en ;
                    <http://www.w3.org/2003/06/sw-vocab-status/ns#term_status> "stable" .


###  http://data.europa.eu/949/minRimWidth
:minRimWidth rdf:type owl:DatatypeProperty ;
             rdfs:domain [ rdf:type owl:Class ;
                           owl:unionOf ( :TrainDetectionSystem
                                         :VehicleType
                                       )
                         ] ;
             rdfs:range xsd:double ;
             :eratvIndex "4.14.2.5" ;
             :rinfIndex "1.1.1.3.7.6" ;
             <http://purl.org/dc/terms/created> "2021-08-08"^^xsd:date ;
             <http://purl.org/dc/terms/modified> "2021-09-01"^^xsd:date ;
             rdfs:comment "Minimum permitted width of the rim, given in millimiters."@en ;
             rdfs:isDefinedBy <http://data.europa.eu/949/> ;
             rdfs:label "Minimum permitted width of the rim"@en ;
             <http://www.w3.org/2003/06/sw-vocab-status/ns#term_status> "stable" .


###  http://data.europa.eu/949/minVehicleImpedance
:minVehicleImpedance rdf:type owl:DatatypeProperty ;
                     rdfs:domain :VehicleType ;
                     rdfs:range xsd:string ;
                     :eratvIndex "4.14.2.17" ;
                     <http://purl.org/dc/terms/created> "2021-09-01"^^xsd:date ;
                     <http://purl.org/dc/terms/modified> "2021-09-01"^^xsd:date ;
                     rdfs:comment "Minimum vehicle impedance (between wheels and pantograph) (only for vehicles equipped for 1500V or 3000V DC)."@en ;
                     rdfs:isDefinedBy <http://data.europa.eu/949/> ;
                     rdfs:label "minimum vehicle impedance"@en ;
                     <http://www.w3.org/2003/06/sw-vocab-status/ns#term_status> "stable" .


###  http://data.europa.eu/949/minWheelDiameter
:minWheelDiameter rdf:type owl:DatatypeProperty ;
                  rdfs:domain [ rdf:type owl:Class ;
                                owl:unionOf ( :TrainDetectionSystem
                                              :VehicleType
                                            )
                              ] ;
                  rdfs:range xsd:integer ;
                  :eratvIndex "4.14.2.6" ;
                  :rinfIndex "1.1.1.3.7.7" ;
                  <http://purl.org/dc/terms/created> "2021-08-08"^^xsd:date ;
                  <http://purl.org/dc/terms/modified> "2021-09-01"^^xsd:date ;
                  rdfs:comment "Minimum permitted wheel diameter, given in millimiters."@en ;
                  rdfs:isDefinedBy <http://data.europa.eu/949/> ;
                  rdfs:label "Minimum permitted wheel diameter"@en ;
                  <http://www.w3.org/2003/06/sw-vocab-status/ns#term_status> "stable" .


###  http://data.europa.eu/949/minimumConcaveVerticalRadius
:minimumConcaveVerticalRadius rdf:type owl:DatatypeProperty ,
                                       owl:FunctionalProperty ;
                              rdfs:domain :VehicleType ;
                              rdfs:range xsd:integer ;
                              :eratvIndex "4.8.6" ;
                              <http://purl.org/dc/terms/created> "2020-08-24"^^xsd:date ;
                              <http://purl.org/dc/terms/modified> "2020-11-03"^^xsd:date ;
                              rdfs:comment "Minimum vertical concave curve radius capability."@en ;
                              rdfs:isDefinedBy <http://data.europa.eu/949/> ;
                              rdfs:label "minimum concave vertical radius"@en ;
                              <http://www.w3.org/2003/06/sw-vocab-status/ns#term_status> "stable" .


###  http://data.europa.eu/949/minimumContactWireHeight
:minimumContactWireHeight rdf:type owl:DatatypeProperty ,
                                   owl:FunctionalProperty ;
                          rdfs:domain [ rdf:type owl:Class ;
                                        owl:unionOf ( :Track
                                                      :VehicleType
                                                    )
                                      ] ;
                          rdfs:range xsd:double ;
                          :eratvIndex "4.10.5" ;
                          :rinfIndex "1.1.1.2.2.6" ;
                          <http://purl.org/dc/terms/created> "2020-08-25"^^xsd:date ;
                          <http://purl.org/dc/terms/modified> "2021-09-11"^^xsd:date ;
                          rdfs:comment "Indication of the minimum contact wire height expressed in metres."@en ;
                          rdfs:isDefinedBy <http://data.europa.eu/949/> ;
                          rdfs:label "Minimum contact wire height"@en ;
                          <http://www.w3.org/2003/06/sw-vocab-status/ns#term_status> "stable" .


###  http://data.europa.eu/949/minimumConvexVerticalRadius
:minimumConvexVerticalRadius rdf:type owl:DatatypeProperty ,
                                      owl:FunctionalProperty ;
                             rdfs:domain :VehicleType ;
                             rdfs:range xsd:integer ;
                             :eratvIndex "4.8.5" ;
                             <http://purl.org/dc/terms/created> "2020-08-24"^^xsd:date ;
                             <http://purl.org/dc/terms/modified> "2020-11-03"^^xsd:date ;
                             rdfs:comment "Minimum vertical convex curve radius capability."@en ;
                             rdfs:isDefinedBy <http://data.europa.eu/949/> ;
                             rdfs:label "minimum convex vertical radius"@en ;
                             <http://www.w3.org/2003/06/sw-vocab-status/ns#term_status> "stable" .


###  http://data.europa.eu/949/minimumHorizontalRadius
:minimumHorizontalRadius rdf:type owl:DatatypeProperty ,
                                  owl:FunctionalProperty ;
                         rdfs:domain [ rdf:type owl:Class ;
                                       owl:unionOf ( :Siding
                                                     :Track
                                                     :VehicleType
                                                   )
                                     ] ;
                         rdfs:range xsd:integer ;
                         :eratvIndex "4.8.4" ;
                         :isCoreParameter "true"^^xsd:boolean ;
                         :rinfIndex "1.1.1.1.3.7" ,
                                    "1.2.2.0.3.2" ;
                         <http://purl.org/dc/terms/created> "2020-08-24"^^xsd:date ;
                         <http://purl.org/dc/terms/modified> "2021-09-10"^^xsd:date ;
                         rdfs:comment "Radius of the smallest horizontal curve of the track in metres."@en ;
                         rdfs:isDefinedBy <http://data.europa.eu/949/> ;
                         rdfs:label "Minimum radius of horizontal curve"@en ;
                         <http://www.w3.org/2003/06/sw-vocab-status/ns#term_status> "stable" .


###  http://data.europa.eu/949/minimumTemperature
:minimumTemperature rdf:type owl:DatatypeProperty ;
                    rdfs:domain [ rdf:type owl:Class ;
                                  owl:unionOf ( :Track
                                                :VehicleType
                                              )
                                ] ;
                    rdfs:range xsd:integer ;
                    :eratvIndex "4.3.1" ;
                    :isCoreParameter "true"^^xsd:boolean ;
                    :rinfIndex "1.1.1.1.2.6" ;
                    <http://purl.org/dc/terms/created> "2020-08-24"^^xsd:date ;
                    <http://purl.org/dc/terms/modified> "2021-09-10"^^xsd:date ;
                    rdfs:comment "Minimum tempertaure allowed for unrestricted operation access, according to European standard."@en ;
                    rdfs:isDefinedBy <http://data.europa.eu/949/> ;
                    rdfs:label "Temperature range (minimum)"@en ;
                    <http://www.w3.org/2003/06/sw-vocab-status/ns#term_status> "stable" .


###  http://data.europa.eu/949/minimumVerticalRadius
:minimumVerticalRadius rdf:type owl:DatatypeProperty ,
                                owl:FunctionalProperty ;
                       rdfs:domain :Siding ;
                       rdfs:range xsd:string ;
                       :rinfIndex "1.2.2.0.3.3" ;
                       <http://purl.org/dc/terms/created> "2020-08-24"^^xsd:date ;
                       <http://purl.org/dc/terms/modified> "2021-09-12"^^xsd:date ;
                       rdfs:comment "Radius of the smallest vertical curve expressed in metres."@en ;
                       rdfs:isDefinedBy <http://data.europa.eu/949/> ;
                       rdfs:label "minimum radius of vertical curve"@en ;
                       <http://www.w3.org/2003/06/sw-vocab-status/ns#term_status> "stable" .


###  http://data.europa.eu/949/minimumWheelDiameter
:minimumWheelDiameter rdf:type owl:DatatypeProperty ,
                               owl:FunctionalProperty ;
                      rdfs:domain [ rdf:type owl:Class ;
                                    owl:unionOf ( :Track
                                                  :VehicleType
                                                )
                                  ] ;
                      rdfs:range xsd:integer ;
                      :eratvIndex "4.8.2" ;
                      :isCoreParameter "true"^^xsd:boolean ;
                      :rinfIndex "1.1.1.1.5.2" ;
                      <http://purl.org/dc/terms/created> "2020-08-24"^^xsd:date ;
                      <http://purl.org/dc/terms/modified> "2021-09-10"^^xsd:date ;
                      rdfs:comment "Maximum unguided length of fixed obtuse crossings is based on a minimum wheel diameter in service expressed in millimetres."@en ;
                      rdfs:isDefinedBy <http://data.europa.eu/949/> ;
                      rdfs:label "Minimum wheel diameter for fixed obtuse crossings"@en ;
                      <http://www.w3.org/2003/06/sw-vocab-status/ns#term_status> "stable" .


###  http://data.europa.eu/949/multipleTrainProtectionRequired
:multipleTrainProtectionRequired rdf:type owl:DatatypeProperty ,
                                          owl:FunctionalProperty ;
                                 rdfs:domain :Track ;
                                 rdfs:range xsd:boolean ;
                                 :rinfIndex "1.1.1.3.5.2" ;
                                 <http://purl.org/dc/terms/created> "2021-08-09"^^xsd:date ;
                                 <http://purl.org/dc/terms/modified> "2021-09-12"^^xsd:date ;
                                 rdfs:comment "Indication whether more than one train protection, control and warning system is required to be on-board and active simultaneously."@en ;
                                 rdfs:isDefinedBy <http://data.europa.eu/949/> ;
                                 rdfs:label "Need for more than one train protection, control and warning system required on board"@en ;
                                 <http://www.w3.org/2003/06/sw-vocab-status/ns#term_status> "unstable" .


###  http://data.europa.eu/949/nationalLoadCapability
:nationalLoadCapability rdf:type owl:DatatypeProperty ;
                        rdfs:domain :Track ;
                        rdfs:range xsd:string ;
                        :rinfIndex "1.1.1.1.2.4.1" ;
                        <http://purl.org/dc/terms/created> "2020-08-24"^^xsd:date ;
                        <http://purl.org/dc/terms/modified> "2021-09-10"^^xsd:date ;
                        rdfs:comment "National classification for load capability."@en ;
                        rdfs:isDefinedBy <http://data.europa.eu/949/> ;
                        rdfs:label "National classification for load capability"@en ;
                        <http://www.w3.org/2003/06/sw-vocab-status/ns#term_status> "stable" .


###  http://data.europa.eu/949/nationalRollingStockFireCategory
:nationalRollingStockFireCategory rdf:type owl:DatatypeProperty ,
                                           owl:FunctionalProperty ;
                                  rdfs:domain :Tunnel ;
                                  rdfs:range xsd:string ;
                                  :rinfIndex "1.1.1.1.8.11" ,
                                             "1.2.1.0.5.8" ,
                                             "1.2.2.0.5.8" ;
                                  <http://purl.org/dc/terms/created> "2020-07-29"^^xsd:date ;
                                  <http://purl.org/dc/terms/modified> "2021-08-10"^^xsd:date ;
                                  rdfs:comment "Applicable national rolling stock fire category for a tunnel."@en ;
                                  rdfs:isDefinedBy <http://data.europa.eu/949/> ;
                                  rdfs:label "National fire category of rolling stock required"@en ;
                                  <http://www.w3.org/2003/06/sw-vocab-status/ns#term_status> "stable" .


###  http://data.europa.eu/949/netElementPosition
:netElementPosition rdf:type owl:DatatypeProperty ;
                    rdfs:domain :SpotLocation ;
                    rdfs:range xsd:integer ;
                    rdfs:isDefinedBy <http://data.europa.eu/949/> ;
                    rdfs:label "netElementPosition"@en .


###  http://data.europa.eu/949/nonCodedRestrictions
:nonCodedRestrictions rdf:type owl:DatatypeProperty ,
                               owl:FunctionalProperty ;
                      rdfs:domain :VehicleType ;
                      rdfs:range xsd:string ;
                      <http://purl.org/dc/terms/created> "2022-06-15" ;
                      <http://purl.org/dc/terms/modified> "2022-06-15"^^xsd:date ;
                      rdfs:comment "Denotes a non coded restrictions for this particular vehicleType, as a set of sentences."@en ;
                      rdfs:isDefinedBy <http://data.europa.eu/949/> ;
                      rdfs:label "non coded restrictions"@en ;
                      <http://www.w3.org/2003/06/sw-vocab-status/ns#term_status> "stable"@en .


###  http://data.europa.eu/949/numberElementsRakeFreightWagons
:numberElementsRakeFreightWagons rdf:type owl:DatatypeProperty ;
                                 rdfs:domain :VehicleType ;
                                 rdfs:range xsd:integer ;
                                 :eratvIndex "4.1.6" ;
                                 <http://purl.org/dc/terms/created> "2021-08-25"^^xsd:date ;
                                 <http://purl.org/dc/terms/modified> "2021-08-25"^^xsd:date ;
                                 rdfs:comment "Number of elements in the rake of freight wagons (only for subcategory 'rake of freight wagons')"@en ;
                                 rdfs:isDefinedBy <http://data.europa.eu/949/> ;
                                 rdfs:label "number elements rake freight wagons"@en ;
                                 <http://www.w3.org/2003/06/sw-vocab-status/ns#term_status> "stable" .


###  http://data.europa.eu/949/numberOfPantographsInContactWithOCL
:numberOfPantographsInContactWithOCL rdf:type owl:DatatypeProperty ,
                                              owl:FunctionalProperty ;
                                     rdfs:domain :VehicleType ;
                                     rdfs:range xsd:integer ;
                                     :eratvIndex "4.10.7" ;
                                     <http://purl.org/dc/terms/created> "2020-08-25"^^xsd:date ;
                                     <http://purl.org/dc/terms/modified> "2020-11-19"^^xsd:date ;
                                     rdfs:comment "Number of pantographs in contact with the overhead contact line (OCL) (to be indicated for each energy supply system the vehicle is equipped for)."@en ;
                                     rdfs:isDefinedBy <http://data.europa.eu/949/> ;
                                     rdfs:label "number of pantographs in contact with OCL"@en ;
                                     <http://www.w3.org/2003/06/sw-vocab-status/ns#term_status> "stable" .


###  http://data.europa.eu/949/numberOfToilets
:numberOfToilets rdf:type owl:DatatypeProperty ;
                 rdfs:domain :VehicleType ;
                 rdfs:range xsd:integer ;
                 :eratvIndex "4.12.1.2" ;
                 <http://purl.org/dc/terms/created> "2021-08-31"^^xsd:date ;
                 <http://purl.org/dc/terms/modified> "2021-08-31"^^xsd:date ;
                 rdfs:comment "Number of toilets."@en ;
                 rdfs:isDefinedBy <http://data.europa.eu/949/> ;
                 rdfs:label "number of toilets"@en ;
                 <http://www.w3.org/2003/06/sw-vocab-status/ns#term_status> "stable" .


###  http://data.europa.eu/949/oclType
:oclType rdf:type owl:DatatypeProperty ;
         rdfs:domain :VehicleType ;
         rdfs:range xsd:string ;
         :eratvIndex "4.10.9" ;
         <http://purl.org/dc/terms/created> "2020-08-25"^^xsd:date ;
         <http://purl.org/dc/terms/modified> "2020-10-03"^^xsd:date ;
         rdfs:comment "OCL type."@en ;
         rdfs:isDefinedBy <http://data.europa.eu/949/> ;
         rdfs:label "ocl type"@en ;
         <http://www.w3.org/2003/06/sw-vocab-status/ns#term_status> "stable" .


###  http://data.europa.eu/949/opName
:opName rdf:type owl:DatatypeProperty ,
                 owl:FunctionalProperty ;
        rdfs:domain :OperationalPoint ;
        rdfs:range xsd:string ;
        :isCoreParameter "true"^^xsd:boolean ;
        :rinfIndex "1.2.0.0.0.1" ;
        <http://purl.org/dc/terms/created> "2021-09-13"^^xsd:date ;
        <http://purl.org/dc/terms/modified> "2021-09-13"^^xsd:date ;
        rdfs:comment "Name of an Operational Point."@en ;
        rdfs:isDefinedBy <http://data.europa.eu/949/> ;
        rdfs:label "Name of Operational point"@en ;
        <http://www.w3.org/2003/06/sw-vocab-status/ns#term_status> "stable" .


###  http://data.europa.eu/949/opTypeGaugeChangeover
:opTypeGaugeChangeover rdf:type owl:DatatypeProperty ,
                                owl:FunctionalProperty ;
                       rdfs:domain :OperationalPoint ;
                       rdfs:range xsd:string ;
                       :rinfIndex "1.2.0.0.0.4.1" ;
                       <http://purl.org/dc/terms/created> "2021-08-11"^^xsd:date ;
                       <http://purl.org/dc/terms/modified> "2021-08-11"^^xsd:date ;
                       rdfs:comment "Type of track gauge changeover facility."@en ;
                       rdfs:isDefinedBy <http://data.europa.eu/949/> ;
                       rdfs:label "Type of track gauge changeover facility"@en ;
                       <http://www.w3.org/2003/06/sw-vocab-status/ns#term_status> "stable" .


###  http://data.europa.eu/949/parkingBrake
:parkingBrake rdf:type owl:DatatypeProperty ;
              rdfs:domain :VehicleType ;
              rdfs:range xsd:boolean ;
              :eratvIndex "4.7.3" ;
              <http://purl.org/dc/terms/created> "2022-04-11"^^xsd:date ;
              <http://purl.org/dc/terms/modified> "2022-04-11"^^xsd:date ;
              rdfs:comment "Indicates whether all vehicles of this type must be equipped with a parking brake."@en ;
              rdfs:isDefinedBy <http://data.europa.eu/949/> ;
              rdfs:label "parking brake"@en ;
              <http://www.w3.org/2003/06/sw-vocab-status/ns#term_status> "stable" .


###  http://data.europa.eu/949/parkingBrakeMandatory
:parkingBrakeMandatory rdf:type owl:DatatypeProperty ;
                       rdfs:domain :VehicleType ;
                       rdfs:range xsd:boolean ;
                       :eratvIndex "4.7.3.1" ;
                       <http://purl.org/dc/terms/created> "2021-08-26"^^xsd:date ;
                       <http://purl.org/dc/terms/modified> "2021-08-26"^^xsd:date ;
                       rdfs:comment "All vehicles of this type must be equipped with a parking brake (parking brake mandatory for vehicles of this type)."@en ;
                       rdfs:isDefinedBy <http://data.europa.eu/949/> ;
                       rdfs:label "parking brake mandatory"@en ;
                       <http://www.w3.org/2003/06/sw-vocab-status/ns#term_status> "stable" .


###  http://data.europa.eu/949/parkingBrakeMaximumGradient
:parkingBrakeMaximumGradient rdf:type owl:DatatypeProperty ,
                                      owl:FunctionalProperty ;
                             rdfs:domain :VehicleType ;
                             rdfs:range xsd:double ;
                             :eratvIndex "4.7.3.3" ;
                             <http://purl.org/dc/terms/created> "2020-08-24"^^xsd:date ;
                             <http://purl.org/dc/terms/modified> "2020-11-03"^^xsd:date ;
                             rdfs:comment "Maximum gradient on which the unit is kept immobilised by the parking brake alone (if the vehicle is fitted with it)."@en ;
                             rdfs:isDefinedBy <http://data.europa.eu/949/> ;
                             rdfs:label "parking brake maximum gradient"@en ;
                             <http://www.w3.org/2003/06/sw-vocab-status/ns#term_status> "stable" .


###  http://data.europa.eu/949/passByNoiseLevel
:passByNoiseLevel rdf:type owl:DatatypeProperty ;
                  rdfs:domain :VehicleType ;
                  rdfs:range xsd:double ;
                  :eratvIndex "4.11.1" ;
                  <http://purl.org/dc/terms/created> "2021-08-31"^^xsd:date ;
                  <http://purl.org/dc/terms/modified> "2021-08-31"^^xsd:date ;
                  rdfs:comment "Pass-by noise level given in dB(A)."@en ;
                  rdfs:isDefinedBy <http://data.europa.eu/949/> ;
                  rdfs:label "pass-by noise level"@en ;
                  <http://www.w3.org/2003/06/sw-vocab-status/ns#term_status> "stable" .


###  http://data.europa.eu/949/permissiblePayload
:permissiblePayload rdf:type owl:DatatypeProperty ,
                             owl:FunctionalProperty ;
                    rdfs:domain :VehicleType ;
                    rdfs:range xsd:string ;
                    :eratvIndex "4.5.1" ;
                    <http://purl.org/dc/terms/created> "2020-08-24"^^xsd:date ;
                    <http://purl.org/dc/terms/modified> "2020-11-03"^^xsd:date ;
                    rdfs:comment "Permissible payload for different line categories."@en ;
                    rdfs:isDefinedBy <http://data.europa.eu/949/> ;
                    rdfs:label "permissible payload"@en ;
                    <http://www.w3.org/2003/06/sw-vocab-status/ns#term_status> "stable" .


###  http://data.europa.eu/949/permittedContactForce
:permittedContactForce rdf:type owl:DatatypeProperty ,
                                owl:FunctionalProperty ;
                       rdfs:domain :Track ;
                       rdfs:range xsd:string ;
                       :rinfIndex "1.1.1.2.5.2" ;
                       <http://purl.org/dc/terms/created> "2020-08-25"^^xsd:date ;
                       <http://purl.org/dc/terms/modified> "2021-09-12"^^xsd:date ;
                       rdfs:comment "Indication of contact force allowed expressed in newtons."@en ;
                       rdfs:isDefinedBy <http://data.europa.eu/949/> ;
                       rdfs:label "Contact force permitted"@en ;
                       <http://www.w3.org/2003/06/sw-vocab-status/ns#term_status> "stable" .


###  http://data.europa.eu/949/phaseInfo
:phaseInfo rdf:type owl:DatatypeProperty ,
                    owl:FunctionalProperty ;
           rdfs:domain :Track ;
           rdfs:range xsd:string ;
           :rinfIndex "1.1.1.2.4.1.2" ;
           <http://purl.org/dc/terms/created> "2021-08-08"^^xsd:date ;
           <http://purl.org/dc/terms/modified> "2021-09-12"^^xsd:date ;
           rdfs:comment "Required information on phase separation. Data is structured as: length [NNN] + switch off breaker [Y/N] + lower pantograph [Y/N])."@en ;
           rdfs:isDefinedBy <http://data.europa.eu/949/> ;
           rdfs:label "Information on phase separation"@en ;
           <http://www.w3.org/2003/06/sw-vocab-status/ns#term_status> "stable" .


###  http://data.europa.eu/949/phaseSeparation
:phaseSeparation rdf:type owl:DatatypeProperty ,
                          owl:FunctionalProperty ;
                 rdfs:domain :Track ;
                 rdfs:range xsd:boolean ;
                 :rinfIndex "1.1.1.2.4.1.1" ;
                 <http://purl.org/dc/terms/created> "2021-08-08"^^xsd:date ;
                 <http://purl.org/dc/terms/modified> "2021-09-12"^^xsd:date ;
                 rdfs:comment "Indication of existence of phase separation and required information."@en ;
                 rdfs:isDefinedBy <http://data.europa.eu/949/> ;
                 rdfs:label "Phase separation"@en ;
                 <http://www.w3.org/2003/06/sw-vocab-status/ns#term_status> "stable" .


###  http://data.europa.eu/949/platformId
:platformId rdf:type owl:DatatypeProperty ,
                     owl:FunctionalProperty ;
            rdfs:domain :Platform ;
            rdfs:range xsd:string ;
            :isCoreParameter "true"^^xsd:boolean ;
            :rinfIndex "1.2.1.0.6.2" ;
            <http://purl.org/dc/terms/created> "2021-09-13"^^xsd:date ;
            <http://purl.org/dc/terms/modified> "2021-09-13"^^xsd:date ;
            rdfs:comment "Unique platform identification or number within an Operational Point."@en ;
            rdfs:isDefinedBy <http://data.europa.eu/949/> ;
            rdfs:label "platform id"@en ;
            <http://www.w3.org/2003/06/sw-vocab-status/ns#term_status> "stable" .


###  http://data.europa.eu/949/portableBoardingAids
:portableBoardingAids rdf:type owl:DatatypeProperty ;
                      rdfs:domain :VehicleType ;
                      rdfs:range xsd:string ;
                      :eratvIndex "4.12.3.3" ;
                      <http://purl.org/dc/terms/created> "2021-08-31"^^xsd:date ;
                      <http://purl.org/dc/terms/modified> "2021-08-31"^^xsd:date ;
                      rdfs:comment "Description of any portable boarding aids if considered in the design of the vehicle for meeting the PRM TSI requirements."@en ;
                      rdfs:isDefinedBy <http://data.europa.eu/949/> ;
                      rdfs:label "portable boarding aids"@en ;
                      <http://www.w3.org/2003/06/sw-vocab-status/ns#term_status> "stable" .


###  http://data.europa.eu/949/posBegin
:posBegin rdf:type owl:DatatypeProperty ;
          rdfs:domain :NetElement ;
          rdfs:range xsd:double ;
          rdfs:isDefinedBy <http://data.europa.eu/949/> ;
          rdfs:label "position begin"@en .


###  http://data.europa.eu/949/posEnd
:posEnd rdf:type owl:DatatypeProperty ;
        rdfs:domain :NetElement ;
        rdfs:range xsd:double ;
        rdfs:isDefinedBy <http://data.europa.eu/949/> ;
        rdfs:label "position end"@en .


###  http://data.europa.eu/949/preventRegenerativeBrakeUse
:preventRegenerativeBrakeUse rdf:type owl:DatatypeProperty ,
                                      owl:FunctionalProperty ;
                             rdfs:domain :VehicleType ;
                             rdfs:range xsd:boolean ;
                             :eratvIndex "4.7.4.3.2" ;
                             <http://purl.org/dc/terms/created> "2020-08-24"^^xsd:date ;
                             <http://purl.org/dc/terms/modified> "2020-11-03"^^xsd:date ;
                             rdfs:comment "Possibility of preventing the use of the regenerative brake (only if fitted with regenerative brake)."@en ;
                             rdfs:isDefinedBy <http://data.europa.eu/949/> ;
                             rdfs:label "prevent regenerative brake use"@en ;
                             <http://www.w3.org/2003/06/sw-vocab-status/ns#term_status> "stable" .


###  http://data.europa.eu/949/prioritySeats
:prioritySeats rdf:type owl:DatatypeProperty ;
               rdfs:domain :VehicleType ;
               rdfs:range xsd:string ;
               :eratvIndex "4.12.2.1" ;
               <http://purl.org/dc/terms/created> "2021-08-31"^^xsd:date ;
               <http://purl.org/dc/terms/modified> "2021-08-31"^^xsd:date ;
               rdfs:comment "Number of priority seats."@en ;
               rdfs:isDefinedBy <http://data.europa.eu/949/> ;
               rdfs:label "priority seats"@en ;
               <http://www.w3.org/2003/06/sw-vocab-status/ns#term_status> "stable" .


###  http://data.europa.eu/949/prmAccessibleToilets
:prmAccessibleToilets rdf:type owl:DatatypeProperty ;
                      rdfs:domain :VehicleType ;
                      rdfs:range xsd:integer ;
                      :eratvIndex "4.12.2.3" ;
                      <http://purl.org/dc/terms/created> "2021-08-31"^^xsd:date ;
                      <http://purl.org/dc/terms/modified> "2021-08-31"^^xsd:date ;
                      rdfs:comment "Number of PRM accessible toilets."@en ;
                      rdfs:isDefinedBy <http://data.europa.eu/949/> ;
                      rdfs:label "prm accessible toilets"@en ;
                      <http://www.w3.org/2003/06/sw-vocab-status/ns#term_status> "stable" .


###  http://data.europa.eu/949/publicNetworkRoaming
:publicNetworkRoaming rdf:type owl:DatatypeProperty ,
                               owl:FunctionalProperty ;
                      rdfs:domain :Track ;
                      rdfs:range xsd:boolean ;
                      :rinfIndex "1.1.1.3.3.6" ;
                      <http://purl.org/dc/terms/created> "2021-08-09"^^xsd:date ;
                      <http://purl.org/dc/terms/modified> "2021-09-12"^^xsd:date ;
                      rdfs:comment "Existence of roaming to public networks."@en ;
                      rdfs:isDefinedBy <http://data.europa.eu/949/> ;
                      rdfs:label "Existence of roaming to public networks"@en ;
                      <http://www.w3.org/2003/06/sw-vocab-status/ns#term_status> "stable" .


###  http://data.europa.eu/949/publicNetworkRoamingDetails
:publicNetworkRoamingDetails rdf:type owl:DatatypeProperty ,
                                      owl:FunctionalProperty ;
                             rdfs:domain :Track ;
                             rdfs:range xsd:string ;
                             :rinfIndex "1.1.1.3.3.7" ;
                             <http://purl.org/dc/terms/created> "2021-08-09"^^xsd:date ;
                             <http://purl.org/dc/terms/modified> "2021-09-12"^^xsd:date ;
                             rdfs:comment "Details on roaming to public networks."@en ;
                             rdfs:isDefinedBy <http://data.europa.eu/949/> ;
                             rdfs:label "Details on roaming to public networks"@en ;
                             <http://www.w3.org/2003/06/sw-vocab-status/ns#term_status> "stable" .


###  http://data.europa.eu/949/quasiStaticGuidingForce
:quasiStaticGuidingForce rdf:type owl:DatatypeProperty ;
                         rdfs:domain :VehicleType ;
                         rdfs:range xsd:double ;
                         :eratvIndex "4.5.4" ;
                         <http://purl.org/dc/terms/created> "2021-08-26"^^xsd:date ;
                         <http://purl.org/dc/terms/modified> "2021-08-26"^^xsd:date ;
                         rdfs:comment "Quasi-static guiding force (if exceeds the limit defined in TSI or not defined in the TSI), given in kN."@en ;
                         rdfs:isDefinedBy <http://data.europa.eu/949/> ;
                         rdfs:label "quasi static guiding force"@en ;
                         <http://www.w3.org/2003/06/sw-vocab-status/ns#term_status> "stable" .


###  http://data.europa.eu/949/radioSwitchOverSpecialConditions
:radioSwitchOverSpecialConditions rdf:type owl:DatatypeProperty ;
                                  rdfs:domain :VehicleType ;
                                  rdfs:range xsd:string ;
                                  :eratvIndex "4.13.2.4" ;
                                  <http://purl.org/dc/terms/created> "2021-08-31"^^xsd:date ;
                                  <http://purl.org/dc/terms/modified> "2021-08-31"^^xsd:date ;
                                  rdfs:comment "Special conditions implemented on-board to switch over between different radio systems. Given as combination of systems installed on board ('System XX'_'System YY')."@en ;
                                  rdfs:isDefinedBy <http://data.europa.eu/949/> ;
                                  rdfs:label "radio switch over special conditions"@en ;
                                  <http://www.w3.org/2003/06/sw-vocab-status/ns#term_status> "stable" .


###  http://data.europa.eu/949/railInclinationMeasurement
:railInclinationMeasurement rdf:type owl:DatatypeProperty ,
                                     owl:FunctionalProperty ;
                            rdfs:domain :Track ;
                            rdfs:range xsd:integer ;
                            :isCoreParameter "true"^^xsd:boolean ;
                            :rinfIndex "1.1.1.1.4.3" ;
                            <http://purl.org/dc/terms/created> "2022-09-06"^^xsd:date ;
                            <http://purl.org/dc/terms/description> "http://data.europa.eu/949/railInclination"^^xsd:anyURI ;
                            rdfs:comment """An angle defining the inclination of the head of a rail relative to the running surface. 
This is a RINF parameter treated as an integer. It has been defined in order to distinguish it from the ERATV parameter, railInclination, which is a SKOS."""@en ,
                                         "The reason for deprecation is that the definition of this porperty is being rolled back, as before, the property railInclination is a SKOS for both RINF and ERATV."@en ;
                            rdfs:isDefinedBy "http://data.europa.eu/949/"^^xsd:anyURI ;
                            rdfs:label "rail inclination measurement"@en ;
                            owl:deprecated "true"^^xsd:boolean ;
                            <http://www.w3.org/2003/06/sw-vocab-status/ns#term_status> "stable"@en .


###  http://data.europa.eu/949/raisedPantographsDistanceAndSpeed
:raisedPantographsDistanceAndSpeed rdf:type owl:DatatypeProperty ;
                                   rdfs:domain :Track ;
                                   rdfs:range xsd:string ;
                                   :rinfIndex "1.1.1.2.3.3" ;
                                   <http://purl.org/dc/terms/created> "2020-08-25"^^xsd:date ;
                                   <http://purl.org/dc/terms/modified> "2021-09-12"^^xsd:date ;
                                   rdfs:comment "Indication of maximum number of raised pantographs per train allowed and minimum spacing centre line to centre line of adjacent pantograph heads, expressed in metres, at the given speed."@en ;
                                   rdfs:isDefinedBy <http://data.europa.eu/949/> ;
                                   rdfs:label "Requirements for number of raised pantographs and spacing between them, at the given speed"@en ;
                                   <http://www.w3.org/2003/06/sw-vocab-status/ns#term_status> "stable" .


###  http://data.europa.eu/949/redLightsRequired
:redLightsRequired rdf:type owl:DatatypeProperty ,
                            owl:FunctionalProperty ;
                   rdfs:domain :Track ;
                   rdfs:range xsd:boolean ;
                   :rinfIndex "1.1.1.1.7.10" ;
                   <http://purl.org/dc/terms/created> "2021-08-08"^^xsd:date ;
                   <http://purl.org/dc/terms/modified> "2021-09-12"^^xsd:date ;
                   rdfs:comment "Indication of a sections where two steady red lights are required in accordance with Regulation (EU) 2019/773"@en ;
                   rdfs:isDefinedBy <http://data.europa.eu/949/> ;
                   rdfs:label "Steady red lights required"@en ;
                   <http://www.w3.org/2003/06/sw-vocab-status/ns#term_status> "stable" .


###  http://data.europa.eu/949/referencePassByNoiseLevel
:referencePassByNoiseLevel rdf:type owl:DatatypeProperty ;
                           rdfs:domain :VehicleType ;
                           rdfs:range xsd:boolean ;
                           :eratvIndex "4.11.2" ;
                           <http://purl.org/dc/terms/created> "2021-08-31"^^xsd:date ;
                           <http://purl.org/dc/terms/modified> "2021-08-31"^^xsd:date ;
                           rdfs:comment "Pass-by noise level was measured under reference conditions."@en ;
                           rdfs:isDefinedBy <http://data.europa.eu/949/> ;
                           rdfs:label "reference pass-by noise level"@en ;
                           <http://www.w3.org/2003/06/sw-vocab-status/ns#term_status> "stable" .


###  http://data.europa.eu/949/relativePosition
:relativePosition rdf:type owl:DatatypeProperty ;
                  rdfs:range xsd:double ;
                  <http://purl.org/dc/terms/created> "2021-04-01"^^xsd:date ;
                  <http://purl.org/dc/terms/modified> "2021-04-01"^^xsd:date ;
                  rdfs:comment "Indicates the position of an object relative to the linear coordinates of the associated topological object."@en ;
                  rdfs:isDefinedBy <http://data.europa.eu/949/> ;
                  rdfs:label "relative position"@en ;
                  <http://www.w3.org/2003/06/sw-vocab-status/ns#term_status> "stable" .


###  http://data.europa.eu/949/requiredSandingOverride
:requiredSandingOverride rdf:type owl:DatatypeProperty ;
                         rdfs:domain :TrainDetectionSystem ;
                         rdfs:range xsd:boolean ;
                         :rinfIndex "1.1.1.3.7.18" ;
                         <http://purl.org/dc/terms/created> "2021-08-08"^^xsd:date ;
                         <http://purl.org/dc/terms/modified> "2021-08-08"^^xsd:date ;
                         rdfs:comment "Indication whether possibility to activate/deactivate sanding devices by driver, according to instructions from the Infrastructure Manager, is required or not."@en ;
                         rdfs:isDefinedBy <http://data.europa.eu/949/> ;
                         rdfs:label "Sanding override by driver required"@en ;
                         <http://www.w3.org/2003/06/sw-vocab-status/ns#term_status> "stable" .


###  http://data.europa.eu/949/shortestDistanceBetweenPantographsInContactWithOCL
:shortestDistanceBetweenPantographsInContactWithOCL rdf:type owl:DatatypeProperty ,
                                                             owl:FunctionalProperty ;
                                                    rdfs:domain :VehicleType ;
                                                    rdfs:range xsd:string ;
                                                    :eratvIndex "4.10.8" ;
                                                    <http://purl.org/dc/terms/created> "2020-08-25"^^xsd:date ;
                                                    <http://purl.org/dc/terms/modified> "2021-09-15"^^xsd:date ;
                                                    rdfs:comment "Shortest distance between two pantographs in contact with the OCL (to be indicated for each energy supply system the vehicle is equipped for; to be indicated for single and, if applicable, multiple operation) (only if number of raised pantographs is more than 1)."@en ;
                                                    rdfs:isDefinedBy <http://data.europa.eu/949/> ;
                                                    rdfs:label "shortest distance between pantographs in contact with OCL"@en ;
                                                    <http://www.w3.org/2003/06/sw-vocab-status/ns#term_status> "stable" .


###  http://data.europa.eu/949/sidingId
:sidingId rdf:type owl:DatatypeProperty ;
          rdfs:subPropertyOf <http://purl.org/dc/terms/identifier> ;
          rdf:type owl:FunctionalProperty ;
          rdfs:domain :Siding ;
          rdfs:range xsd:string ;
          :isCoreParameter "true"^^xsd:boolean ;
          :rinfIndex "1.2.2.0.0.2" ;
          <http://purl.org/dc/terms/created> "2021-09-13"^^xsd:date ;
          <http://purl.org/dc/terms/modified> "2021-09-13"^^xsd:date ;
          rdfs:comment "Unique siding identification or number within an Operational Point."@en ;
          rdfs:isDefinedBy <http://data.europa.eu/949/> ;
          rdfs:label "Identification of siding"@en ;
          <http://www.w3.org/2003/06/sw-vocab-status/ns#term_status> "stable" .


###  http://data.europa.eu/949/sleepingPlaces
:sleepingPlaces rdf:type owl:DatatypeProperty ;
                rdfs:domain :VehicleType ;
                rdfs:range xsd:string ;
                :eratvIndex "4.12.1.3" ;
                <http://purl.org/dc/terms/created> "2021-08-31"^^xsd:date ;
                <http://purl.org/dc/terms/modified> "2021-09-15"^^xsd:date ;
                rdfs:comment "Number of sleeping places."@en ;
                rdfs:isDefinedBy <http://data.europa.eu/949/> ;
                rdfs:label "sleeping places"@en ;
                <http://www.w3.org/2003/06/sw-vocab-status/ns#term_status> "stable" .


###  http://data.europa.eu/949/specificInformation
:specificInformation rdf:type owl:DatatypeProperty ,
                              owl:FunctionalProperty ;
                     rdfs:domain :Track ;
                     rdfs:range xsd:string ;
                     :rinfIndex "1.1.1.1.3.5.1" ;
                     <http://purl.org/dc/terms/created> "2021-08-03"^^xsd:date ;
                     <http://purl.org/dc/terms/modified> "2021-09-10"^^xsd:date ;
                     rdfs:comment "This parameters allows the IM to provide plain text with specific information about the track."@en ;
                     rdfs:isDefinedBy <http://data.europa.eu/949/> ;
                     rdfs:label "Specific information"@en ;
                     <http://www.w3.org/2003/06/sw-vocab-status/ns#term_status> "stable" .


###  http://data.europa.eu/949/startIntrinsicCoordinate
:startIntrinsicCoordinate rdf:type owl:DatatypeProperty ;
                          rdfs:domain :NetElement ;
                          rdfs:range xsd:double ;
                          <http://purl.org/dc/terms/created> "2021-04-01"^^xsd:date ;
                          <http://purl.org/dc/terms/modified> "2021-04-01"^^xsd:date ;
                          rdfs:comment "Indicates the coordinate point where a linear object begins."@en ;
                          rdfs:isDefinedBy <http://data.europa.eu/949/> ;
                          rdfs:label "start intrinsic coordinate"@en ;
                          <http://www.w3.org/2003/06/sw-vocab-status/ns#term_status> "stable" .


###  http://data.europa.eu/949/startingNoiseLevel
:startingNoiseLevel rdf:type owl:DatatypeProperty ;
                    rdfs:domain :VehicleType ;
                    rdfs:range xsd:double ;
                    :eratvIndex "4.11.4" ;
                    <http://purl.org/dc/terms/created> "2021-08-31"^^xsd:date ;
                    <http://purl.org/dc/terms/modified> "2021-08-31"^^xsd:date ;
                    rdfs:comment "starting noise level given in dB(A)."@en ;
                    rdfs:isDefinedBy <http://data.europa.eu/949/> ;
                    rdfs:label "starting noise level"@en ;
                    <http://www.w3.org/2003/06/sw-vocab-status/ns#term_status> "stable" .


###  http://data.europa.eu/949/staticAxleLoadExceptionalPayload
:staticAxleLoadExceptionalPayload rdf:type owl:DatatypeProperty ,
                                           owl:FunctionalProperty ;
                                  rdfs:domain :VehicleType ;
                                  rdfs:range xsd:double ;
                                  :eratvIndex "4.5.3.3" ;
                                  <http://purl.org/dc/terms/created> "2020-08-24"^^xsd:date ;
                                  <http://purl.org/dc/terms/modified> "2020-11-03"^^xsd:date ;
                                  rdfs:comment "Static axle load under exceptional payload."@en ;
                                  rdfs:isDefinedBy <http://data.europa.eu/949/> ;
                                  rdfs:label "static axle load under exceptional payload"@en ;
                                  <http://www.w3.org/2003/06/sw-vocab-status/ns#term_status> "stable" .


###  http://data.europa.eu/949/staticAxleLoadNormalPayload
:staticAxleLoadNormalPayload rdf:type owl:DatatypeProperty ,
                                      owl:FunctionalProperty ;
                             rdfs:domain :VehicleType ;
                             rdfs:range xsd:double ;
                             :eratvIndex "4.5.3.2" ;
                             <http://purl.org/dc/terms/created> "2020-08-24"^^xsd:date ;
                             <http://purl.org/dc/terms/modified> "2020-11-03"^^xsd:date ;
                             rdfs:comment "Static axle load under normal payload."@en ;
                             rdfs:isDefinedBy <http://data.europa.eu/949/> ;
                             rdfs:label "static axle load under normal payload"@en ;
                             <http://www.w3.org/2003/06/sw-vocab-status/ns#term_status> "stable" .


###  http://data.europa.eu/949/staticAxleLoadWorkingOrder
:staticAxleLoadWorkingOrder rdf:type owl:DatatypeProperty ,
                                     owl:FunctionalProperty ;
                            rdfs:domain :VehicleType ;
                            rdfs:range xsd:double ;
                            :eratvIndex "4.5.3.1" ;
                            <http://purl.org/dc/terms/created> "2020-08-24"^^xsd:date ;
                            <http://purl.org/dc/terms/modified> "2020-11-03"^^xsd:date ;
                            rdfs:comment "Static axle load in working order."@en ;
                            rdfs:isDefinedBy <http://data.europa.eu/949/> ;
                            rdfs:label "static axle load in working order"@en ;
                            <http://www.w3.org/2003/06/sw-vocab-status/ns#term_status> "stable" .


###  http://data.europa.eu/949/stationaryNoiseLevel
:stationaryNoiseLevel rdf:type owl:DatatypeProperty ;
                      rdfs:domain :VehicleType ;
                      rdfs:range xsd:double ;
                      :eratvIndex "4.11.3" ;
                      <http://purl.org/dc/terms/created> "2021-08-31"^^xsd:date ;
                      <http://purl.org/dc/terms/modified> "2021-08-31"^^xsd:date ;
                      rdfs:comment "stationary noise level given in dB(A)."@en ;
                      rdfs:isDefinedBy <http://data.europa.eu/949/> ;
                      rdfs:label "stationary noise level"@en ;
                      <http://www.w3.org/2003/06/sw-vocab-status/ns#term_status> "stable" .


###  http://data.europa.eu/949/structuralCategory
:structuralCategory rdf:type owl:DatatypeProperty ;
                    rdfs:domain :VehicleType ;
                    rdfs:range xsd:string ;
                    :eratvIndex "4.1.10" ;
                    <http://purl.org/dc/terms/created> "2021-08-25"^^xsd:date ;
                    <http://purl.org/dc/terms/modified> "2021-08-25"^^xsd:date ;
                    rdfs:comment "Structural category."@en ;
                    rdfs:isDefinedBy <http://data.europa.eu/949/> ;
                    rdfs:label "structural category"@en ;
                    <http://www.w3.org/2003/06/sw-vocab-status/ns#term_status> "stable" .


###  http://data.europa.eu/949/structureCheckLocation
:structureCheckLocation rdf:type owl:DatatypeProperty ;
                        rdfs:domain :Track ;
                        rdfs:range xsd:double ;
                        :rinfIndex "1.1.1.1.2.4.3" ;
                        <http://purl.org/dc/terms/created> "2020-08-24"^^xsd:date ;
                        <http://purl.org/dc/terms/modified> "2021-09-10"^^xsd:date ;
                        rdfs:comment "Railway location of structures requiring specific checks."@en ;
                        rdfs:isDefinedBy <http://data.europa.eu/949/> ;
                        rdfs:label "Railway location of structures requiring specific checks"@en ;
                        <http://www.w3.org/2003/06/sw-vocab-status/ns#term_status> "stable" .


###  http://data.europa.eu/949/switchProtectControlWarning
:switchProtectControlWarning rdf:type owl:DatatypeProperty ,
                                      owl:FunctionalProperty ;
                             rdfs:domain :Track ;
                             rdfs:range xsd:boolean ;
                             :rinfIndex "1.1.1.3.8.1" ;
                             <http://purl.org/dc/terms/created> "2021-08-09"^^xsd:date ;
                             <http://purl.org/dc/terms/modified> "2021-09-12"^^xsd:date ;
                             rdfs:comment "Existence of switch over between different protection, control and warning systems while running."@en ;
                             rdfs:isDefinedBy <http://data.europa.eu/949/> ;
                             rdfs:label "Existence of switch over between different protection, control and warning systems while running"@en ;
                             <http://www.w3.org/2003/06/sw-vocab-status/ns#term_status> "stable" .


###  http://data.europa.eu/949/switchRadioSystem
:switchRadioSystem rdf:type owl:DatatypeProperty ,
                            owl:FunctionalProperty ;
                   rdfs:domain :Track ;
                   rdfs:range xsd:boolean ;
                   :rinfIndex "1.1.1.3.8.2" ;
                   <http://purl.org/dc/terms/created> "2021-08-09"^^xsd:date ;
                   <http://purl.org/dc/terms/modified> "2021-09-12"^^xsd:date ;
                   rdfs:comment "Indication whether a switch over between different radio systems and no communication system whilst running exist."@en ;
                   rdfs:isDefinedBy <http://data.europa.eu/949/> ;
                   rdfs:label "Existence of switch over between different radio systems"@en ;
                   <http://www.w3.org/2003/06/sw-vocab-status/ns#term_status> "stable" .


###  http://data.europa.eu/949/systemSeparationInfo
:systemSeparationInfo rdf:type owl:DatatypeProperty ,
                               owl:FunctionalProperty ;
                      rdfs:domain :Track ;
                      rdfs:range xsd:string ;
                      :rinfIndex "1.1.1.2.4.2.2" ;
                      <http://purl.org/dc/terms/created> "2021-08-08"^^xsd:date ;
                      <http://purl.org/dc/terms/modified> "2021-09-12"^^xsd:date ;
                      rdfs:comment "Required information on system separation. Data is structured as: length [NNN] + switch off breaker [Y/N] + lower pantograph [Y/N] +[CharacterString]."@en ;
                      rdfs:isDefinedBy <http://data.europa.eu/949/> ;
                      rdfs:label "Information on system separation"@en ;
                      <http://www.w3.org/2003/06/sw-vocab-status/ns#term_status> "stable" .


###  http://data.europa.eu/949/tafTAPCode
:tafTAPCode rdf:type owl:DatatypeProperty ;
            rdfs:subPropertyOf <http://purl.org/dc/terms/identifier> ;
            rdf:type owl:FunctionalProperty ;
            rdfs:domain :OperationalPoint ;
            rdfs:range xsd:string ;
            :rinfIndex "1.2.0.0.0.3" ;
            <http://purl.org/dc/terms/created> "2020-07-29"^^xsd:date ;
            <http://purl.org/dc/terms/modified> "2021-08-11"^^xsd:date ;
            rdfs:comment "Primary code developed for TAF/TAP."@en ;
            rdfs:isDefinedBy <http://data.europa.eu/949/> ;
            rdfs:label "OP TAF/TAP primary code"@en ;
            <http://www.w3.org/2003/06/sw-vocab-status/ns#term_status> "stable" .


###  http://data.europa.eu/949/tenGISId
:tenGISId rdf:type owl:DatatypeProperty ,
                   owl:FunctionalProperty ;
          rdfs:domain :Track ;
          rdfs:range xsd:string ;
          :rinfIndex "1.1.1.1.2.1.2" ;
          <http://purl.org/dc/terms/created> "2021-08-03"^^xsd:date ;
          <http://purl.org/dc/terms/modified> "2021-09-10"^^xsd:date ;
          rdfs:comment "Indication of the GIS identity (GIS ID) of the section of TEN-T database to which the track belongs."@en ;
          rdfs:isDefinedBy <http://data.europa.eu/949/> ;
          rdfs:label "TEN GIS identity"@en ;
          <http://www.w3.org/2003/06/sw-vocab-status/ns#term_status> "stable" .


###  http://data.europa.eu/949/thermalCapacityDistance
:thermalCapacityDistance rdf:type owl:DatatypeProperty ,
                                  owl:FunctionalProperty ;
                         rdfs:domain :VehicleType ;
                         rdfs:range xsd:double ;
                         :eratvIndex "4.7.2.1.4" ;
                         <http://purl.org/dc/terms/created> "2020-08-24"^^xsd:date ;
                         <http://purl.org/dc/terms/modified> "2020-11-03"^^xsd:date ;
                         rdfs:comment "Thermal capacity distance. If no reference case is indicated."@en ;
                         rdfs:isDefinedBy <http://data.europa.eu/949/> ;
                         rdfs:label "thermal capacity distance"@en ;
                         <http://www.w3.org/2003/06/sw-vocab-status/ns#term_status> "stable" .


###  http://data.europa.eu/949/thermalCapacityGradient
:thermalCapacityGradient rdf:type owl:DatatypeProperty ,
                                  owl:FunctionalProperty ;
                         rdfs:domain :VehicleType ;
                         rdfs:range xsd:double ;
                         :eratvIndex "4.7.2.1.3" ;
                         <http://purl.org/dc/terms/created> "2020-08-24"^^xsd:date ;
                         <http://purl.org/dc/terms/modified> "2020-11-03"^^xsd:date ;
                         rdfs:comment "Thermal capacity gradient. If no reference case is indicated."@en ;
                         rdfs:isDefinedBy <http://data.europa.eu/949/> ;
                         rdfs:label "thermal capacity gradient"@en ;
                         <http://www.w3.org/2003/06/sw-vocab-status/ns#term_status> "stable" .


###  http://data.europa.eu/949/thermalCapacitySpeed
:thermalCapacitySpeed rdf:type owl:DatatypeProperty ,
                               owl:FunctionalProperty ;
                      rdfs:domain :VehicleType ;
                      rdfs:range xsd:double ;
                      :eratvIndex "4.7.2.1.2" ;
                      <http://purl.org/dc/terms/created> "2020-08-24"^^xsd:date ;
                      <http://purl.org/dc/terms/modified> "2020-11-03"^^xsd:date ;
                      rdfs:comment "Thermal capacity speed. If no reference case is indicated."@en ;
                      rdfs:isDefinedBy <http://data.europa.eu/949/> ;
                      rdfs:label "thermal capacity speed"@en ;
                      <http://www.w3.org/2003/06/sw-vocab-status/ns#term_status> "stable" .


###  http://data.europa.eu/949/thermalCapacityTime
:thermalCapacityTime rdf:type owl:DatatypeProperty ,
                              owl:FunctionalProperty ;
                     rdfs:domain :VehicleType ;
                     rdfs:range xsd:integer ;
                     :eratvIndex "4.7.2.1.5" ;
                     <http://purl.org/dc/terms/created> "2020-08-24"^^xsd:date ;
                     <http://purl.org/dc/terms/modified> "2020-11-03"^^xsd:date ;
                     rdfs:comment "Thermal capacity time. If no reference case is indicated."@en ;
                     rdfs:isDefinedBy <http://data.europa.eu/949/> ;
                     rdfs:label "thermal capacity time"@en ;
                     <http://www.w3.org/2003/06/sw-vocab-status/ns#term_status> "stable" .


###  http://data.europa.eu/949/tiltingSupported
:tiltingSupported rdf:type owl:DatatypeProperty ;
                  rdfs:domain :Track ;
                  rdfs:range xsd:boolean ;
                  :rinfIndex "1.1.1.3.12.1" ;
                  <http://purl.org/dc/terms/created> "2021-08-09"^^xsd:date ;
                  <http://purl.org/dc/terms/modified> "2021-09-12"^^xsd:date ;
                  rdfs:comment "Indication whether tilting functions are supported by ETCS."@en ;
                  rdfs:isDefinedBy <http://data.europa.eu/949/> ;
                  rdfs:label "Indication whether tilting functions are supported by ETCS"@en ;
                  <http://www.w3.org/2003/06/sw-vocab-status/ns#term_status> "stable" .


###  http://data.europa.eu/949/totalVehicleMass
:totalVehicleMass rdf:type owl:DatatypeProperty ,
                           owl:FunctionalProperty ;
                  rdfs:domain :VehicleType ;
                  rdfs:range xsd:integer ;
                  :eratvIndex "4.5.5" ;
                  <http://purl.org/dc/terms/created> "2021-08-26"^^xsd:date ;
                  <http://purl.org/dc/terms/modified> "2021-08-26"^^xsd:date ;
                  rdfs:comment "Total vehicle mass (for each vehicle of the unit), given in kg."@en ;
                  rdfs:isDefinedBy <http://data.europa.eu/949/> ;
                  rdfs:label "total vehicle mass"@en ;
                  <http://www.w3.org/2003/06/sw-vocab-status/ns#term_status> "stable" .


###  http://data.europa.eu/949/trackId
:trackId rdf:type owl:DatatypeProperty ;
         rdfs:subPropertyOf <http://purl.org/dc/terms/identifier> ;
         rdf:type owl:FunctionalProperty ;
         rdfs:domain :Track ;
         rdfs:range xsd:string ;
         :isCoreParameter "true"^^xsd:boolean ;
         :rinfIndex "1.1.1.0.0.1" ,
                    "1.2.1.0.0.2" ;
         <http://purl.org/dc/terms/created> "2021-09-09"^^xsd:date ;
         <http://purl.org/dc/terms/modified> "2021-09-09"^^xsd:date ;
         rdfs:comment "Unique track identification or unique track number within a Section of Line."@en ;
         rdfs:isDefinedBy <http://data.europa.eu/949/> ;
         rdfs:label "Identification of track"@en ;
         <http://www.w3.org/2003/06/sw-vocab-status/ns#term_status> "stable" .


###  http://data.europa.eu/949/trainControlSwitchOverSpecialConditions
:trainControlSwitchOverSpecialConditions rdf:type owl:DatatypeProperty ;
                                         rdfs:domain :VehicleType ;
                                         rdfs:range xsd:string ;
                                         :eratvIndex "4.13.1.6" ;
                                         <http://purl.org/dc/terms/created> "2021-08-31"^^xsd:date ;
                                         <http://purl.org/dc/terms/modified> "2021-08-31"^^xsd:date ;
                                         rdfs:comment "Special conditions implemented on-board to switch over between different train protection control and warning systems. Given as combination of systems installed on board ('System XX'_'System YY')."@en ;
                                         rdfs:isDefinedBy <http://data.europa.eu/949/> ;
                                         rdfs:label "train control switch over special conditions"@en ;
                                         <http://www.w3.org/2003/06/sw-vocab-status/ns#term_status> "stable" .


###  http://data.europa.eu/949/trainDetectionSystemSpecificCheckDocument
:trainDetectionSystemSpecificCheckDocument rdf:type owl:DatatypeProperty ;
                                           rdfs:domain :Track ;
                                           rdfs:range xsd:string ;
                                           :rinfIndex "1.1.1.3.7.1.3" ;
                                           <http://purl.org/dc/terms/created> "2021-08-03"^^xsd:date ;
                                           <http://purl.org/dc/terms/modified> "2021-09-12"^^xsd:date ;
                                           rdfs:comment "Document with the procedure(s) related to the type of track circuits declared in 1.1.1.3.7.1.2."@en ;
                                           rdfs:isDefinedBy <http://data.europa.eu/949/> ;
                                           rdfs:label "Document with the procedure(s) related to the type of track circuits declared in 1.1.1.3.7.1.2"@en ;
                                           <http://www.w3.org/2003/06/sw-vocab-status/ns#term_status> "stable" .


###  http://data.europa.eu/949/trainIntegrityOnBoardRequired
:trainIntegrityOnBoardRequired rdf:type owl:DatatypeProperty ,
                                        owl:FunctionalProperty ;
                               rdfs:domain :Track ;
                               rdfs:range xsd:boolean ;
                               :isCoreParameter "true"^^xsd:boolean ;
                               :rinfIndex "1.1.1.3.2.8" ;
                               <http://purl.org/dc/terms/created> "2020-08-31"^^xsd:date ;
                               <http://purl.org/dc/terms/modified> "2021-09-12"^^xsd:date ;
                               rdfs:comment "Indication whether Train Integrity monitoring system (TIMS) is required to access the line for safety reasons."@en ;
                               rdfs:isDefinedBy <http://data.europa.eu/949/> ;
                               rdfs:label "Train integrity confirmation from on-board necessary for line access"@en ;
                               <http://www.w3.org/2003/06/sw-vocab-status/ns#term_status> "stable" .


###  http://data.europa.eu/949/transportableOnFerry
:transportableOnFerry rdf:type owl:DatatypeProperty ;
                      rdfs:domain :VehicleType ;
                      rdfs:range xsd:boolean ;
                      :eratvIndex "4.8.8" ;
                      <http://purl.org/dc/terms/created> "2021-08-31"^^xsd:date ;
                      <http://purl.org/dc/terms/modified> "2021-08-31"^^xsd:date ;
                      rdfs:comment "Indicates the suitability for transport on ferries."@en ;
                      rdfs:isDefinedBy <http://data.europa.eu/949/> ;
                      rdfs:label "transportable on ferry"@en ;
                      <http://www.w3.org/2003/06/sw-vocab-status/ns#term_status> "stable" .


###  http://data.europa.eu/949/tsiCompliant
:tsiCompliant rdf:type owl:DatatypeProperty ;
              rdfs:range xsd:boolean ;
              <http://purl.org/dc/terms/created> "2020-11-03"^^xsd:date ;
              <http://purl.org/dc/terms/modified> "2020-11-03"^^xsd:date ;
              rdfs:comment "Indicates if a certain property is TSI compliant."@en ;
              rdfs:isDefinedBy <http://data.europa.eu/949/> ;
              rdfs:label "tsi compliant"@en ;
              <http://www.w3.org/2003/06/sw-vocab-status/ns#term_status> "stable" .


###  http://data.europa.eu/949/tsiSwitchCrossing
:tsiSwitchCrossing rdf:type owl:DatatypeProperty ,
                            owl:FunctionalProperty ;
                   rdfs:domain :Track ;
                   rdfs:range xsd:boolean ;
                   :isCoreParameter "true"^^xsd:boolean ;
                   :rinfIndex "1.1.1.1.5.1" ;
                   <http://purl.org/dc/terms/created> "2021-08-03"^^xsd:date ;
                   <http://purl.org/dc/terms/modified> "2021-09-10"^^xsd:date ;
                   rdfs:comment "Switches and crossings are maintained to in service limit dimension as specified in TSI."@en ;
                   rdfs:isDefinedBy <http://data.europa.eu/949/> ;
                   rdfs:label "TSI compliance of in service values for switches and crossings"@en ;
                   <http://www.w3.org/2003/06/sw-vocab-status/ns#term_status> "stable" .


###  http://data.europa.eu/949/tunnel
:tunnel rdf:type owl:DatatypeProperty ;
        rdfs:domain :Track ;
        rdfs:range xsd:boolean ;
        rdfs:isDefinedBy <http://data.europa.eu/949/> ;
        rdfs:label "is tunnel"@en ;
        <http://www.w3.org/2004/02/skos/core#definition> "Whether or not a track is associated with a tunnel."@en .


###  http://data.europa.eu/949/tunnelDocRef
:tunnelDocRef rdf:type owl:DatatypeProperty ;
              rdfs:domain :Tunnel ;
              rdfs:range xsd:string ;
              :rinfIndex "1.1.1.1.8.8.2" ;
              <http://purl.org/dc/terms/created> "2021-08-03"^^xsd:date ;
              <http://purl.org/dc/terms/modified> "2021-08-03"^^xsd:date ;
              rdfs:comment "Reference to a document available from the IM with precise description of the tunnel."@en ;
              rdfs:isDefinedBy <http://data.europa.eu/949/> ;
              rdfs:label "Reference to a document available from the IM with precise description of the tunnel"@en ;
              <http://www.w3.org/2003/06/sw-vocab-status/ns#term_status> "stable" .


###  http://data.europa.eu/949/tunnelIdentification
:tunnelIdentification rdf:type owl:DatatypeProperty ;
                      rdfs:subPropertyOf <http://purl.org/dc/terms/identifier> ;
                      rdf:type owl:FunctionalProperty ;
                      rdfs:domain :Tunnel ;
                      rdfs:range xsd:string ;
                      :isCoreParameter "true"^^xsd:boolean ;
                      :rinfIndex "1.1.1.1.8.2" ,
                                 "1.2.1.0.5.2" ,
                                 "1.2.2.0.5.2" ;
                      <http://purl.org/dc/terms/created> "2021-08-03"^^xsd:date ;
                      <http://purl.org/dc/terms/modified> "2021-09-13"^^xsd:date ;
                      rdfs:comment "Unique tunnel identification or unique number within Member State."@en ;
                      rdfs:isDefinedBy <http://data.europa.eu/949/> ;
                      rdfs:label "Tunnel identification"@en ;
                      <http://www.w3.org/2003/06/sw-vocab-status/ns#term_status> "stable" .


###  http://data.europa.eu/949/typeVersionNumber
:typeVersionNumber rdf:type owl:DatatypeProperty ,
                            owl:FunctionalProperty ;
                   rdfs:domain :VehicleType ;
                   rdfs:range xsd:string ;
                   <http://purl.org/dc/terms/created> "2020-11-22"^^xsd:date ;
                   <http://purl.org/dc/terms/modified> "2020-11-22"^^xsd:date ;
                   rdfs:comment "Serial number that identifies a vehicle type."@en ;
                   rdfs:isDefinedBy <http://data.europa.eu/949/> ;
                   rdfs:label "type version number"@en ;
                   <http://www.w3.org/2003/06/sw-vocab-status/ns#term_status> "stable" .


###  http://data.europa.eu/949/umax2
:umax2 rdf:type owl:DatatypeProperty ;
       rdfs:domain :ContactLineSystem ;
       rdfs:range xsd:integer ;
       :rinfIndex "1.1.1.2.2.1.3" ;
       <http://purl.org/dc/terms/created> "2020-08-24"^^xsd:date ;
       <http://purl.org/dc/terms/modified> "2021-08-06"^^xsd:date ;
       rdfs:comment "Umax2 for lines referred to in sections 7.4.2.2.1 and 7.4.2.11.1 of Regulation (EU)1301/2014. Specific for the French network."@en ;
       rdfs:isDefinedBy <http://data.europa.eu/949/> ;
       rdfs:label "Umax2 for lines referred to in sections 7.4.2.2.1 and 7.4.2.11.1 of Regulation (EU)1301/2014."@en ;
       <http://www.w3.org/2003/06/sw-vocab-status/ns#term_status> "stable" .


###  http://data.europa.eu/949/uopid
:uopid rdf:type owl:DatatypeProperty ;
       rdfs:subPropertyOf <http://purl.org/dc/terms/identifier> ;
       rdf:type owl:FunctionalProperty ;
       rdfs:domain :OperationalPoint ;
       rdfs:range xsd:string ;
       :isCoreParameter "true"^^xsd:boolean ;
       :rinfIndex "1.2.0.0.0.2" ;
       <http://purl.org/dc/terms/created> "2020-07-29"^^xsd:date ;
       <http://purl.org/dc/terms/modified> "2021-08-11"^^xsd:date ;
       rdfs:comment "Code composed of country code and alphanumeric operational point code, as defined in RINF."@en ;
       rdfs:isDefinedBy <http://data.europa.eu/949/> ;
       rdfs:label "Unique OP ID"@en ;
       <http://www.w3.org/2003/06/sw-vocab-status/ns#term_status> "stable" .


###  http://data.europa.eu/949/usesGroup555
:usesGroup555 rdf:type owl:DatatypeProperty ,
                       owl:FunctionalProperty ;
              rdfs:domain [ rdf:type owl:Class ;
                            owl:unionOf ( :Track
                                          :VehicleType
                                        )
                          ] ;
              rdfs:range xsd:boolean ;
              :eratvIndex "4.13.2.12" ;
              :rinfIndex "1.1.1.3.3.4" ;
              <http://purl.org/dc/terms/created> "2020-08-31"^^xsd:date ;
              <http://purl.org/dc/terms/modified> "2021-09-12"^^xsd:date ;
              rdfs:comment "Indication if group 555 is needed/used."@en ;
              rdfs:isDefinedBy <http://data.europa.eu/949/> ;
              rdfs:label "Use of group 555"@en ;
              <http://www.w3.org/2003/06/sw-vocab-status/ns#term_status> "stable" .


###  http://data.europa.eu/949/validityEndDate
:validityEndDate rdf:type owl:DatatypeProperty ;
                 rdfs:domain :ValidityPeriod ;
                 rdfs:range xsd:date ;
                 <http://purl.org/dc/terms/created> "2022-10-19"^^xsd:date ;
                 rdfs:comment "Defines the validity end date (e.g., an operational point that is not valid anymore), so that it is possible to filter out those that are not applicable for a specific application (e.g., for route planning)"@en ;
                 rdfs:isDefinedBy "http://data.europa.eu/949/"^^xsd:anyURI ;
                 rdfs:label "validity end date"@en ;
                 <http://www.w3.org/2003/06/sw-vocab-status/ns#term_status> "stable"@en .


###  http://data.europa.eu/949/validityStartDate
:validityStartDate rdf:type owl:DatatypeProperty ;
                   rdfs:domain :ValidityPeriod ;
                   rdfs:range xsd:date ;
                   <http://purl.org/dc/terms/created> "2022-10-20"^^xsd:date ;
                   rdf:label "validity start date"@en ;
                   rdfs:comment "Defines the validity start date (e.g., an operational point that is not valid now since it is planned for the future), so that it is possible to filter out those that are not applicable for a specific application (e.g., for route planning)"@en ;
                   rdfs:isDefinedBy "http://data.europa.eu/949/"^^xsd:anyURI ;
                   <http://www.w3.org/2003/06/sw-vocab-status/ns#term_status> "stable"@en .


###  http://data.europa.eu/949/vehicleContactForce
:vehicleContactForce rdf:type owl:DatatypeProperty ,
                              owl:FunctionalProperty ;
                     rdfs:domain :VehicleType ;
                     rdfs:range xsd:integer ;
                     :eratvIndex "4.10.15" ;
                     <http://purl.org/dc/terms/created> "2020-08-25"^^xsd:date ;
                     <http://purl.org/dc/terms/modified> "2020-11-03"^^xsd:date ;
                     rdfs:comment "Mean contact force."@en ;
                     rdfs:isDefinedBy <http://data.europa.eu/949/> ;
                     rdfs:label "vehicle contact force"@en ;
                     <http://www.w3.org/2003/06/sw-vocab-status/ns#term_status> "stable" .


###  http://data.europa.eu/949/vehicleKinematicGaugeOther
:vehicleKinematicGaugeOther rdf:type owl:DatatypeProperty ;
                            rdfs:domain :VehicleType ;
                            rdfs:range xsd:string ;
                            :eratvIndex "4.2.2" ;
                            <http://purl.org/dc/terms/created> "2022-05-30" ;
                            rdfs:comment "Vehicle kinematic gauge  that corresponds to other gauges assessed using the kinematic method"@en ;
                            rdfs:isDefinedBy <http://data.europa.eu/949/> ;
                            rdfs:label "vehicle kinematic gauge other"@en ;
                            <http://www.w3.org/2003/06/sw-vocab-status/ns#term_status> "stable"@en .


###  http://data.europa.eu/949/vehicleMaxSandingOutput
:vehicleMaxSandingOutput rdf:type owl:DatatypeProperty ;
                         rdfs:domain :VehicleType ;
                         rdfs:range xsd:string ;
                         :eratvIndex "4.14.2.13" ;
                         <http://purl.org/dc/terms/created> "2021-09-01"^^xsd:date ;
                         <http://purl.org/dc/terms/modified> "2021-09-01"^^xsd:date ;
                         rdfs:comment "Vehicle Maximum sanding output, given in grams per second."@en ;
                         rdfs:isDefinedBy <http://data.europa.eu/949/> ;
                         rdfs:label "vehicle max sanding output"@en ;
                         <http://www.w3.org/2003/06/sw-vocab-status/ns#term_status> "stable" .


###  http://data.europa.eu/949/vehicleNumber
:vehicleNumber rdf:type owl:DatatypeProperty ;
               rdfs:domain :Vehicle ;
               rdfs:range xsd:string ;
               <http://purl.org/dc/terms/created> "2020-11-24"^^xsd:date ;
               <http://purl.org/dc/terms/modified> "2020-11-24"^^xsd:date ;
               rdfs:comment "Identification number of a vehicle or wagon."@en ;
               rdfs:isDefinedBy <http://data.europa.eu/949/> ;
               rdfs:label "vehicle number"@en ;
               <http://www.w3.org/2003/06/sw-vocab-status/ns#term_status> "stable" .


###  http://data.europa.eu/949/vehiclePantographHead
:vehiclePantographHead rdf:type owl:DatatypeProperty ;
                       rdfs:domain :VehicleType ;
                       rdfs:range xsd:string ;
                       :eratvIndex "4.10.6" ;
                       <http://purl.org/dc/terms/created> "2020-08-25"^^xsd:date ;
                       <http://purl.org/dc/terms/modified> "2020-11-03"^^xsd:date ;
                       rdfs:comment "Pantograph head geometry (to be indicated for each energy supply system the vehicle is equipped for)."@en ;
                       rdfs:isDefinedBy <http://data.europa.eu/949/> ;
                       rdfs:label "vehicle pantograph head"@en ;
                       <http://www.w3.org/2003/06/sw-vocab-status/ns#term_status> "stable" .


###  http://data.europa.eu/949/vehicleSeries
:vehicleSeries rdf:type owl:DatatypeProperty ;
               rdfs:domain :Vehicle ;
               rdfs:range xsd:string ;
               <http://purl.org/dc/terms/created> "2020-11-22"^^xsd:date ;
               <http://purl.org/dc/terms/modified> "2020-11-22"^^xsd:date ;
               rdfs:comment "Manufacturing series of a vehicle."@en ;
               rdfs:isDefinedBy <http://data.europa.eu/949/> ;
               rdfs:label "vehicle series"@en ;
               <http://www.w3.org/2003/06/sw-vocab-status/ns#term_status> "unstable" .


###  http://data.europa.eu/949/vehiclesComposingFixedFormation
:vehiclesComposingFixedFormation rdf:type owl:DatatypeProperty ,
                                          owl:FunctionalProperty ;
                                 rdfs:domain :VehicleType ;
                                 rdfs:range xsd:integer ;
                                 :eratvIndex "4.1.12" ;
                                 <http://purl.org/dc/terms/created> "2021-08-25"^^xsd:date ;
                                 <http://purl.org/dc/terms/modified> "2021-08-25"^^xsd:date ;
                                 rdfs:comment "Number of vehicles composing the fixed formation (for fixed formation only). Note: the value is mandatory for all vehicle categories. If the vehicle is composed of only one car, the indicated value shall be '1'."@en ;
                                 rdfs:isDefinedBy <http://data.europa.eu/949/> ;
                                 rdfs:label "vehicles composing fixed formation"@en ;
                                 <http://www.w3.org/2003/06/sw-vocab-status/ns#term_status> "stable" .


###  http://data.europa.eu/949/verificationCCS
:verificationCCS rdf:type owl:DatatypeProperty ;
                 rdfs:domain :Track ;
                 rdfs:range xsd:string ;
                 :rinfIndex "1.1.1.3.1.1" ;
                 <http://purl.org/dc/terms/created> "2021-08-08"^^xsd:date ;
                 <http://purl.org/dc/terms/modified> "2022-07-28"^^xsd:date ;
                 rdfs:comment "Unique number for EC declarations concerning requirements of CCS (Command - Control and Signalling subsystem) on the specific track."@en ;
                 rdfs:isDefinedBy <http://data.europa.eu/949/> ;
                 rdfs:label "EC declaration of verification for track (CCS)"@en ;
                 <http://www.w3.org/2003/06/sw-vocab-status/ns#term_status> "stable" .


###  http://data.europa.eu/949/verificationENE
:verificationENE rdf:type owl:DatatypeProperty ;
                 rdfs:domain :Track ;
                 rdfs:range xsd:string ;
                 :rinfIndex "1.1.1.2.1.1" ;
                 <http://purl.org/dc/terms/created> "2021-08-08"^^xsd:date ;
                 <http://purl.org/dc/terms/modified> "2021-09-11"^^xsd:date ;
                 rdfs:comment "Unique number for EC declarations concerning requirements of ENE (ENErgy subsystem) on the specific track."@en ;
                 rdfs:isDefinedBy <http://data.europa.eu/949/> ;
                 rdfs:label "EC declaration of verification for track (ENE)"@en ;
                 <http://www.w3.org/2003/06/sw-vocab-status/ns#term_status> "stable" .


###  http://data.europa.eu/949/verificationINF
:verificationINF rdf:type owl:DatatypeProperty ;
                 rdfs:domain [ rdf:type owl:Class ;
                               owl:unionOf ( :Siding
                                             :Track
                                           )
                             ] ;
                 rdfs:range xsd:string ;
                 :rinfIndex "1.1.1.1.1.1" ,
                            "1.2.1.0.1.1" ,
                            "1.2.2.0.1.1" ;
                 <http://purl.org/dc/terms/created> "2021-08-03"^^xsd:date ;
                 <http://purl.org/dc/terms/modified> "2021-09-09"^^xsd:date ;
                 rdfs:comment "Unique number for EC declarations concerning requirements of INF (INFrastructure) TSI."@en ;
                 rdfs:isDefinedBy <http://data.europa.eu/949/> ;
                 rdfs:label "EC declaration of verification for track/siding [INF]"@en ;
                 <http://www.w3.org/2003/06/sw-vocab-status/ns#term_status> "stable" .


###  http://data.europa.eu/949/verificationSRT
:verificationSRT rdf:type owl:DatatypeProperty ;
                 rdfs:domain :Tunnel ;
                 rdfs:range xsd:string ;
                 :rinfIndex "1.1.1.1.8.5" ,
                            "1.2.1.0.5.3" ,
                            "1.2.2.0.5.3" ;
                 <http://purl.org/dc/terms/created> "2021-08-03"^^xsd:date ;
                 <http://purl.org/dc/terms/modified> "2021-09-02"^^xsd:date ;
                 rdfs:comment "Unique number for EC declarations concerning requirements of SRT (Safety in Railway Tunnels) TSI for infrastructure system."@en ;
                 rdfs:isDefinedBy <http://data.europa.eu/949/> ;
                 rdfs:label "EC declaration of verification for tunnel (SRT)"@en ;
                 <http://www.w3.org/2003/06/sw-vocab-status/ns#term_status> "stable" .


###  http://data.europa.eu/949/voiceOperationalCommImpl
:voiceOperationalCommImpl rdf:type owl:DatatypeProperty ,
                                   owl:FunctionalProperty ;
                          rdfs:domain :VehicleType ;
                          rdfs:range xsd:string ;
                          :eratvIndex "4.13.2.6" ;
                          <http://purl.org/dc/terms/created> "2021-08-31"^^xsd:date ;
                          <http://purl.org/dc/terms/modified> "2021-08-31"^^xsd:date ;
                          rdfs:comment "Voice and operational communication implementation."@en ;
                          rdfs:isDefinedBy <http://data.europa.eu/949/> ;
                          rdfs:label "voice operational communication implementation"@en ;
                          <http://www.w3.org/2003/06/sw-vocab-status/ns#term_status> "stable" .


###  http://data.europa.eu/949/voltage
:voltage rdf:type owl:DatatypeProperty ;
         rdfs:domain :NetElement ;
         rdfs:range xsd:double ;
         <http://purl.org/dc/terms/source> "https://otl.prorail.nl/imx/vigerend/M_VOLTAGE"^^xsd:anyURI ;
         rdfs:isDefinedBy <http://data.europa.eu/949/> ;
         rdfs:label "voltage"@en .


###  http://data.europa.eu/949/wheelSetGaugeTransformationMethod
:wheelSetGaugeTransformationMethod rdf:type owl:DatatypeProperty ;
                                   rdfs:domain :VehicleType ;
                                   rdfs:range xsd:string ;
                                   :eratvIndex "4.1.3.b" ;
                                   <http://purl.org/dc/terms/created> "2021-08-25"^^xsd:date ;
                                   <http://purl.org/dc/terms/modified> "2021-08-25"^^xsd:date ;
                                   rdfs:comment "Wheel gauge transformation method. Defined if more than one wheel gauges have been selected."@en ;
                                   rdfs:isDefinedBy <http://data.europa.eu/949/> ;
                                   rdfs:label "wheel set gauge transformation method"@en ;
                                   <http://www.w3.org/2003/06/sw-vocab-status/ns#term_status> "stable" .


###  http://data.europa.eu/949/wheelchairSleepingPlaces
:wheelchairSleepingPlaces rdf:type owl:DatatypeProperty ;
                          rdfs:domain :VehicleType ;
                          rdfs:range xsd:string ;
                          :eratvIndex "4.12.2.4" ;
                          <http://purl.org/dc/terms/created> "2021-08-31"^^xsd:date ;
                          <http://purl.org/dc/terms/modified> "2021-08-31"^^xsd:date ;
                          rdfs:comment "Number of wheelchair accessible sleeping places."@en ;
                          rdfs:isDefinedBy <http://data.europa.eu/949/> ;
                          rdfs:label "wheelchair sleeping spaces"@en ;
                          <http://www.w3.org/2003/06/sw-vocab-status/ns#term_status> "stable" .


###  http://data.europa.eu/949/wheelchairSpaces
:wheelchairSpaces rdf:type owl:DatatypeProperty ;
                  rdfs:domain :VehicleType ;
                  rdfs:range xsd:string ;
                  :eratvIndex "4.12.2.2" ;
                  <http://purl.org/dc/terms/created> "2021-08-31"^^xsd:date ;
                  <http://purl.org/dc/terms/modified> "2021-08-31"^^xsd:date ;
                  rdfs:comment "Number of wheelchair spaces."@en ;
                  rdfs:isDefinedBy <http://data.europa.eu/949/> ;
                  rdfs:label "wheelchair spaces"@en ;
                  <http://www.w3.org/2003/06/sw-vocab-status/ns#term_status> "stable" .


###  http://purl.org/dc/terms/identifier
<http://purl.org/dc/terms/identifier> rdf:type owl:DatatypeProperty .


#################################################################
#    Classes
#################################################################

###  http://data.europa.eu/949/Border
:Border rdf:type owl:Class ;
        rdfs:subClassOf :OperationalPoint ;
        <http://purl.org/dc/terms/source> "https://wiki3.railml.org/wiki/IS:border"^^xsd:anyURI ;
        rdfs:isDefinedBy <http://data.europa.eu/949/> ;
        rdfs:label "border"@en ;
        <http://www.w3.org/2004/02/skos/core#definition> "A border point is used to separate the railway network due to different reasons. Typical examples are country borders, the change of owning infrastructure manager or the border of a station."@en .


###  http://data.europa.eu/949/Certificate
:Certificate rdf:type owl:Class ;
             <http://purl.org/dc/terms/created> "2022-06-15"^^xsd:date ;
             <http://purl.org/dc/terms/modified> "2022-06-15"^^xsd:date ;
             rdfs:isDefinedBy <http://data.europa.eu/949/> ;
             rdfs:label "Certificate"@en ;
             <http://www.w3.org/2003/06/sw-vocab-status/ns#term_status> "stable"@en .


###  http://data.europa.eu/949/ContactLineSystem
:ContactLineSystem rdf:type owl:Class ;
                   <http://purl.org/dc/terms/created> "2021-08-04"^^xsd:date ;
                   <http://purl.org/dc/terms/modified> "2021-08-04"^^xsd:date ;
                   rdfs:comment "System that is used to transmit electrical energy to road or rail vehicles."@en ;
                   rdfs:isDefinedBy <http://data.europa.eu/949/> ;
                   rdfs:label "Contact Line System"@en ;
                   <http://www.w3.org/2003/06/sw-vocab-status/ns#term_status> "stable" .


###  http://data.europa.eu/949/ETCSLevel
:ETCSLevel rdf:type owl:Class ;
           <http://purl.org/dc/terms/created> "2021-08-07"^^xsd:date ;
           <http://purl.org/dc/terms/modified> "2021-08-07"^^xsd:date ;
           rdfs:comment "ERTMS / ETCS application level related to the track side equipment."@en ;
           rdfs:isDefinedBy <http://data.europa.eu/949/> ;
           rdfs:label "ETCS Level"@en ;
           <http://www.w3.org/2003/06/sw-vocab-status/ns#term_status> "stable" .


###  http://data.europa.eu/949/EraFeature
:EraFeature rdf:type owl:Class ;
            rdfs:subClassOf <http://www.opengis.net/ont/geosparql#Feature> ;
            <http://purl.org/dc/terms/created> "2022-07-07"@en ;
            rdfs:comment "Class that encompasses the features that have been physically implemented (class PhysicalImplementationFeature) and the topological objects (class Topological Object). It is a subclass of the geographical Feature class that has a spatial representation."@en ;
            rdfs:isDefinedBy <http://data.europa.eu/949/> ;
            rdfs:label "ERA Feature"@en .


###  http://data.europa.eu/949/FreightTerminal
:FreightTerminal rdf:type owl:Class ;
                 rdfs:subClassOf :PrincipalLocation ;
                 rdf:label "Freight Terminal"@en ;
                 rdfs:isDefinedBy <http://data.europa.eu/949/> .


###  http://data.europa.eu/949/GradientCurve
:GradientCurve rdf:type owl:Class ;
               rdfs:subClassOf rdf:Bag ;
               rdfs:isDefinedBy <http://data.europa.eu/949/> ;
               rdfs:label "Gradient Curve"@en .


###  http://data.europa.eu/949/InfrastructureManager
:InfrastructureManager rdf:type owl:Class ;
                       rdfs:subClassOf <http://www.w3.org/ns/org#Organization> ;
                       <http://purl.org/dc/terms/source> "https://wiki3.railml.org/wiki/CO:infrastructureManager"^^xsd:anyURI ;
                       rdfs:isDefinedBy <http://data.europa.eu/949/> ;
                       rdfs:label "Infrastructure manager"@en ;
                       <http://www.w3.org/2004/02/skos/core#definition> "The infrastructure manager owns and operates the railway network and related infrastructure."@en ;
                       <http://www.w3.org/2004/02/skos/core#scopeNote> "See point (2) of Article 3 of Directive 2012/34/EU of the European Parliament and of the Council establishing a single European railway area."@en .


###  http://data.europa.eu/949/Junction
:Junction rdf:type owl:Class ;
          rdfs:subClassOf :PrincipalLocation ;
          rdfs:isDefinedBy <http://data.europa.eu/949/> ;
          rdfs:label "Junction"@en .


###  http://data.europa.eu/949/LineReference
:LineReference rdf:type owl:Class ;
               <http://purl.org/dc/terms/created> "2021-01-29"^^xsd:date ;
               <http://purl.org/dc/terms/modified> "2021-01-29"^^xsd:date ;
               rdfs:comment "A reference to a specific national railway line."@en ;
               rdfs:isDefinedBy <http://data.europa.eu/949/> ;
               rdfs:label "Line Reference"@en ;
               <http://www.w3.org/2003/06/sw-vocab-status/ns#term_status> "stable" .


###  http://data.europa.eu/949/LinearLocation
:LinearLocation rdf:type owl:Class ;
                rdfs:isDefinedBy <http://data.europa.eu/949/> ;
                rdfs:label "linear location"@en ;
                <http://www.w3.org/2004/02/skos/core#scopeNote> "Defines location information as a linear shape (no branches) with a start- and end point. (Definition RSM)"@en .


###  http://data.europa.eu/949/Loop
:Loop rdf:type owl:Class ;
      rdfs:subClassOf :Track ;
      <http://purl.org/dc/terms/source> "Official Journal of the European Union L 139 I/85"@en ;
      rdfs:isDefinedBy <http://data.europa.eu/949/> ;
      rdfs:label "Loop"@en ;
      <http://www.w3.org/2004/02/skos/core#definition> "Track, connected to the main track, used for passing, crossing and stabling."@en .


###  http://data.europa.eu/949/Manufacturer
:Manufacturer rdf:type owl:Class ;
              rdfs:subClassOf <http://www.w3.org/ns/org#Organization> ;
              <http://purl.org/dc/terms/created> "2020-11-19"^^xsd:date ;
              <http://purl.org/dc/terms/modified> "2020-11-19"^^xsd:date ;
              rdfs:comment "A company or organization that manufactures vehicles."@en ;
              rdfs:isDefinedBy <http://data.europa.eu/949/> ;
              rdfs:label "Manufacturer"@en ;
              <http://www.w3.org/2003/06/sw-vocab-status/ns#term_status> "stable" .


###  http://data.europa.eu/949/NationalRailwayLine
:NationalRailwayLine rdf:type owl:Class ;
                     <http://purl.org/dc/terms/created> "2021-01-25"^^xsd:date ;
                     <http://purl.org/dc/terms/modified> "2021-08-03"^^xsd:date ;
                     rdfs:comment "Railway line within a member state."@en ;
                     rdfs:isDefinedBy <http://data.europa.eu/949/> ;
                     rdfs:label "National Railway Line"@en ;
                     <http://www.w3.org/2003/06/sw-vocab-status/ns#term_status> "stable" .


###  http://data.europa.eu/949/NetElement
:NetElement rdf:type owl:Class ;
            rdfs:subClassOf :TopologicalObject ;
            <http://purl.org/dc/terms/created> "2021-04-01"^^xsd:date ;
            <http://purl.org/dc/terms/modified> "2021-04-01"^^xsd:date ;
            rdfs:comment "Base class for defining nodes in the connectivity graph representing the topological network."@en ;
            rdfs:isDefinedBy <http://data.europa.eu/949/> ;
            rdfs:label "Net Element"@en ;
            rdfs:seeAlso "http://wiki.railtopomodel.org/index.php?title=Main_Page" ;
            <http://www.w3.org/2003/06/sw-vocab-status/ns#term_status> "stable" .


###  http://data.europa.eu/949/NetRelation
:NetRelation rdf:type owl:Class ;
             rdfs:subClassOf :TopologicalObject ;
             <http://purl.org/dc/terms/created> "2021-04-01"^^xsd:date ;
             <http://purl.org/dc/terms/modified> "2021-04-01"^^xsd:date ;
             rdfs:comment "Base class for defining edges in the connectivity graph representing the topological network."@en ;
             rdfs:isDefinedBy <http://data.europa.eu/949/> ;
             rdfs:label "Net Relation"@en ;
             rdfs:seeAlso "http://wiki.railtopomodel.org/index.php?title=Main_Page" ;
             <http://www.w3.org/2003/06/sw-vocab-status/ns#term_status> "stable" .


###  http://data.europa.eu/949/OperationalPoint
:OperationalPoint rdf:type owl:Class ;
                  rdfs:subClassOf :PhysicalImplementationFeature ;
                  <http://purl.org/dc/terms/created> "2020-07-29"^^xsd:date ;
                  <http://purl.org/dc/terms/modified> "2022-07-07"^^xsd:date ;
                  rdfs:comment "An operational point (OP) means any location for train service operations, where train services may begin and end or change route, and where passenger or freight services may be provided; operational point also means any location at boundaries between Member States or infrastructure managers."@en ;
                  rdfs:isDefinedBy <http://data.europa.eu/949/> ;
                  rdfs:label "Operational Point"@en ;
                  <http://www.w3.org/2003/06/sw-vocab-status/ns#term_status> "stable" .


###  http://data.europa.eu/949/OverCrossing
:OverCrossing rdf:type owl:Class ;
              rdfs:subClassOf :OperationalPoint ;
              <http://purl.org/dc/terms/source> "https://wiki3.railml.org/wiki/IS:overCrossing"^^xsd:anyURI ;
              rdfs:isDefinedBy <http://data.europa.eu/949/> ;
              rdfs:label "over crossing"@en ;
              <http://www.w3.org/2004/02/skos/core#definition> "An over crossing describes a crossing, where something crosses over the railway line. From constructional point of view an over crossing can be a bridge or a tunnel."@nl .


###  http://data.europa.eu/949/PhysicalImplementationFeature
:PhysicalImplementationFeature rdf:type owl:Class ;
                               rdfs:subClassOf :EraFeature ;
                               <http://purl.org/dc/terms/created> "2022-07-07" ;
                               rdfs:comment """This class encompasses all those classes that represent features that are physically implemented in the European railway infrastructure. It is a subclass of the geographical class Feature that has a spatial representation. It covers sidings, tracks, platforms, tunnels, operational points, and sections of line.
A feature that has been physically implemented can be abstracted (hasAbstraction) as a topological object. It also is related to the infrastructure manager through the property infrastructureMgr.""" ;
                               rdfs:isDefinedBy <http://data.europa.eu/949/> ;
                               rdfs:label "Physical Implementation Feature"@en .


###  http://data.europa.eu/949/Platform
:Platform rdf:type owl:Class ;
          rdfs:subClassOf :PhysicalImplementationFeature ;
          <http://purl.org/dc/terms/created> "2021-08-02"^^xsd:date ;
          <http://purl.org/dc/terms/modified> "2022-07-07"^^xsd:date ;
          rdfs:comment "Platform for the purpose of RINF is understood as a platform edge. A platform concerns only the part of the structure neighbouring to the track (interfaced with trains)."@en ;
          rdfs:isDefinedBy <http://data.europa.eu/949/> ;
          rdfs:label "Platform"@en ;
          <http://www.w3.org/2003/06/sw-vocab-status/ns#term_status> "stable" .


###  http://data.europa.eu/949/PrincipalLocation
:PrincipalLocation rdf:type owl:Class ;
                   owl:equivalentClass [ owl:intersectionOf ( :OperationalPoint
                                                              [ rdf:type owl:Restriction ;
                                                                owl:onProperty :opType ;
                                                                owl:someValuesFrom <http://www.w3.org/2004/02/skos/core#Concept>
                                                              ]
                                                            ) ;
                                         rdf:type owl:Class
                                       ] ;
                   rdfs:isDefinedBy <http://data.europa.eu/949/> ;
                   rdfs:label "principal location"@en .


###  http://data.europa.eu/949/SectionOfLine
:SectionOfLine rdf:type owl:Class ;
               rdfs:subClassOf :PhysicalImplementationFeature ,
                               [ rdf:type owl:Restriction ;
                                 owl:onProperty :lineNationalId ;
                                 owl:qualifiedCardinality "1"^^xsd:nonNegativeInteger ;
                                 owl:onClass :NationalRailwayLine
                               ] ,
                               [ rdf:type owl:Restriction ;
                                 owl:onProperty :opEnd ;
                                 owl:qualifiedCardinality "1"^^xsd:nonNegativeInteger ;
                                 owl:onClass :OperationalPoint
                               ] ,
                               [ rdf:type owl:Restriction ;
                                 owl:onProperty :opStart ;
                                 owl:qualifiedCardinality "1"^^xsd:nonNegativeInteger ;
                                 owl:onClass :OperationalPoint
                               ] ;
               <http://purl.org/dc/terms/created> "2021-04-02"^^xsd:date ;
               <http://purl.org/dc/terms/modified> "2022-07-07"^^xsd:date ;
               rdfs:comment "A section of line means the part of line between adjacent operational points and may consist of several tracks."@en ;
               rdfs:isDefinedBy <http://data.europa.eu/949/> ;
               rdfs:label "Section Of Line"@en ;
               <http://www.w3.org/2003/06/sw-vocab-status/ns#term_status> "stable" .


###  http://data.europa.eu/949/Siding
:Siding rdf:type owl:Class ;
        rdfs:subClassOf :PhysicalImplementationFeature ;
        <http://purl.org/dc/terms/created> "2021-08-10"^^xsd:date ;
        <http://purl.org/dc/terms/modified> "2022-07-07"^^xsd:date ;
        <http://purl.org/dc/terms/source> "Official Journal of the European Union L 139 I/85" ;
        rdfs:comment "Sidings are all those tracks where running trains in service movements ends and which are not used for operational routing of a train."@en ;
        rdfs:isDefinedBy <http://data.europa.eu/949/> ;
        rdfs:label "Siding"@en ;
        <http://www.w3.org/2003/06/sw-vocab-status/ns#term_status> "stable" ;
        <http://www.w3.org/2004/02/skos/core#definition> "Siding Any track(s) within an operational point which is not used for operational routing of a train."@en .


###  http://data.europa.eu/949/Signal
:Signal rdf:type owl:Class ;
        rdfs:subClassOf :OperationalPoint ;
        <http://purl.org/dc/terms/created> "2021-04-01"^^xsd:date ;
        <http://purl.org/dc/terms/modified> "2021-04-01"^^xsd:date ;
        rdfs:comment "A railway signal is an installation next to the railway track for signalling the maximum allowed speed in the next block section to the train driver."@en ;
        rdfs:isDefinedBy <http://data.europa.eu/949/> ;
        rdfs:label "Signal"@en ;
        rdfs:seeAlso "https://wiki3.railml.org/DataModel/3.1/IS/" ;
        <http://www.w3.org/2003/06/sw-vocab-status/ns#term_status> "stable" .


###  http://data.europa.eu/949/SpeedSection
:SpeedSection rdf:type owl:Class ;
              rdfs:subClassOf rdf:Bag ;
              rdfs:isDefinedBy <http://data.europa.eu/949/> ;
              rdfs:label "Speed Section"@en .


###  http://data.europa.eu/949/SpotLocation
:SpotLocation rdf:type owl:Class ;
              <http://purl.org/dc/terms/created> "2022-05-04"^^xsd:date ;
              <http://purl.org/dc/terms/source> "https://wiki3.railml.org/wiki/RTM:spotLocation"^^xsd:anyURI ;
              rdfs:isDefinedBy <http://data.europa.eu/949/> ;
              rdfs:label "Spot Location"@en ;
              <http://www.w3.org/2003/06/sw-vocab-status/ns#term_status> "unstable" .


###  http://data.europa.eu/949/Station
:Station rdf:type owl:Class ;
         rdfs:subClassOf :PrincipalLocation ;
         rdfs:isDefinedBy <http://data.europa.eu/949/> ;
         rdfs:label "Station"@en .


###  http://data.europa.eu/949/StoppingPlace
:StoppingPlace rdf:type owl:Class ;
               rdfs:subClassOf :SpotLocation ;
               <http://purl.org/dc/terms/created> "2022-05-04"^^xsd:date ;
               <http://purl.org/dc/terms/source> "https://wiki3.railml.org/wiki/IS:stoppingPlace"^^xsd:anyURI ;
               rdfs:isDefinedBy <http://data.europa.eu/949/> ;
               rdfs:label "Stopping Place"@en ;
               <http://www.w3.org/2003/06/sw-vocab-status/ns#term_status> "unstable" .


###  http://data.europa.eu/949/Switch
:Switch rdf:type owl:Class ;
        rdfs:subClassOf :OperationalPoint ;
        <http://purl.org/dc/terms/source> "https://otl.prorail.nl/imx/vigerend/ERTMSSwitch"^^xsd:anyURI ,
                                          "https://wiki2.railml.org/wiki/IS:switch"^^xsd:anyURI ;
        rdfs:isDefinedBy <http://data.europa.eu/949/> ;
        rdfs:label "switch"@en .


###  http://data.europa.eu/949/TopologicalObject
:TopologicalObject rdf:type owl:Class ;
                   rdfs:subClassOf :EraFeature ;
                   <http://purl.org/dc/terms/created> "2022-05-04"^^xsd:date ;
                   rdfs:isDefinedBy <http://data.europa.eu/949/> ;
                   rdfs:label "Topological Object"@en ;
                   <http://www.w3.org/2003/06/sw-vocab-status/ns#term_status> "unstable" .


###  http://data.europa.eu/949/Track
:Track rdf:type owl:Class ;
       rdfs:subClassOf :PhysicalImplementationFeature ;
       <http://purl.org/dc/terms/created> "2020-07-29"^^xsd:date ;
       <http://purl.org/dc/terms/modified> "2022-07-07"^^xsd:date ;
       rdfs:comment "A running track that is used for train service movements."@en ;
       rdfs:isDefinedBy <http://data.europa.eu/949/> ;
       rdfs:label "Track"@en ;
       <http://www.w3.org/2003/06/sw-vocab-status/ns#term_status> "stable" .


###  http://data.europa.eu/949/TrainDetectionSystem
:TrainDetectionSystem rdf:type owl:Class ;
                      <http://purl.org/dc/terms/created> "2021-08-07"^^xsd:date ;
                      <http://purl.org/dc/terms/modified> "2021-08-07"^^xsd:date ;
                      rdfs:comment "System used to detect the position of vehicles in the railway track."@en ;
                      rdfs:isDefinedBy <http://data.europa.eu/949/> ;
                      rdfs:label "Train Detection System"@en ;
                      <http://www.w3.org/2003/06/sw-vocab-status/ns#term_status> "stable" .


###  http://data.europa.eu/949/Tunnel
:Tunnel rdf:type owl:Class ;
        rdfs:subClassOf :PhysicalImplementationFeature ;
        <http://purl.org/dc/terms/created> "2020-07-29"^^xsd:date ;
        <http://purl.org/dc/terms/modified> "2022-07-07"^^xsd:date ;
        rdfs:comment "A railway tunnel is an excavation or a construction around the track provided to allow the railway to pass for example higher land, buildings or water."@en ;
        rdfs:isDefinedBy <http://data.europa.eu/949/> ;
        rdfs:label "Tunnel"@en ;
        <http://www.w3.org/2003/06/sw-vocab-status/ns#term_status> "stable" .


###  http://data.europa.eu/949/ValidityPeriod
:ValidityPeriod rdf:type owl:Class ;
                <http://purl.org/dc/terms/created> "2022-10-21"^^xsd:date ;
                rdf:label "Validity period"@en ;
                rdfs:comment "Class to define validity start date and validity end date for objects in the infrastructure such as operational points."@en ;
                rdfs:isDefinedBy "http://data.europa.eu/949/"^^xsd:anyURI ;
                <http://www.w3.org/2003/06/sw-vocab-status/ns#term_status> "stable" .


###  http://data.europa.eu/949/Vehicle
:Vehicle rdf:type owl:Class ;
         <http://purl.org/dc/terms/created> "2020-11-22"^^xsd:date ;
         <http://purl.org/dc/terms/modified> "2020-11-22"^^xsd:date ;
         rdfs:comment "A specific vehicle or wagon able to operate over railway lines."@en ;
         rdfs:isDefinedBy <http://data.europa.eu/949/> ;
         rdfs:label "Vehicle"@en ;
         <http://www.w3.org/2003/06/sw-vocab-status/ns#term_status> "stable" .


###  http://data.europa.eu/949/VehicleKeeper
:VehicleKeeper rdf:type owl:Class ;
               rdfs:subClassOf <http://www.w3.org/ns/org#Organization> ;
               <http://purl.org/dc/terms/created> "2020-11-23"^^xsd:date ;
               <http://purl.org/dc/terms/modified> "2020-11-23"^^xsd:date ;
               rdfs:comment "A company or organization that owns or operates a certain vehicle."@en ;
               rdfs:isDefinedBy <http://data.europa.eu/949/> ;
               rdfs:label "Vehicle Keeper"@en ;
               <http://www.w3.org/2003/06/sw-vocab-status/ns#term_status> "stable" .


###  http://data.europa.eu/949/VehicleType
:VehicleType rdf:type owl:Class ;
             rdfs:subClassOf [ rdf:type owl:Restriction ;
                               owl:onProperty :manufacturer ;
                               owl:qualifiedCardinality "1"^^xsd:nonNegativeInteger ;
                               owl:onClass :Manufacturer
                             ] ;
             <http://purl.org/dc/terms/created> "2020-07-29"^^xsd:date ;
             <http://purl.org/dc/terms/modified> "2020-07-29"^^xsd:date ;
             rdfs:comment "A vehicle type that has been authorized to operate on the EU railway infrastructure."@en ;
             rdfs:isDefinedBy <http://data.europa.eu/949/> ;
             rdfs:label "Vehicle Type"@en ;
             <http://www.w3.org/2003/06/sw-vocab-status/ns#term_status> "stable" .


###  http://www.w3.org/1999/02/22-rdf-syntax-ns#Bag
rdf:Bag rdf:type owl:Class .


###  http://www.w3.org/2000/01/rdf-schema#Resource
rdfs:Resource rdf:type owl:Class .


###  http://www.w3.org/2003/01/geo/wgs84_pos#Point
<http://www.w3.org/2003/01/geo/wgs84_pos#Point> rdf:type owl:Class ;
                                                rdfs:subClassOf <http://www.w3.org/2003/01/geo/wgs84_pos#SpatialThing> ;
                                                rdfs:comment """ 
Uniquely identified by lat/long/alt. i.e.

spaciallyIntersects(P1, P2) :- lat(P1, LAT), long(P1, LONG), alt(P1, ALT),
  lat(P2, LAT), long(P2, LONG), alt(P2, ALT).

sameThing(P1, P2) :- type(P1, Point), type(P2, Point), spaciallyIntersects(P1, P2).
  """ ,
                                                             """A point, typically described using a coordinate system relative to Earth, such as WGS84.
  """ ;
                                                rdfs:label "point" .


###  http://www.w3.org/2003/01/geo/wgs84_pos#SpatialThing
<http://www.w3.org/2003/01/geo/wgs84_pos#SpatialThing> rdf:type owl:Class ;
                                                       rdfs:comment """Anything with spatial extent, i.e. size, shape, or position.
 e.g. people, places, bowling balls, as well as abstract areas like cubes.
""" ;
                                                       rdfs:label "SpatialThing" .


###  http://www.w3.org/ns/org#Organization
<http://www.w3.org/ns/org#Organization> rdf:type owl:Class .


#################################################################
#    Individuals
#################################################################

###  http://data.europa.eu/949/concepts/op-types/borderStation
<http://data.europa.eu/949/concepts/op-types/borderStation> rdf:type owl:NamedIndividual .


###  http://data.europa.eu/949/concepts/op-types/station
<http://data.europa.eu/949/concepts/op-types/station> rdf:type owl:NamedIndividual .


#################################################################
#    Annotations
#################################################################

<http://www.w3.org/2003/01/geo/wgs84_pos#> <http://purl.org/dc/elements/1.1/date> "$Date: 2009/04/20 15:00:30 $" ;
                                           <http://purl.org/dc/elements/1.1/description> """A vocabulary for representing latitude, longitude and 
 altitude information in the WGS84 geodetic reference datum. 
 Version $Id: wgs84_pos.rdf,v 1.22 2009/04/20 15:00:30 timbl Exp $. See http://www.w3.org/2003/01/geo/ for more details.""" ;
                                           <http://purl.org/dc/elements/1.1/title> "WGS84 Geo Positioning: an RDF vocabulary" ;
                                           rdfs:comment """
Recent changes to this namespace:
$Log: wgs84_pos.rdf,v $
Revision 1.22  2009/04/20 15:00:30  timbl
Remove the time bits which have been deal with elsewhere eg in iCal.

Revision 1.21  2009/04/20 12:52:47  timbl
try again

Revision 1.20  2009/04/20 12:42:11  timbl
Add Event (edited ages ago and never checked in), and location (following discussion http://chatlogs.planetrdf.com/swig/2009-04-20#T12-36-09)

Revision 1.19  2009/04/20 12:36:31  timbl
Add Event (edited ages ago and never checked in), and location (following discussion http://chatlogs.planetrdf.com/swig/2009-04-20#T12-36-09)

Revision 1.18  2006/02/01 22:01:04  danbri
Clarified that lat and long are decimal degrees, and that alt is decimal metres about local reference ellipsoid

Revision 1.17  2004/02/06 17:38:12  danbri
Fixed a bad commit screwup

Revision 1.15  2003/04/19 11:24:08  danbri
Fixed the typo even more.

Revision 1.14  2003/04/19 11:16:56  danbri
fixed a typo

Revision 1.13  2003/02/19 22:27:27  connolly
relaxed domain constraints on lat/long/alt from Point to SpatialThing

Revision 1.12  2003/01/12 01:41:41  danbri
Trying local copy of XSLT doc.

Revision 1.11  2003/01/12 01:20:18  danbri
added a link to morten's xslt rdfs viewer.

Revision 1.10  2003/01/11 18:56:49  danbri
Removed datatype range from lat and long properties, since they would
have required each occurance of the property to mention the datatype.

Revision 1.9  2003/01/11 11:41:31  danbri
Another typo; repaired rdfs:Property to rdf:Property x4

Revision 1.8  2003/01/11 11:05:02  danbri
Added an rdfs:range for each lat/long/alt property,
http://www.w3.org/2001/XMLSchema#float

Revision 1.7  2003/01/10 20:25:16  danbri
Longer rdfs:comment for Point, trying to be Earth-centric and neutral about
coordinate system(s) at the same time. Feedback welcomed.

Revision 1.6  2003/01/10 20:18:30  danbri
Added CVS log comments into the RDF/XML as an rdfs:comment property of the
vocabulary. Note that this is not common practice (but seems both harmless
and potentially useful).


revision 1.5
date: 2003/01/10 20:14:31;  author: danbri;  state: Exp;  lines: +16 -5
Updated schema:
Added a dc:date, added url for more info. Changed the rdfs:label of the
namespace from gp to geo. Added a class Point, set as the rdfs:domain of
each property. Added XML comment on the lat_long property suggesting that
we might not need it (based on #rdfig commentary from implementors).

revision 1.4
date: 2003/01/10 20:01:07;  author: danbri;  state: Exp;  lines: +6 -5
Fixed typo; several rdfs:about attributes are now rdf:about. Thanks to MortenF in
#rdfig for catching this error.

revision 1.3
date: 2003/01/10 11:59:03;  author: danbri;  state: Exp;  lines: +4 -3
fixed buglet in vocab, added more wgs links

revision 1.2
date: 2003/01/10 11:01:11;  author: danbri;  state: Exp;  lines: +4 -4
Removed alt from the as-a-flat-string property, and switched from
space separated to comma separated.

revision 1.1
date: 2003/01/10 10:53:23;  author: danbri;  state: Exp;
basic geo vocab

""" ;
                                           rdfs:label "geo" .


<http://www.w3.org/2003/01/geo/wgs84_pos#lat_long> rdfs:comment "A comma-separated representation of a latitude, longitude coordinate." ;
                                                   rdfs:label "lat/long" .


<http://www.w3.org/2003/01/geo/wgs84_pos#location> :isCoreParameter "true"^^xsd:boolean ;
                                                   rdfs:comment """The relation between something and the point, 
 or other geometrical thing in space, where it is.  For example, the realtionship between
 a radio tower and a Point with a given lat and long.
 Or a relationship between a park and its outline as a closed arc of points, or a road and
 its location as a arc (a sequence of points).
 Clearly in practice there will be limit to the accuracy of any such statement, but one would expect
 an accuracy appropriate for the size of the object and uses such as mapping .
 """ ;
                                                   rdfs:label "location" .


###  Generated by the OWL API (version 5.1.18) https://github.com/owlcs/owlapi/
